@prefix owl:   <http://www.w3.org/2002/07/owl#> .
@prefix dct:   <http://purl.org/dc/terms/> .
@prefix rdfs:  <http://www.w3.org/2000/01/rdf-schema#> .
@prefix prov:  <http://www.w3.org/ns/prov#> .
@prefix rdf:   <http://www.w3.org/1999/02/22-rdf-syntax-ns#> .
@prefix ids:   <https://w3id.org/idsa/core/> .
@prefix vann:  <http://purl.org/vocab/vann/> .
@prefix void:  <http://rdfs.org/ns/void#> .
@prefix voaf:  <http://purl.org/vocommons/voaf#> .
@prefix foaf:  <http://xmlns.com/foaf/0.1/> .
@prefix cc:    <http://creativecommons.org/ns#> .
@prefix xsd:   <http://www.w3.org/2001/XMLSchema#> .

ids:    rdf:type                       voaf:Vocabulary ;
        rdf:type                       owl:Ontology ;
        rdfs:isDefinedBy               ids: ;
        rdfs:label                     "IDS Information Model"@en ;
        dct:title                      "The International Data Spaces Information Model"@en ;
        rdfs:comment                   "This ontology defines classes and properties for describing participants, infrastructure, data and services of the International Data Spaces (formerly known as Industrial Data Space)." ;
        cc:license                     <http://www.apache.org/licenses/LICENSE-2.0> ;
        dct:creator                    <https://github.com/cmader> ;
        dct:creator                    <https://github.com/jpullmann> ;
        dct:creator                    <http://sebastian.tramp.name> ;
        dct:contributor                _:b0 ;
        dct:contributor                _:b1 ;
        dct:contributor                <https://github.com/sebbader> ;
        dct:contributor                <https://github.com/Maboeckmann> ;
        dct:contributor                <https://github.com/clange> ;
        dct:contributor                <https://github.com/HaydarAk> ;
        dct:contributor                <https://github.com/jlangkau> ;
        dct:contributor                <https://github.com/JohannesLipp> ;
        dct:contributor                <https://github.com/mkollenstart> ;
        dct:contributor                <https://github.com/lcomet> ;
        dct:publisher                  ids:IDSA ;
        dct:created                    "2017-09-26"^^xsd:date ;
        dct:modified                   "2021-10-07"^^xsd:date ;
        owl:versionInfo                "4.2.0" ;
        owl:versionIRI                 ids:4.2.0 ;
        vann:preferredNamespaceUri     "https://w3id.org/idsa/core/" ;
        vann:preferredNamespacePrefix  "ids" ;
        rdfs:seeAlso                   <https://international-data-spaces-association.github.io/InformationModel/> ;
        void:vocabulary                vann: ;
        void:vocabulary                void: ;
        void:vocabulary                voaf: ;
        void:vocabulary                dct: ;
        void:vocabulary                foaf: .

<http://www.apache.org/licenses/LICENSE-2.0>
        rdfs:label  "Apache License Version 2.0, January 2004" .

ids:IDSA  rdf:type     dct:Agent ;
        rdf:type       foaf:Organization ;
        foaf:homepage  <https://www.internationaldataspaces.org> ;
        rdfs:label     "International Data Spaces Association" .

<http://sebastian.tramp.name>
        rdf:type   dct:Agent ;
        rdf:type   foaf:Person ;
        foaf:name  "Sebastian Tramp" .

<https://github.com/cmader>
        rdf:type   dct:Agent ;
        rdf:type   foaf:Person ;
        foaf:name  "Christian Mader" .

<https://github.com/jpullmann>
        rdf:type   dct:Agent ;
        rdf:type   foaf:Person ;
        foaf:name  "Jaroslav Pullmann" .

_:b0    rdf:type   dct:Agent ;
        rdf:type   foaf:Person ;
        foaf:name  "Andreas Müller" .

_:b1    rdf:type   dct:Agent ;
        rdf:type   foaf:Person ;
        foaf:name  "Anna Kasprzik" .

<https://github.com/sebbader>
        rdf:type   dct:Agent ;
        rdf:type   foaf:Person ;
        foaf:name  "Sebastian Bader" .

<https://github.com/HaydarAk>
        rdf:type   dct:Agent ;
        rdf:type   foaf:Person ;
        foaf:name  "Haydar Akyürek" .

<https://github.com/JohannesLipp>
        rdf:type   dct:Agent ;
        rdf:type   foaf:Person ;
        foaf:name  "Johannes Lipp" .

<https://github.com/clange>
        rdf:type   dct:Agent ;
        rdf:type   foaf:Person ;
        foaf:name  "Christoph Lange" .

<https://github.com/Maboeckmann>
        rdf:type   dct:Agent ;
        rdf:type   foaf:Person ;
        foaf:name  "Matthias Böckmann" .

<https://github.com/jlangkau>
        rdf:type   dct:Agent ;
        rdf:type   foaf:Person ;
        foaf:name  "Jörg Langkau" .

<https://github.com/mkollenstart>
        rdf:type   dct:Agent ;
        rdf:type   foaf:Person ;
        foaf:name  "Maarten Kollenstart" .

<https://github.com/JohannesLipp>
        rdf:type   dct:Agent ;
        rdf:type   foaf:Person ;
        foaf:name  "Johannes Theissen-Lipp" .

<https://github.com/lcomet>
        rdf:type   dct:Agent ;
        rdf:type   foaf:Person ;
        foaf:name  "Lina Molinas Comet" .

ids:    owl:imports  <file:///wdir/InformationModel/ttl-sources/model/adms.ttl> ;
        owl:imports  <file:///wdir/InformationModel/ttl-sources/model/communication/AppRoute.ttl> ;
        owl:imports  <file:///wdir/InformationModel/ttl-sources/model/communication/Endpoint.ttl> ;
        owl:imports  <file:///wdir/InformationModel/ttl-sources/model/communication/Message.ttl> ;
        owl:imports  <file:///wdir/InformationModel/ttl-sources/model/communication/Proxy.ttl> ;
        owl:imports  <file:///wdir/InformationModel/ttl-sources/model/content/Artifact.ttl> ;
        owl:imports  <file:///wdir/InformationModel/ttl-sources/model/content/ArtifactState.ttl> ;
        owl:imports  <file:///wdir/InformationModel/ttl-sources/model/content/Asset.ttl> ;
        owl:imports  <file:///wdir/InformationModel/ttl-sources/model/content/Concept.ttl> ;
        owl:imports  <file:///wdir/InformationModel/ttl-sources/model/content/ContentType.ttl> ;
        owl:imports  <file:///wdir/InformationModel/ttl-sources/model/content/DataApp.ttl> ;
        owl:imports  <file:///wdir/InformationModel/ttl-sources/model/content/DigitalContent.ttl> ;
        owl:imports  <file:///wdir/InformationModel/ttl-sources/model/content/Language.ttl> ;
        owl:imports  <file:///wdir/InformationModel/ttl-sources/model/content/MediaType.ttl> ;
        owl:imports  <file:///wdir/InformationModel/ttl-sources/model/content/PaymentModalities.ttl> ;
        owl:imports  <file:///wdir/InformationModel/ttl-sources/model/content/Representation.ttl> ;
        owl:imports  <file:///wdir/InformationModel/ttl-sources/model/content/Resource.ttl> ;
        owl:imports  <file:///wdir/InformationModel/ttl-sources/model/content/UsageControlObject.ttl> ;
        owl:imports  <file:///wdir/InformationModel/ttl-sources/model/context/Event.ttl> ;
        owl:imports  <file:///wdir/InformationModel/ttl-sources/model/context/SpatialEntity.ttl> ;
        owl:imports  <file:///wdir/InformationModel/ttl-sources/model/context/TemporalEntity.ttl> ;
        owl:imports  <file:///wdir/InformationModel/ttl-sources/model/contract/Action.ttl> ;
        owl:imports  <file:///wdir/InformationModel/ttl-sources/model/contract/BinaryOperator.ttl> ;
        owl:imports  <file:///wdir/InformationModel/ttl-sources/model/contract/Constraint.ttl> ;
        owl:imports  <file:///wdir/InformationModel/ttl-sources/model/contract/Contract.ttl> ;
        owl:imports  <file:///wdir/InformationModel/ttl-sources/model/contract/LeftOperand.ttl> ;
        owl:imports  <file:///wdir/InformationModel/ttl-sources/model/contract/Rule.ttl> ;
        owl:imports  <file:///wdir/InformationModel/ttl-sources/model/contract/UsagePolicyClass.ttl> ;
        owl:imports  <file:///wdir/InformationModel/ttl-sources/model/governance/Certification.ttl> ;
        owl:imports  <file:///wdir/InformationModel/ttl-sources/model/governance/License.ttl> ;
        owl:imports  <file:///wdir/InformationModel/ttl-sources/model/infrastructure/AppStore.ttl> ;
        owl:imports  <file:///wdir/InformationModel/ttl-sources/model/infrastructure/Broker.ttl> ;
        owl:imports  <file:///wdir/InformationModel/ttl-sources/model/infrastructure/Catalog.ttl> ;
        owl:imports  <file:///wdir/InformationModel/ttl-sources/model/infrastructure/ClearingHouse.ttl> ;
        owl:imports  <file:///wdir/InformationModel/ttl-sources/model/infrastructure/ConfigurationModel.ttl> ;
        owl:imports  <file:///wdir/InformationModel/ttl-sources/model/infrastructure/Connector.ttl> ;
        owl:imports  <file:///wdir/InformationModel/ttl-sources/model/infrastructure/DAPS.ttl> ;
        owl:imports  <file:///wdir/InformationModel/ttl-sources/model/infrastructure/IdentityProvider.ttl> ;
        owl:imports  <file:///wdir/InformationModel/ttl-sources/model/infrastructure/InfrastructureComponent.ttl> ;
        owl:imports  <file:///wdir/InformationModel/ttl-sources/model/infrastructure/ParIS.ttl> ;
        owl:imports  <file:///wdir/InformationModel/ttl-sources/model/infrastructure/PublicKey.ttl> ;
        owl:imports  <file:///wdir/InformationModel/ttl-sources/model/participant/BusinessIdentifier.ttl> ;
        owl:imports  <file:///wdir/InformationModel/ttl-sources/model/participant/Participant.ttl> ;
        owl:imports  <file:///wdir/InformationModel/ttl-sources/model/security/AuthInfo.ttl> ;
        owl:imports  <file:///wdir/InformationModel/ttl-sources/model/security/AuthStandard.ttl> ;
        owl:imports  <file:///wdir/InformationModel/ttl-sources/model/security/SecurityProfile.ttl> ;
        owl:imports  <file:///wdir/InformationModel/ttl-sources/model/security/Token.ttl> ;
        owl:imports  <file:///wdir/InformationModel/ttl-sources/model/security/UserAuthentication.ttl> ;
        owl:imports  <file:///wdir/InformationModel/ttl-sources/model/shared/Described.ttl> ;
        owl:imports  <file:///wdir/InformationModel/ttl-sources/model/shared/DescribedSemantically.ttl> ;
        owl:imports  <file:///wdir/InformationModel/ttl-sources/model/shared/Named.ttl> ;
        owl:imports  <file:///wdir/InformationModel/ttl-sources/model/traceability/ConnectorDeployMode.ttl> ;
        owl:imports  <file:///wdir/InformationModel/ttl-sources/model/traceability/ConnectorStatus.ttl> ;
        owl:imports  <file:///wdir/InformationModel/ttl-sources/model/traceability/LogLevel.ttl> ;
        owl:imports  <file:///wdir/InformationModel/ttl-sources/model/traceability/ManagedEntity.ttl> ;
        owl:imports  <file:///wdir/InformationModel/ttl-sources/taxonomies/Certification.ttl> ;
        owl:imports  <file:///wdir/InformationModel/ttl-sources/taxonomies/Contract.ttl> ;
        owl:imports  <file:///wdir/InformationModel/ttl-sources/taxonomies/Message.ttl> ;
        owl:imports  <file:///wdir/InformationModel/ttl-sources/taxonomies/Representation.ttl> ;
        owl:imports  <file:///wdir/InformationModel/ttl-sources/taxonomies/Resource.ttl> ;
        owl:imports  <file:///wdir/InformationModel/ttl-sources/codes/Action.ttl> ;
        owl:imports  <file:///wdir/InformationModel/ttl-sources/codes/AppEndpointType.ttl> ;
        owl:imports  <file:///wdir/InformationModel/ttl-sources/codes/ArtifactState.ttl> ;
        owl:imports  <file:///wdir/InformationModel/ttl-sources/codes/Audience.ttl> ;
        owl:imports  <file:///wdir/InformationModel/ttl-sources/codes/BinaryOperators.ttl> ;
        owl:imports  <file:///wdir/InformationModel/ttl-sources/codes/CertificationLevel.ttl> ;
        owl:imports  <file:///wdir/InformationModel/ttl-sources/codes/ConnectorDeployMode.ttl> ;
        owl:imports  <file:///wdir/InformationModel/ttl-sources/codes/ConnectorStatus.ttl> ;
        owl:imports  <file:///wdir/InformationModel/ttl-sources/codes/ContentType.ttl> ;
        owl:imports  <file:///wdir/InformationModel/ttl-sources/codes/Frequency.ttl> ;
        owl:imports  <file:///wdir/InformationModel/ttl-sources/codes/KeyType.ttl> ;
        owl:imports  <file:///wdir/InformationModel/ttl-sources/codes/Language.ttl> ;
        owl:imports  <file:///wdir/InformationModel/ttl-sources/codes/LeftOperand.ttl> ;
        owl:imports  <file:///wdir/InformationModel/ttl-sources/codes/LogLevel.ttl> ;
        owl:imports  <file:///wdir/InformationModel/ttl-sources/codes/Mediatype.ttl> ;
        owl:imports  <file:///wdir/InformationModel/ttl-sources/codes/PaymentModality.ttl> ;
        owl:imports  <file:///wdir/InformationModel/ttl-sources/codes/QueryLanguage.ttl> ;
        owl:imports  <file:///wdir/InformationModel/ttl-sources/codes/QueryScope.ttl> ;
        owl:imports  <file:///wdir/InformationModel/ttl-sources/codes/QueryTarget.ttl> ;
        owl:imports  <file:///wdir/InformationModel/ttl-sources/codes/RejectionReason.ttl> ;
        owl:imports  <file:///wdir/InformationModel/ttl-sources/codes/RequestTemplate.ttl> ;
        owl:imports  <file:///wdir/InformationModel/ttl-sources/codes/SecurityGuarantee.ttl> ;
        owl:imports  <file:///wdir/InformationModel/ttl-sources/codes/TokenFormat.ttl> ;
        owl:imports  <file:///wdir/InformationModel/ttl-sources/codes/UsagePolicyClass.ttl> .
@prefix owl:   <http://www.w3.org/2002/07/owl#> .
@prefix rdfs:  <http://www.w3.org/2000/01/rdf-schema#> .
@prefix xsd:   <http://www.w3.org/2001/XMLSchema#> .
@prefix ids:   <https://w3id.org/idsa/core/> .

ids:AppRoute  rdf:type  owl:Class ;
        rdfs:label    "App Route"@en ;
        rdfs:comment  "\n    ids:AppRoute describes the communication between data apps (such as in a data processing pipeline) inside an IDS Connector.\n    An ids:AppRoute consist of multiple app endpoints which exchange data. The communication pipeline between two adjacent data apps is represented by the ids:RouteStep class.\n    ids:AppRoute also holds the information about the app endpoints, which are at the start and end of the whole processing pipeline.\n    "@en .

ids:RouteStep  rdf:type  owl:Class ;
        rdfs:subClassOf  ids:AppRoute ;
        rdfs:label       "Route step"@en ;
        rdfs:comment     "RouteSteps hold information about a communication pipelines between apps. A RouteStep should hold\n    one value for the ids:appRouteStart and/or ids:appRouteEnd properties, so that communication between app endpoints remain distinguishable.\n    "@en .

ids:routeDeployMethod
        rdf:type      owl:DatatypeProperty ;
        rdfs:label    "route deploy method"@en ;
        rdfs:domain   ids:AppRoute ;
        rdfs:range    xsd:string ;
        rdfs:comment  "Supplementary information about, e.g., the technology used, for routes." .

ids:routeDescription  rdf:type  owl:DatatypeProperty ;
        rdfs:label    "route description "@en ;
        rdfs:domain   ids:AppRoute ;
        rdfs:range    xsd:string ;
        rdfs:comment  "Route description."@en .

ids:routeConfiguration
        rdf:type      owl:DatatypeProperty ;
        rdfs:label    "route configuration"@en ;
        rdfs:domain   ids:AppRoute ;
        rdfs:range    xsd:string ;
        rdfs:comment  "Configuration details (e.g., contents of a config file) used to configure the route. Should be Base64 encoded."@en .

ids:hasSubRoute  rdf:type  owl:ObjectProperty ;
        rdfs:label    "sub route"@en ;
        rdfs:domain   ids:AppRoute ;
        rdfs:range    ids:RouteStep ;
        rdfs:comment  "Route between two or more app endpoints inside a app routing pipeline."@en .

ids:appRouteStart  rdf:type  owl:ObjectProperty ;
        rdfs:label    "app route start"@en ;
        rdfs:domain   ids:AppRoute ;
        rdfs:range    ids:Endpoint ;
        rdfs:comment  "Start of a route."@en .

ids:appRouteEnd  rdf:type  owl:ObjectProperty ;
        rdfs:label    "app route end"@en ;
        rdfs:domain   ids:AppRoute ;
        rdfs:range    ids:Endpoint ;
        rdfs:comment  "End of a route."@en .

ids:appRouteOutput  rdf:type  owl:ObjectProperty ;
        rdfs:domain   ids:AppRoute ;
        rdfs:range    ids:Resource ;
        rdfs:label    "app route output"@en ;
        rdfs:comment  "ids:Resource that corresponds to the output of an app route.\nRationale: whereas an ids:Endpoint can have an ids:endpointArtifact, it is additionally important that the data flow inside the ids:Connector / ids:ConfigurationModel is aware of the ids:ContractOffer (a property of ids:Resource!) associated with the data coming into the Connector or going out of the Connector.\nUse: Whenever properties of this Resource change, it may make sense to notify the ids:broker(s) configured for this AppRoute.\nNote: In an ids:AppRoute that is the sequence of multiple ids:RouteSteps, the output resource of one step serves immediately as the input that is processed by the subsequent step(s).  An ids:SystemAdapter typically does not change the ids:Resource, but might rather make it available in a different dcat:Distribution.  An ids:SmartDataApp might replate its input(s) by an entirely different (e.g., fused) resource.\n"@en .

ids:appRouteBroker  rdf:type  owl:ObjectProperty ;
        rdfs:domain   ids:AppRoute ;
        rdfs:range    ids:Broker ;
        rdfs:label    "app route broker"@en ;
        rdfs:comment  "One or more ids:Broker(s) to which changes/updates of this route's ids:appRouteOutput ids:Resource are announced.\nThis should be a subset of those Brokers that have been configured as ids:configuredBrokers in the ids:ConfigurationModel of which this is an ids:appRoute.\n"@en .

ids:appRouteClearingHouse
        rdf:type      owl:ObjectProperty ;
        rdfs:domain   ids:AppRoute ;
        rdfs:range    ids:ClearingHouse ;
        rdfs:label    "app route broker"@en ;
        rdfs:comment  "One or more ids:ClearingHouse(s) to which information of this route's data exchange are notified.\nThis should be a subset of clearing houses listed in the corresponding ids:ClearingHouseCatalog for a given configuration model. The Configuration Model ids:configuredClearingHouse in the ids:ConfigurationModel of which this is an ids:appRoute.\n"@en .

ids:requiredDataApp  rdf:type  owl:ObjectProperty ;
        rdfs:domain   ids:RouteStep ;
        rdfs:range    ids:AppRepresentation ;
        rdfs:label    "requiredDataApp"@en ;
        rdfs:comment  "Refers to the concrete app representation (ids:AppRepresentation) for a data app (ids:DataApp) which is deployed in the Connector maintained by the Configuration Model and\n    whoose endpoint (ids:AppEndpoint) is used in this ids:RouteStep. The referred app representation should be part of the catalog of AppResources in the\n    corresponding Configuration Model (cf. ids:configuredAppResource property in class ids:ConfigurationModel).\n    "@en .
@prefix owl:   <http://www.w3.org/2002/07/owl#> .
@prefix rdf:   <http://www.w3.org/1999/02/22-rdf-syntax-ns#> .
@prefix rdfs:  <http://www.w3.org/2000/01/rdf-schema#> .
@prefix xsd:   <http://www.w3.org/2001/XMLSchema#> .
@prefix dct:   <http://purl.org/dc/terms/> .
@prefix ids:   <https://w3id.org/idsa/core/> .

ids:Endpoint  rdf:type  owl:Class ;
        rdfs:label    "Endpoint"@en ;
        rdfs:comment  "Access point of data exchange, service interaction and service description."@en .

ids:ConnectorEndpoint
        rdf:type         owl:Class ;
        rdfs:subClassOf  ids:Endpoint ;
        rdfs:label       "Connector Endpoint"@en ;
        rdfs:comment     "Connector-specific endpoint exposing Artifacts."@en .

ids:AppEndpoint  rdf:type  owl:Class ;
        rdfs:subClassOf  ids:Endpoint ;
        rdfs:label       "DataApp Endpoint"@en ;
        rdfs:comment     "Description of endpoints a DataApp offers."@en .

ids:AppEndpointType  rdf:type  owl:Class ;
        rdfs:label    "App endpoint type"@en ;
        rdfs:comment  "Class of endpoint types a data app offers."@en .

ids:GenericEndpoint  rdf:type  owl:Class ;
        rdfs:subClassOf  ids:Endpoint ;
        rdfs:label       "Generic Endpoint"@en ;
        rdfs:comment     "Generic endpoints describe non-IDS-specific endpoints, e.g., to integrate external services."@en .

ids:IdsProtocolSpecification
        rdf:type      owl:Class ;
        rdfs:label    "Protocol Specification" ;
        rdfs:comment  "List of all defined Protocol Specifications, for instance IDS-CP or IDS over Multipart."@en .

ids:accessURL  rdf:type  owl:DatatypeProperty ;
        rdfs:label    "access URL"@en ;
        rdfs:domain   ids:Endpoint ;
        rdfs:range    xsd:anyURI ;
        rdfs:comment  "Access URL of an endpoint."@en ;
        rdfs:seeAlso  <https://tools.ietf.org/html/rfc3986#section-3> .

ids:endpointInformation
        rdf:type      owl:DatatypeProperty ;
        rdfs:domain   ids:Endpoint ;
        rdfs:range    xsd:string ;
        rdfs:label    "endpoint information"@en ;
        rdfs:comment  "Human-readable information and description of the endpoint."@en .

ids:endpointDocumentation
        rdf:type      owl:DatatypeProperty ;
        rdfs:domain   ids:Endpoint ;
        rdfs:range    xsd:anyURI ;
        rdfs:label    "endpoint documentation"@en ;
        rdfs:comment  "IRI reference to a documentation of the endpoint, e.g., reference to an OpenAPI-based documentation."@en .

ids:endpointArtifact  rdf:type  owl:ObjectProperty ;
        rdfs:label    "endpoint artifact"@en ;
        rdfs:domain   ids:ConnectorEndpoint ;
        rdfs:range    ids:Artifact ;
        rdfs:comment  "Content instance mediated via this individual endpoint (1:1 mapping)."@en .

ids:path  rdf:type    owl:DatatypeProperty ;
        rdfs:label    "path"@en ;
        rdfs:domain   ids:Endpoint ;
        rdfs:range    xsd:string ;
        rdfs:comment  "Relative path, topic or queue at which the content is published by the related host."@en .

ids:inboundPath  rdf:type  owl:DatatypeProperty ;
        rdfs:label    "inbound topic"@en ;
        rdfs:domain   ids:Endpoint ;
        rdfs:range    xsd:string ;
        rdfs:comment  "Relative path used for inbound communication via this endpoint, i.e., input messages and faults only."@en .

ids:outboundPath  rdf:type  owl:DatatypeProperty ;
        rdfs:label    "outbound topic"@en ;
        rdfs:domain   ids:Endpoint ;
        rdfs:range    xsd:string ;
        rdfs:comment  "Relative path used for outbound communication via this endpoint, i.e., output messages and faults only."@en .

ids:apiSpecifiation  rdf:type  owl:ObjectProperty ;
        rdfs:label    "follows API specification" ;
        rdfs:comment  "Declares which endpoint specification is supported by this IDS endpoint." ;
        rdfs:domain   ids:Endpoint ;
        rdfs:range    ids:IdsProtocolSpecification .

ids:appEndpointType  rdf:type  owl:ObjectProperty ;
        rdfs:domain   ids:AppEndpoint ;
        rdfs:range    ids:AppEndpointType ;
        rdfs:label    "App endpoint type"@en ;
        rdfs:comment  "Type of an app endpoint. Data apps have different endpoint types, e.g., for input, output or health status."@en .

ids:appEndpointPort  rdf:type  owl:DatatypeProperty ;
        rdfs:domain   ids:AppEndpoint ;
        rdfs:range    xsd:integer ;
        rdfs:label    "app endpoint port"@en ;
        rdfs:comment  "Port used to access the endpoint."@en .

ids:appEndpointMediaType
        rdf:type      owl:ObjectProperty ;
        rdfs:domain   ids:AppEndpoint ;
        rdfs:range    dct:MediaType ;
        rdfs:label    "app endpoint media type"@en ;
        rdfs:comment  "Mediatype, such as IANA types, of the data an endpoint expects or returns ."@en .

ids:genericEndpointAuthentication
        rdf:type      owl:ObjectProperty ;
        rdfs:domain   ids:GenericEndpoint ;
        rdfs:range    ids:BasicAuthentication ;
        rdfs:label    "generic endpoint authentication"@en ;
        rdfs:comment  "Authentication credentials for generic endpoints. "@en .

ids:genericEndpointConfiguration
        rdf:type      owl:DatatypeProperty ;
        rdfs:domain   ids:GenericEndpoint ;
        rdfs:range    xsd:string ;
        rdfs:label    "generic endpoint configuration"@en ;
        rdfs:comment  "Endpoint-specific configuration details (e.g., contents of a config file) used for the endpoint."@en .

ids:appEndpointProtocol
        rdf:type      owl:DatatypeProperty ;
        rdfs:domain   ids:AppEndpoint ;
        rdfs:range    xsd:string ;
        rdfs:label    "app endpoint protocol"@en ;
        rdfs:comment  "Protocol used to communicate with the app endpoint."@en .
@prefix owl:   <http://www.w3.org/2002/07/owl#> .
@prefix rdf:   <http://www.w3.org/1999/02/22-rdf-syntax-ns#> .
@prefix rdfs:  <http://www.w3.org/2000/01/rdf-schema#> .
@prefix xsd:   <http://www.w3.org/2001/XMLSchema#> .
@prefix foaf:  <http://xmlns.com/foaf/0.1/> .
@prefix dct:   <http://purl.org/dc/terms/> .
@prefix ids:   <https://w3id.org/idsa/core/> .

ids:Message  rdf:type  owl:Class ;
        rdfs:label    "Message"@en ;
        rdfs:comment  "Metadata describing payload exchanged by interacting Connectors."@en .

ids:modelVersion  rdf:type  owl:DatatypeProperty ;
        rdfs:label    "model version"@en ;
        rdfs:domain   ids:Message ;
        rdfs:range    xsd:string ;
        rdfs:comment  "Version of the Information Model against which the Message should be interpreted."@en .

ids:correlationMessage
        rdf:type      owl:ObjectProperty ;
        rdfs:label    "consumer connector"@en ;
        rdfs:domain   ids:Message ;
        rdfs:range    ids:Message ;
        rdfs:comment  "Correlated message, e.g., a response to a previous request."@en .

ids:issuerConnector  rdf:type  owl:DatatypeProperty ;
        rdfs:label    "issuer connector"@en ;
        rdfs:domain   ids:Message ;
        rdfs:range    ids:Connector ;
        rdfs:comment  "The Connector which is the origin of the message."@en .

ids:recipientConnector
        rdf:type      owl:ObjectProperty ;
        rdfs:label    "recipient connector"@en ;
        rdfs:domain   ids:Message ;
        rdfs:range    ids:Connector ;
        rdfs:comment  "The Connector which is the recipient of the message."@en .

ids:senderAgent  rdf:type  owl:DatatypeProperty ;
        rdfs:label    "sender agent"@en ;
        rdfs:domain   ids:Message ;
        rdfs:range    foaf:Agent ;
        rdfs:comment  "The Agent which initiated the Message."@en .

ids:recipientAgent  rdf:type  owl:DatatypeProperty ;
        rdfs:label    "recipient agent"@en ;
        rdfs:domain   ids:Message ;
        rdfs:range    foaf:Agent ;
        rdfs:comment  "The Agent for which the Mesaage is intended."@en .

ids:securityToken  rdf:type  owl:ObjectProperty ;
        rdfs:label    "Security token"@en ;
        rdfs:domain   ids:Message ;
        rdfs:range    ids:DynamicAttributeToken ;
        rdfs:comment  "A token representing a claim that the message sender supports a certain security profile."@en .

ids:authorizationToken
        rdf:type      owl:ObjectProperty ;
        rdfs:label    "Authorization token"@en ;
        rdfs:domain   ids:Message ;
        rdfs:range    ids:Token ;
        rdfs:comment  "An authorization token like JSON Web Token."@en .

ids:transferContract  rdf:type  owl:ObjectProperty ;
        rdfs:label    "transferContract"@en ;
        rdfs:domain   ids:Message ;
        rdfs:range    ids:Contract ;
        rdfs:comment  "The contract which is (or will be) the legal basis of the data transfer."@en .

ids:contentVersion  rdf:type  owl:DatatypeProperty ;
        rdfs:label    "contentVersion"@en ;
        rdfs:domain   ids:Message ;
        rdfs:range    xsd:string ;
        rdfs:comment  "Version of the content in the payload. Use digits and semantic versioning pattern like MAJOR.MINOR.PATCH."@en .
@prefix owl:   <http://www.w3.org/2002/07/owl#> .
@prefix rdfs:  <http://www.w3.org/2000/01/rdf-schema#> .
@prefix dct:   <http://purl.org/dc/terms/> .
@prefix xsd:   <http://www.w3.org/2001/XMLSchema#> .
@prefix ids:   <https://w3id.org/idsa/core/> .

ids:Proxy  rdf:type   owl:Class ;
        rdfs:label    "Proxy"@en ;
        rdfs:comment  "Holds Proxy information."@en ;
        rdfs:seeAlso  <https://tools.ietf.org/html/rfc2068> .

ids:proxyURI  rdf:type  owl:DatatypeProperty ;
        rdfs:domain   ids:Proxy ;
        rdfs:range    xsd:anyURI ;
        rdfs:seeAlso  <https://www.gnu.org/software/emacs/manual/html_node/url/Proxies.html> ;
        rdfs:label    "proxy URI"@en ;
        rdfs:comment  "URI of the proxy server."@en .

ids:noProxy  rdf:type  owl:DatatypeProperty ;
        rdfs:domain   ids:Proxy ;
        rdfs:range    xsd:anyURI ;
        rdfs:seeAlso  <https://www.gnu.org/software/emacs/manual/html_node/url/Proxies.html> ;
        rdfs:label    "no proxy"@en ;
        rdfs:comment  "URLs that should be excluded from proxying.GNU emcs documentation contains a good explanation for the usage of noProxy."@en .

ids:proxyAuthentication
        rdf:type      owl:DatatypeProperty ;
        rdfs:domain   ids:Proxy ;
        rdfs:range    ids:BasicAuthentication ;
        rdfs:label    "proxy Authentication"@en ;
        rdfs:comment  "authentication information for the proxy"@en .
@prefix owl:   <http://www.w3.org/2002/07/owl#> .
@prefix rdfs:  <http://www.w3.org/2000/01/rdf-schema#> .
@prefix dct:   <http://purl.org/dc/terms/> .
@prefix xsd:   <http://www.w3.org/2001/XMLSchema#> .
@prefix odrl:  <http://www.w3.org/ns/odrl/2/> .
@prefix ids:   <https://w3id.org/idsa/core/> .

ids:actionRefinement  rdf:type  owl:ObjectProperty ;
        rdfs:label    "action refinement"@en ;
        rdfs:domain   odrl:Action ;
        rdfs:range    odrl:Constraint ;
        rdfs:comment  "Constraint that refines an Action."@en .

ids:pxpEndpoint  rdf:type  owl:ObjectProperty ;
        rdfs:label    "has PXP endpoint"@en ;
        rdfs:domain   odrl:Action ;
        rdfs:range    ids:PXP ;
        rdfs:comment  "The reference to the PXP which operates a specific action, URI or reference to an associated PXP interface."@en .
@prefix owl:   <http://www.w3.org/2002/07/owl#> .
@prefix rdfs:  <http://www.w3.org/2000/01/rdf-schema#> .
@prefix dct:   <http://purl.org/dc/terms/> .
@prefix xsd:   <http://www.w3.org/2001/XMLSchema#> .
@prefix odrl:  <http://www.w3.org/ns/odrl/2/> .
@prefix ids:   <https://w3id.org/idsa/core/> .

ids:BinaryOperator  rdfs:subClassOf  odrl:Operator ;
        rdf:type         owl:Class ;
        rdfs:label       "BinaryOperator"@en ;
        rdfs:comment     "The class of binary operators."@en .
@prefix owl:   <http://www.w3.org/2002/07/owl#> .
@prefix rdfs:  <http://www.w3.org/2000/01/rdf-schema#> .
@prefix dct:   <http://purl.org/dc/terms/> .
@prefix xsd:   <http://www.w3.org/2001/XMLSchema#> .
@prefix odrl:  <http://www.w3.org/ns/odrl/2/> .
@prefix rdf:   <http://www.w3.org/1999/02/22-rdf-syntax-ns#> .
@prefix ids:   <https://w3id.org/idsa/core/> .

ids:pipEndpoint  rdf:type  owl:ObjectProperty ;
        rdfs:label    "has PIP endpoint"@en ;
        rdfs:domain   odrl:Constraint ;
        rdfs:range    ids:PIP ;
        rdfs:comment  "The reference to the endpoint which provides the current state of the feature of interest (as referrenced by the leftOperand) can be retrieved."@en .
@prefix owl:   <http://www.w3.org/2002/07/owl#> .
@prefix dct:   <http://purl.org/dc/terms/> .
@prefix rdfs:  <http://www.w3.org/2000/01/rdf-schema#> .
@prefix odrl:  <http://www.w3.org/ns/odrl/2/> .
@prefix xsd:   <http://www.w3.org/2001/XMLSchema#> .
@prefix ids:   <https://w3id.org/idsa/core/> .

ids:Contract  rdf:type   owl:Class ;
        rdfs:subClassOf  odrl:Policy ;
        rdfs:label       "Contract"@en ;
        rdfs:comment     "Abstract set of rules governing the usage of a Resource."@en .

ids:ContractAgreement
        rdf:type          owl:Class ;
        rdfs:subClassOf   ids:Contract ;
        rdfs:subClassOf   odrl:Agreement ;
        rdfs:label        "Contract agreement"@en ;
        rdfs:comment      "Contract governing the actual usage of a Resource that has been agreed by all parties."@en ;
        owl:disjointWith  ids:ContractRequest ;
        owl:disjointWith  ids:ContractOffer .

ids:ContractRequest  rdf:type  owl:Class ;
        rdfs:subClassOf   ids:Contract ;
        rdfs:subClassOf   odrl:Request ;
        rdfs:label        "Contract request"@en ;
        rdfs:comment      "Contract issued by the Data Consumer requesting the usage of a Resource at particular conditions."@en ;
        owl:disjointWith  ids:ContractAgreement ;
        owl:disjointWith  ids:ContractOffer .

ids:ContractOffer  rdf:type  owl:Class ;
        rdfs:subClassOf   ids:Contract ;
        rdfs:subClassOf   odrl:Offer ;
        rdfs:label        "Contract offer"@en ;
        rdfs:comment      "Contract issued by the Data Provider offering the usage of a Resource at particular conditions."@en ;
        owl:disjointWith  ids:ContractAgreement ;
        owl:disjointWith  ids:ContractRequest .

ids:contractStart  rdf:type  owl:DatatypeProperty ;
        rdfs:domain   ids:Contract ;
        rdfs:range    xsd:dateTimeStamp ;
        rdfs:label    "Contract start"@en ;
        rdfs:comment  "Absolute datetime the Contract is requested, offered or expected to start, depending on the type of Contract."@en .

ids:contractEnd  rdf:type  owl:DatatypeProperty ;
        rdfs:domain   ids:Contract ;
        rdfs:range    xsd:dateTimeStamp ;
        rdfs:label    "Contract end"@en ;
        rdfs:comment  "Absolute datetime the Contract is requested, offered or expected to end. If omitted, the contract has to be explicitly terminated by any of the parties."@en .

ids:contractDate  rdf:type  owl:DatatypeProperty ;
        rdfs:domain   ids:Contract ;
        rdfs:range    xsd:dateTimeStamp ;
        rdfs:label    "Contract date"@en ;
        rdfs:comment  "Absolute datetime of signing the Contract."@en .

ids:provider  rdf:type  owl:ObjectProperty ;
        rdfs:domain   ids:Contract ;
        rdfs:range    ids:Participant ;
        rdfs:label    "Provider"@en ;
        rdfs:comment  "Provider of a Resource or Service that is the subject matter of the contract. This party may differ from the Assigner specified by the Contract rules."@en .

ids:consumer  rdf:type  owl:ObjectProperty ;
        rdfs:domain   ids:Contract ;
        rdfs:range    ids:Participant ;
        rdfs:label    "Consumer"@en ;
        rdfs:comment  "Consumer of a Resource or Service that is the subject matter of the Contract. This party may differ from the Assignee specified by the Contract rules."@en .

ids:contractDocument  rdf:type  owl:ObjectProperty ;
        rdfs:domain   ids:Contract ;
        rdfs:range    ids:TextResource ;
        rdfs:label    "Contract document"@en ;
        rdfs:comment  "Equivalent human-readable encoding of this machine-interpretable Contract."@en .

ids:contractAnnex  rdf:type  owl:ObjectProperty ;
        rdfs:domain   ids:Contract ;
        rdfs:range    ids:Resource ;
        rdfs:label    "Annex to contract"@en ;
        rdfs:comment  "Any type of resource related to the Contract."@en .
@prefix owl:   <http://www.w3.org/2002/07/owl#> .
@prefix rdfs:  <http://www.w3.org/2000/01/rdf-schema#> .
@prefix dct:   <http://purl.org/dc/terms/> .
@prefix xsd:   <http://www.w3.org/2001/XMLSchema#> .
@prefix odrl:  <http://www.w3.org/ns/odrl/2/> .
@prefix ids:   <https://w3id.org/idsa/core/> .
@prefix skos:  <http://www.w3.org/2004/02/skos/core#> .

ids:broader  rdf:type  owl:ObjectProperty ;
        skos:broader  odrl:includedIn ;
        rdfs:seeAlso  skos:broader ;
        rdfs:label    "broader LeftOperand"@en ;
        rdfs:domain   odrl:LeftOperand ;
        rdfs:range    odrl:LeftOperand ;
        rdfs:comment  "This LeftOperand is transitively included in the object LeftOperand."@en .
@prefix owl:   <http://www.w3.org/2002/07/owl#> .
@prefix rdfs:  <http://www.w3.org/2000/01/rdf-schema#> .
@prefix dct:   <http://purl.org/dc/terms/> .
@prefix xsd:   <http://www.w3.org/2001/XMLSchema#> .
@prefix odrl:  <http://www.w3.org/ns/odrl/2/> .
@prefix rdf:   <http://www.w3.org/1999/02/22-rdf-syntax-ns#> .
@prefix ids:   <https://w3id.org/idsa/core/> .

ids:target  rdf:type  owl:ObjectProperty ;
        rdfs:domain   odrl:Rule ;
        rdfs:range    odrl:Asset ;
        rdfs:label    "target"@en ;
        rdfs:comment  "The subject of the policy statement (odrl:Rule)."@en .

ids:preDuty  rdfs:subPropertyOf  odrl:duty ;
        rdf:type            owl:ObjectProperty ;
        rdfs:label          "pre-duty"@en ;
        rdfs:domain         odrl:Permission ;
        rdfs:range          odrl:Duty ;
        rdfs:comment        "A Duty imposed by the Rule, which must be executed before the Rule."@en .

ids:postDuty  rdfs:subPropertyOf  odrl:duty ;
        rdf:type            owl:ObjectProperty ;
        rdfs:label          "post-duty"@en ;
        rdfs:domain         odrl:Permission ;
        rdfs:range          odrl:Duty ;
        rdfs:comment        "A Duty imposed by the Rule, which must be executed after the Rule."@en .
@prefix owl:   <http://www.w3.org/2002/07/owl#> .
@prefix rdfs:  <http://www.w3.org/2000/01/rdf-schema#> .
@prefix ids:   <https://w3id.org/idsa/core/> .
@prefix xsd:   <http://www.w3.org/2001/XMLSchema#> .

ids:UsageControlComponent
        rdf:type      owl:Class ;
        rdfs:label    "Usage Control Component"@en ;
        rdfs:comment  "Defined usage control component (i.e. PIP, PXP, etc.) in the IDS."@en .

ids:PXP  rdf:type        owl:Class ;
        rdfs:subClassOf  ids:UsageControlComponent ;
        rdfs:label       "policy execution point"@en ;
        rdfs:comment     "The reference to the PXP that operates a specific action, URI or reference to an associated PXP interface."@en .

ids:PIP  rdf:type        owl:Class ;
        rdfs:subClassOf  ids:UsageControlComponent ;
        rdfs:label       "policy information point"@en ;
        rdfs:comment     "Refers to the PIP that provides a specific piece of information (URI/reference to an associated PIP interface). "@en .

ids:interfaceDescription
        rdf:type      owl:ObjectProperty ;
        rdfs:label    "interface description"@en ;
        rdfs:domain   ids:UsageControlComponent ;
        rdfs:range    xsd:anyURI ;
        rdfs:comment  "The reference to a URI that provides the interface description of a usage control endpoint."@en .

ids:endpointURI  rdf:type  owl:ObjectProperty ;
        rdfs:label    "endpoint URI"@en ;
        rdfs:domain   ids:UsageControlComponent ;
        rdfs:range    xsd:anyURI ;
        rdfs:comment  "The reference to a URI that expresses an exact endpoint of that usage control endpoint."@en .
@prefix owl:   <http://www.w3.org/2002/07/owl#> .
@prefix rdfs:  <http://www.w3.org/2000/01/rdf-schema#> .
@prefix ids:   <https://w3id.org/idsa/core/> .

ids:UsagePolicyClass  rdf:type  owl:Class ;
        rdfs:label    "Usage policy class"@en ;
        rdfs:comment  "Defined usage policy classes in the IDS."@en .
@prefix dct:   <http://purl.org/dc/terms/> .
@prefix dcat:  <http://www.w3.org/ns/dcat#> .
@prefix owl:   <http://www.w3.org/2002/07/owl#> .
@prefix rdf:   <http://www.w3.org/1999/02/22-rdf-syntax-ns#> .
@prefix rdfs:  <http://www.w3.org/2000/01/rdf-schema#> .
@prefix odrl:  <http://www.w3.org/ns/odrl/2/> .
@prefix xsd:   <http://www.w3.org/2001/XMLSchema#> .
@prefix ids:   <https://w3id.org/idsa/core/> .

ids:Artifact  rdf:type    owl:Class ;
        rdfs:subClassOf   odrl:Asset ;
        rdfs:subClassOf   ids:RepresentationInstance ;
        rdfs:label        "Artifact"@en ;
        rdfs:comment      "Instance of a Representation materialized at a partiuclar version and point in time. Possesses characteristics like file name, size, creation date etc."@en ;
        owl:disjointWith  ids:Value .

ids:byteSize  rdf:type      owl:DatatypeProperty ;
        rdfs:subPropertyOf  dcat:byteSize ;
        rdfs:label          "byte size"@en ;
        rdfs:comment        "Size of the Artifact in bytes."@en ;
        rdfs:domain         ids:Artifact ;
        rdfs:range          xsd:integer .

ids:fileName  rdf:type  owl:DatatypeProperty ;
        rdfs:label    "file name"@en ;
        rdfs:comment  "Name of the Artifcat file."@en ;
        rdfs:domain   ids:Artifact ;
        rdfs:range    xsd:string .

ids:checkSum  rdf:type  owl:DatatypeProperty ;
        rdfs:domain   ids:Artifact ;
        rdfs:range    xsd:string ;
        rdfs:label    "checksum"@en ;
        rdfs:comment  "Checksum of the artifact"@en .

ids:duration  rdf:type  owl:DatatypeProperty ;
        rdfs:domain   ids:Artifact ;
        rdfs:range    xsd:decimal ;
        rdfs:label    "duration"@en ;
        rdfs:comment  "Duration of the media resource in seconds."@en .
@prefix owl:   <http://www.w3.org/2002/07/owl#> .
@prefix rdfs:  <http://www.w3.org/2000/01/rdf-schema#> .
@prefix skos:  <http://www.w3.org/2004/02/skos/core#> .
@prefix dct:   <http://purl.org/dc/terms/> .
@prefix xsd:   <http://www.w3.org/2001/XMLSchema#> .
@prefix geo:   <http://www.opengis.net/ont/geosparql#> .
@prefix wgs84: <https://www.w3.org/2003/01/geo/wgs84_pos#> .
@prefix odrl:  <http://www.w3.org/ns/odrl/2/> .
@prefix time:  <http://www.w3.org/2006/time#> .
@prefix org:   <http://www.w3.org/ns/org#> .
@prefix ids:   <https://w3id.org/idsa/core/> .
@prefix idsc:  <https://w3id.org/idsa/code/> .

ids:ArtifactState  rdf:type  owl:Class ;
        rdfs:label    "Artifact State"@en ;
        rdfs:comment  "The state which an ids:Artifact may have or not."@en .
@prefix dct:   <http://purl.org/dc/terms/> .
@prefix dcat:  <http://www.w3.org/ns/dcat#> .
@prefix ids:   <https://w3id.org/idsa/core/> .
@prefix owl:   <http://www.w3.org/2002/07/owl#> .
@prefix rdf:   <http://www.w3.org/1999/02/22-rdf-syntax-ns#> .
@prefix rdfs:  <http://www.w3.org/2000/01/rdf-schema#> .
@prefix xsd:   <http://www.w3.org/2001/XMLSchema#> .
@prefix odrl:  <http://www.w3.org/ns/odrl/2/> .

ids:assetSource  rdf:type   owl:ObjectProperty ;
        rdfs:subPropertyOf  odrl:source ;
        rdfs:label          "asset source"@en ;
        rdfs:domain         odrl:AssetCollection ;
        rdfs:range          xsd:anyURI ;
        rdfs:comment        "A remote link to the location (PIP) where this AssetCollection and its members are maintained."@en .
@prefix owl:   <http://www.w3.org/2002/07/owl#> .
@prefix rdfs:  <http://www.w3.org/2000/01/rdf-schema#> .
@prefix xsd:   <http://www.w3.org/2001/XMLSchema#> .
@prefix ids:   <https://w3id.org/idsa/core/> .

ids:DataApp  rdf:type  owl:Class ;
        rdfs:label    "DataApp"@en ;
        rdfs:comment  "Self-contained, self-descriptive software package that is distributed via the App Store and deployed inside a Connector; provides access to data and data processing capa­bilities; the interface of a Data App is semantically described by the IDS Information Model."@en .

ids:appDocumentation  rdf:type  owl:DatatypeProperty ;
        rdfs:domain   ids:DataApp ;
        rdfs:range    xsd:string ;
        rdfs:label    "app documentation"@en ;
        rdfs:comment  "text documentation of the data app"@en .

ids:appEndpoint  rdf:type  owl:ObjectProperty ;
        rdfs:label    "app endpoint"@en ;
        rdfs:domain   ids:DataApp ;
        rdfs:range    ids:AppEndpoint ;
        rdfs:comment  "Endpoints of a data app"@en .

ids:appEnvironmentVariables
        rdf:type      owl:DatatypeProperty ;
        rdfs:label    "app environment variables"@en ;
        rdfs:comment  "Necessary or optional environment variables of a data app."@en ;
        rdfs:domain   ids:DataApp ;
        rdfs:range    xsd:string .

ids:appStorageConfiguration
        rdf:type      owl:DatatypeProperty ;
        rdfs:label    "app storage configuration"@en ;
        rdfs:comment  "Storage configuration of a data app. Value may differ based on the app ecosystem, e.g., a writeable path in the file system or a volume name (e.g., for containerized apps)"@en ;
        rdfs:domain   ids:DataApp ;
        rdfs:range    xsd:string .

ids:supportedUsagePolicies
        rdf:type      owl:ObjectProperty ;
        rdfs:domain   ids:DataApp ;
        rdfs:range    ids:UsagePolicyClass ;
        rdfs:label    "supported usage policies"@en ;
        rdfs:comment  "IDS Usage Policies a DataApp supports"@en .

ids:SystemAdapter  rdf:type  owl:Class ;
        rdfs:subClassOf  ids:DataApp ;
        rdfs:label       "System Adapter"@en ;
        rdfs:comment     "Data Apps that integrate sources and sinks of digital content maintained internally on Participant's premises with a Connector."@en .

ids:OrchestrationApp  rdf:type  owl:Class ;
        rdfs:subClassOf  ids:DataApp ;
        rdfs:label       "Orchestration App"@en ;
        rdfs:comment     "Apps for orchestrating System Adapter Apps or Smart Data Apps, inside a Connector."@en .

ids:SmartDataApp  rdf:type  owl:Class ;
        rdfs:subClassOf  ids:DataApp ;
        rdfs:label       "Smart DataApp"@en ;
        rdfs:comment     "Smart DataApps are executing any kind of necessary data processing or transformation."@en .
@prefix rdf:   <http://www.w3.org/1999/02/22-rdf-syntax-ns#> .
@prefix owl:   <http://www.w3.org/2002/07/owl#> .
@prefix rdfs:  <http://www.w3.org/2000/01/rdf-schema#> .
@prefix dct:   <http://purl.org/dc/terms/> .
@prefix dcat:  <http://www.w3.org/ns/dcat#> .
@prefix skos:  <http://www.w3.org/2004/02/skos/core#> .
@prefix ids:   <https://w3id.org/idsa/core/> .
@prefix xsd:   <http://www.w3.org/2001/XMLSchema#> .

ids:DigitalContent  rdf:type  owl:Class ;
        rdfs:subClassOf  ids:Described ;
        rdfs:subClassOf  dcat:Dataset ;
        rdfs:label       "Digital content"@en ;
        rdfs:comment     "Digital content of a particular type providing hints on its usage, e.g., listening to an Audio, navigating a Structure or accessing a List by an index."@en ;
        rdfs:seeAlso     <https://en.wikipedia.org/wiki/Digital_content> ;
        rdfs:seeAlso     <http://www.ontodm.com/doku.php?id=ontodt> ;
        rdfs:seeAlso     <http://schema.org/DataType> ;
        rdfs:seeAlso     <http://schema.org/additionalType> ;
        rdfs:seeAlso     <https://github.com/twosixlabs/icas-ontology/blob/master/ontology/mime.ttl> ;
        rdfs:seeAlso     <http://www.ddialliance.org/Specification/DDI-CV/GeneralDataFormat_2.0.html> .

ids:contentType  rdf:type   owl:ObjectProperty ;
        rdfs:subPropertyOf  dct:type ;
        rdfs:domain         ids:DigitalContent ;
        rdfs:range          dct:DCMIType ;
        rdfs:label          "content type"@en ;
        rdfs:comment        "Detailed type, genre or interpretation of the Digital Content."@en .

ids:contentPart  rdf:type  owl:ObjectProperty ;
        rdfs:label    "content part"@en ;
        rdfs:domain   ids:DigitalContent ;
        rdfs:range    ids:DigitalContent ;
        rdfs:comment  "Reference to a Digital Content (physically or logically) included, definition of part-whole hierarchies."@en .

ids:representation  rdf:type  owl:ObjectProperty ;
        rdfs:label    "representation"@en ;
        rdfs:domain   ids:DigitalContent ;
        rdfs:range    dcat:Distribution ;
        rdfs:comment  "Representation of the content."@en .

ids:defaultRepresentation
        rdf:type            owl:ObjectProperty ;
        rdfs:subPropertyOf  ids:representation ;
        rdfs:label          "Default representation"@en ;
        rdfs:domain         ids:DigitalContent ;
        rdfs:range          dcat:Distribution ;
        rdfs:comment        "Default representation of the content."@en .

ids:contentStandard  rdf:type  owl:DatatypeProperty ;
        rdfs:subPropertyOf  dct:conformsTo ;
        rdfs:domain         ids:DigitalContent ;
        rdfs:range          xsd:anyURI ;
        rdfs:label          "content standard"@en ;
        rdfs:comment        "IRI containing document, which defines the standard for the given Digital Content. The content is assumed to conform to that Standard."@en .
@prefix owl:   <http://www.w3.org/2002/07/owl#> .
@prefix rdfs:  <http://www.w3.org/2000/01/rdf-schema#> .
@prefix dct:   <http://purl.org/dc/terms/> .
@prefix ids:   <https://w3id.org/idsa/core/> .

ids:Language  rdf:type  owl:Class ;
        rdfs:label    "Language"@en ;
        rdfs:comment  "The class of languages potentially being used by textual Data Assets."@en .
@prefix owl:   <http://www.w3.org/2002/07/owl#> .
@prefix rdfs:  <http://www.w3.org/2000/01/rdf-schema#> .
@prefix dct:   <http://purl.org/dc/terms/> .
@prefix ids:   <https://w3id.org/idsa/core/> .
@prefix xsd:   <http://www.w3.org/2001/XMLSchema#> .
@prefix idsc:  <https://w3id.org/idsa/code/> .

ids:CustomMediaType  rdf:type  owl:Class ;
        rdfs:subClassOf  dct:MediaType ;
        rdfs:label       "Custom Media Type"@en ;
        rdfs:comment     "A selection of custom media types to be used for data published on the IDS when no IANA type is available."@en .

ids:IANAMediaType  rdf:type  owl:Class ;
        rdfs:subClassOf  dct:MediaType ;
        rdfs:label       "IANA Media Type"@en ;
        rdfs:comment     "The class of media types registered with IANA."@en ;
        rdfs:seeAlso     <https://www.iana.org/assignments/media-types/> ;
        rdfs:seeAlso     <http://www.sparontologies.net/mediatype/> ;
        rdfs:seeAlso     <http://dx.doi.org/10.6084/m9.figshare.1608294> .

ids:filenameExtension
        rdf:type      owl:DatatypeProperty ;
        rdfs:label    "filename extension"@en ;
        rdfs:domain   dct:MediaType ;
        rdfs:range    xsd:string ;
        rdfs:comment  "Suffix of a file name, typically separated by a period, indicating the nature and intended processing of the file."@en ;
        rdfs:seeAlso  <https://en.wikipedia.org/wiki/Filename_extension> .
@prefix dct:   <http://purl.org/dc/terms/> .
@prefix ids:   <https://w3id.org/idsa/core/> .
@prefix owl:   <http://www.w3.org/2002/07/owl#> .
@prefix rdf:   <http://www.w3.org/1999/02/22-rdf-syntax-ns#> .
@prefix rdfs:  <http://www.w3.org/2000/01/rdf-schema#> .
@prefix xsd:   <http://www.w3.org/2001/XMLSchema#> .

ids:PaymentModality  rdf:type  owl:Class ;
        rdfs:label    "Payment Modality"@en ;
        rdfs:comment  "Various pricing modalities such as idsc:FREE, idsc:FIXED_PRICE and idsc:NEGOTIATION_BASIS can be used as a pre-selection to annotate the terms of the contract. Depending on the requirements, additional free text information can be attached."@en .
@prefix owl:   <http://www.w3.org/2002/07/owl#> .
@prefix rdfs:  <http://www.w3.org/2000/01/rdf-schema#> .
@prefix dct:   <http://purl.org/dc/terms/> .
@prefix dcat:  <http://www.w3.org/ns/dcat#> .
@prefix rdf:   <http://www.w3.org/1999/02/22-rdf-syntax-ns#> .
@prefix xsd:   <http://www.w3.org/2001/XMLSchema#> .
@prefix ids:   <https://w3id.org/idsa/core/> .

ids:RepresentationInstance
        rdf:type      owl:Class ;
        rdfs:label    "Representation instance"@en ;
        rdfs:comment  "A particular instance of given representation."@en .

ids:Value  rdf:type       owl:Class ;
        rdfs:subClassOf   ids:RepresentationInstance ;
        rdfs:label        "Value"@en ;
        rdfs:comment      "Literal, inline value instantiation of a representation."@en ;
        owl:disjointWith  ids:Artifact .

ids:instance  rdf:type  owl:ObjectProperty ;
        rdfs:domain   dcat:Distribution ;
        rdfs:range    ids:RepresentationInstance ;
        rdfs:label    "instance"@en ;
        rdfs:comment  "Reference to an instance of given representation, i.e. inline value or file placeholder."@en .

ids:representationStandard
        rdf:type            owl:DatatypeProperty ;
        rdfs:subPropertyOf  dct:conformsTo ;
        rdfs:domain         dcat:Distribution ;
        rdfs:range          xsd:anyURI ;
        rdfs:label          "representation standard"@en ;
        rdfs:comment        "Standards document defining the given Representation (in contrast to general Resource content). The Representation is assumed to conform to that Standard."@en .
@prefix dct:   <http://purl.org/dc/terms/> .
@prefix ids:   <https://w3id.org/idsa/core/> .
@prefix foaf:  <http://xmlns.com/foaf/0.1/> .
@prefix owl:   <http://www.w3.org/2002/07/owl#> .
@prefix rdf:   <http://www.w3.org/1999/02/22-rdf-syntax-ns#> .
@prefix rdfs:  <http://www.w3.org/2000/01/rdf-schema#> .
@prefix xsd:   <http://www.w3.org/2001/XMLSchema#> .
@prefix odrl:  <http://www.w3.org/ns/odrl/2/> .

ids:Resource  rdf:type   owl:Class ;
        rdfs:subClassOf  ids:DescribedSemantically ;
        rdfs:subClassOf  ids:DigitalContent ;
        rdfs:subClassOf  ids:ManagedEntity ;
        rdfs:subClassOf  odrl:Asset ;
        rdfs:label       "Resource"@en ;
        rdfs:comment     "Resource is a single digital content or a coherent set of digital contents. Resource content is formalized in Representations and optionally materialized as Artifacts. The Resource's content is exposed via defined Interfaces at various protocol Endpoints."@en ;
        rdfs:seeAlso     <https://www.w3.org/TR/vocab-dcat/#class-dataset> .

ids:resourcePart  rdf:type  owl:ObjectProperty ;
        rdfs:subPropertyOf  ids:contentPart ;
        rdfs:label          "resource part"@en ;
        rdfs:domain         ids:Resource ;
        rdfs:range          ids:Resource ;
        rdfs:comment        "Reference to a Resource (physically or logically) included, definition of part-whole hierarchies."@en .

ids:resourceEndpoint  rdf:type  owl:ObjectProperty ;
        rdfs:label    "resource endpoint"@en ;
        rdfs:domain   ids:Resource ;
        rdfs:range    ids:ConnectorEndpoint ;
        rdfs:comment  "Reference to the Endpoints that serve the resource's content or let you exchange messages with an IDS Connector."@en .

ids:contractOffer  rdf:type  owl:ObjectProperty ;
        rdfs:domain   ids:Resource ;
        rdfs:range    ids:ContractOffer ;
        rdfs:label    "contract offer"@en ;
        rdfs:comment  "Reference to a Contract Offer defining the authorized use of the Resource."@en .

ids:paymentModality  rdf:type  owl:ObjectProperty ;
        rdfs:domain   ids:Resource ;
        rdfs:range    ids:PaymentModality ;
        rdfs:label    "payment modality"@en ;
        rdfs:comment  "Various pricing modalities such as idsc:FREE, idsc:FIXED_PRICE and idsc:NEGOTIATION_BASIS can be used as a pre-selection to annotate the terms of the contract. Depending on the requirements, additional free text information can be attached."@en .

ids:sovereign  rdf:type  owl:ObjectProperty ;
        rdfs:domain   ids:Resource ;
        rdfs:range    foaf:Agent ;
        rdfs:label    "sovereign"@en ;
        rdfs:comment  "The 'owner', i.e. sovereign of the data."@en .

ids:sample  rdf:type  owl:ObjectProperty ;
        rdfs:label    "sample"@en ;
        rdfs:domain   ids:Resource ;
        rdfs:range    ids:Resource ;
        rdfs:comment  "Sample Resource instance."@en .

ids:variant  rdf:type  owl:ObjectProperty ;
        rdfs:label    "variant"@en ;
        rdfs:domain   ids:Resource ;
        rdfs:range    ids:Resource ;
        rdfs:comment  "(Equivalent) variant of given Resource, e.g., a translation."@en .
@prefix owl:   <http://www.w3.org/2002/07/owl#> .
@prefix rdfs:  <http://www.w3.org/2000/01/rdf-schema#> .
@prefix dct:   <http://purl.org/dc/terms/> .
@prefix xsd:   <http://www.w3.org/2001/XMLSchema#> .
@prefix odrl:  <http://www.w3.org/ns/odrl/2/> .
@prefix ids:   <https://w3id.org/idsa/core/> .

ids:UsageControlObject
        rdf:type      owl:Class ;
        rdfs:label    "Usage Control Object"@en ;
        rdfs:comment  "A data element containing all relevant information for usage control engines."@en .

ids:data  rdf:type    owl:ObjectProperty ;
        rdfs:label    "has data"@en ;
        rdfs:domain   ids:UsageControlObject ;
        rdfs:range    xsd:anyURI ;
        rdfs:comment  "The related data or a pointer/reference to it."@en .

ids:user  rdf:type    owl:ObjectProperty ;
        rdfs:label    "has user"@en ;
        rdfs:domain   ids:UsageControlObject ;
        rdfs:range    ids:Participant ;
        rdfs:comment  "The participant intending to use the data."@en .

ids:source  rdf:type  owl:ObjectProperty ;
        rdfs:label    "source"@en ;
        rdfs:domain   ids:UsageControlObject ;
        rdfs:range    xsd:anyURI ;
        rdfs:comment  "The application which provided the data object. Should be a valid URI. Must be unique in the regarded environment."@en .

ids:contract  rdf:type  owl:ObjectProperty ;
        rdfs:label    "has contract"@en ;
        rdfs:domain   ids:UsageControlObject ;
        rdfs:range    ids:ContractAgreement ;
        rdfs:comment  "The target contract defining the usage of the data object."@en .

ids:usageDuration  rdf:type  owl:ObjectProperty ;
        rdfs:label    "usage duration"@en ;
        rdfs:domain   ids:UsageControlObject ;
        rdfs:range    xsd:duration ;
        rdfs:comment  "Duration, which this asset is in use by now. Might be calculated on the fly when requested by a Usage Control Engine."@en .

ids:accessed  rdf:type  owl:ObjectProperty ;
        rdfs:label    "last accessed"@en ;
        rdfs:domain   ids:UsageControlObject ;
        rdfs:range    xsd:dateTimeStamp ;
        rdfs:comment  "Last read or write access."@en .

ids:hasState  rdf:type  owl:ObjectProperty ;
        rdfs:label    "has state"@en ;
        rdfs:domain   ids:UsageControlObject ;
        rdfs:range    ids:ArtifactState ;
        rdfs:comment  "The list of combined current states of the data object."@en .

ids:requester  rdf:type  owl:ObjectProperty ;
        rdfs:label    "requesting application"@en ;
        rdfs:domain   ids:UsageControlObject ;
        rdfs:range    xsd:anyURI ;
        rdfs:comment  "\tThe target application requesting the usage. Should be some locally unique identifiers, preferably URIs."@en .
@prefix owl:   <http://www.w3.org/2002/07/owl#> .
@prefix rdf:   <http://www.w3.org/1999/02/22-rdf-syntax-ns#> .
@prefix rdfs:  <http://www.w3.org/2000/01/rdf-schema#> .
@prefix xsd:   <http://www.w3.org/2001/XMLSchema#> .
@prefix ids:   <https://w3id.org/idsa/core/> .
@prefix dct:   <http://purl.org/dc/terms/> .

ids:BusinessIdentifier
        rdf:type      owl:Class ;
        rdfs:label    "Business Identifier"@en ;
        rdfs:comment  "A business identifier is a identification number used to identify a company. E.g., the Data Universal Numbering System, abbreviated as DUNS"@en .

ids:identifierSystem  rdf:type  owl:DatatypeProperty ;
        rdfs:domain   ids:BusinessIdentifier ;
        rdfs:range    xsd:string ;
        rdfs:label    "identifier system"@en ;
        rdfs:comment  "This property is used to define the system used as an business identifier. E.g., DUNS or SIRET."@en .
@prefix owl:   <http://www.w3.org/2002/07/owl#> .
@prefix rdf:   <http://www.w3.org/1999/02/22-rdf-syntax-ns#> .
@prefix rdfs:  <http://www.w3.org/2000/01/rdf-schema#> .
@prefix foaf:  <http://xmlns.com/foaf/0.1/> .
@prefix org:   <http://www.w3.org/ns/org#> .
@prefix xsd:   <http://www.w3.org/2001/XMLSchema#> .
@prefix odrl:  <http://www.w3.org/ns/odrl/2/> .
@prefix ids:   <https://w3id.org/idsa/core/> .

ids:Participant  rdf:type  owl:Class ;
        rdfs:subClassOf  foaf:Agent ;
        rdfs:subClassOf  odrl:Party ;
        rdfs:subClassOf  ids:ManagedEntity ;
        rdfs:subClassOf  org:Organization ;
        rdfs:label       "Participant"@en ;
        rdfs:comment     "Stakeholder in the International Data Spaces, assuming one or more of the predefined roles; every participant is given a unique identity by the Identity Provider."@en .

ids:legalName  rdf:type  owl:DatatypeProperty ;
        rdfs:domain   ids:Participant ;
        rdfs:range    xsd:string ;
        rdfs:label    "legal name"@en ;
        rdfs:comment  "The complete legal name of a Participant. Unlike the title property for the participant which refers to the commonly used name or term for the Participant, a legal name identifies a participant for legal, administrative and other official purposes."@en .

ids:memberParticipant
        rdfs:subPropertyOf  org:hasMember ;
        rdf:type            owl:ObjectProperty ;
        rdfs:domain         ids:Participant ;
        rdfs:range          ids:Participant ;
        rdfs:label          "member participant"@en ;
        rdfs:comment        "Indicates that a participant has a member which is again a participant. This is useful for defining hierarchical relations in a participant's organization as well as identifying groups of participants to capture, e.g., members of a collaboration."@en .

ids:participantCertification
        rdf:type      owl:ObjectProperty ;
        rdfs:label    "participant certification"@en ;
        rdfs:domain   ids:Participant ;
        rdfs:range    ids:ParticipantCertification ;
        rdfs:comment  "Certification issued for the given Participant."@en .

ids:participantRefinement
        rdf:type      owl:ObjectProperty ;
        rdfs:label    "participant refinement"@en ;
        rdfs:domain   ids:Participant ;
        rdfs:range    odrl:Constraint ;
        rdfs:comment  "Conditions which needs to be satisfied that a single Participant can be seen as a member of the subject Participant. For instance, all Participants with their headquarter in Europe might be a potential consumer of GDPR-releated data."@en .

ids:businessIdentifier
        rdf:type      owl:ObjectProperty ;
        rdfs:domain   ids:Participant ;
        rdfs:range    ids:BusinessIdentifier ;
        rdfs:label    "has business identifier"@en ;
        rdfs:comment  "Company identifiers, described via ids:BusinessIdentifier."@en .

ids:vatID  rdf:type   owl:DatatypeProperty ;
        rdfs:domain   ids:Participant ;
        rdfs:range    xsd:string ;
        rdfs:label    "VAT ID"@en ;
        rdfs:comment  "The Value Added Tax ID (VAT ID) is used in the EU to clearly identify a company or entity which is liable for Value Added Tax."@en .

ids:legalForm  rdf:type  owl:DatatypeProperty ;
        rdfs:domain   ids:Participant ;
        rdfs:range    xsd:string ;
        rdfs:label    "legal form"@en ;
        rdfs:seeAlso  <https://www.gleif.org/en/about-lei/code-lists/iso-20275-entity-legal-forms-code-list/> ;
        rdfs:comment  "Legal form of the participant. It is advisable to use an existing standard such as ISO-20275."@en .

ids:jurisdiction  rdf:type  owl:DatatypeProperty ;
        rdfs:domain   ids:Participant ;
        rdfs:range    xsd:string ;
        rdfs:label    "legal form"@en ;
        rdfs:comment  "jurisdiction / court which is responsible for the entity. The use of existing standards such as ISO 3166-2 is recommended."@en .

ids:memberPerson  rdfs:subPropertyOf  org:hasMember ;
        rdf:type            owl:ObjectProperty ;
        rdfs:domain         ids:Participant ;
        rdfs:range          foaf:Person ;
        rdfs:label          "memberPerson"@en ;
        rdfs:comment        "Indicates membership of a person to an organization."@en .

ids:siteAddress  rdf:type  owl:DatatypeProperty ;
        rdfs:domain   org:Site ;
        rdfs:range    xsd:string ;
        rdfs:label    "site address"@en ;
        rdfs:comment  "Indicates an address for the site."@en .
@prefix owl:   <http://www.w3.org/2002/07/owl#> .
@prefix rdfs:  <http://www.w3.org/2000/01/rdf-schema#> .
@prefix dct:   <http://purl.org/dc/terms/> .
@prefix xsd:   <http://www.w3.org/2001/XMLSchema#> .
@prefix ids:   <https://w3id.org/idsa/core/> .

ids:AuthInfo  rdf:type  owl:Class ;
        rdfs:label    "AuthInfo"@en ;
        rdfs:comment  "Holds authentication information so that connections to the Connector's data offerings can be establised."@en .

ids:authService  rdf:type  owl:ObjectProperty ;
        rdfs:domain   ids:AuthInfo ;
        rdfs:range    xsd:anyURI ;
        rdfs:label    "authService"@en ;
        rdfs:comment  "The URL of the authentication service that is provided by the Connector."@en .

ids:authStandard  rdf:type  owl:ObjectProperty ;
        rdfs:domain   ids:AuthInfo ;
        rdfs:range    ids:AuthStandard ;
        rdfs:label    "authStandard"@en ;
        rdfs:comment  "The standard used by the authentication service that is provided by the Connector."@en .
@prefix owl:   <http://www.w3.org/2002/07/owl#> .
@prefix rdfs:  <http://www.w3.org/2000/01/rdf-schema#> .
@prefix dct:   <http://purl.org/dc/terms/> .
@prefix xsd:   <http://www.w3.org/2001/XMLSchema#> .
@prefix ids:   <https://w3id.org/idsa/core/> .
@prefix idsc:  <https://w3id.org/idsa/code/> .

ids:AuthStandard  rdf:type  owl:Class ;
        rdfs:label    "AuthStandard"@en ;
        rdfs:comment  "The class of authentication standards that may be supported by Connectors."@en .

idsc:OAUTH2_JWT  rdf:type  ids:AuthStandard ;
        rdfs:comment  "OAUTH2 via JWT" .
@prefix owl:   <http://www.w3.org/2002/07/owl#> .
@prefix rdfs:  <http://www.w3.org/2000/01/rdf-schema#> .
@prefix xsd:   <http://www.w3.org/2001/XMLSchema#> .
@prefix dct:   <http://purl.org/dc/terms/> .
@prefix ids:   <https://w3id.org/idsa/core/> .

ids:SecurityProfile  rdf:type  owl:Class ;
        rdfs:label    "SecurityProfile"@en ;
        rdfs:comment  "Set of security guarantees claimed by a Connector. Connectors may asses their mutual technical reliability and trustworthiness by evaluating each other’s security profile."@en .

ids:SecurityGuarantee
        rdf:type      owl:Class ;
        rdfs:label    "Security guarantee"@en ;
        rdfs:comment  "Security guarantee claimed by a security profile."@en .

ids:securityGuarantee
        rdf:type      owl:ObjectProperty ;
        rdfs:domain   ids:SecurityProfile ;
        rdfs:range    ids:SecurityGuarantee ;
        rdfs:label    "Security guarantee"@en ;
        rdfs:comment  "Reference to a security guarantee supported by given profile."@en .
@prefix owl:   <http://www.w3.org/2002/07/owl#> .
@prefix rdfs:  <http://www.w3.org/2000/01/rdf-schema#> .
@prefix dct:   <http://purl.org/dc/terms/> .
@prefix xsd:   <http://www.w3.org/2001/XMLSchema#> .
@prefix ids:   <https://w3id.org/idsa/core/> .

ids:Token  rdf:type   owl:Class ;
        rdfs:label    "Token."@en ;
        rdfs:comment  "A token (e.g., for authorization) mediated as part of the message."@en .

ids:DynamicAttributeToken
        rdf:type         owl:Class ;
        rdfs:subClassOf  ids:Token ;
        rdfs:label       "Dynamic Attribute Token (DAT)."@en ;
        rdfs:comment     "A JSON Web Token (e.g., for authorization) mediated as part of the message, formerly known as the 'DAPS Token'. The complete JWT *including* header, payload and signiture is referenced by this class and *not* only the JSON element in the payload. See ids:DatPayload for the payload definition."@en ;
        rdfs:seeAlso     <https://tools.ietf.org/html/rfc7519> ;
        rdfs:seeAlso     ids:DatPayload .

ids:TokenFormat  rdf:type  owl:Class ;
        rdfs:label    "Token format"@en ;
        rdfs:comment  "Possible formats for (security-related) tokens."@en .

ids:JwtPayload  rdf:type  owl:Class ;
        rdfs:label    "JWT Payload"@en ;
        rdfs:comment  "The payload of an JSON Web Token as a RDF class. Is used as the common parent of e.g., DatPayload and DatRequestPayload."@en .

ids:transportCertsSha256
        rdf:type      owl:DatatypeProperty ;
        rdfs:domain   ids:JwtPayload ;
        rdfs:range    xsd:string ;
        rdfs:label    "transportCertsSha256"@en ;
        rdfs:comment  "Separate certificates for IDS identification and transport encryption opens an attack vector for relay attacks. In order to prevent these attacks, a binding of this transport certificates to the connector is required. The inclusion of SHA256 fingerprints of currently valid transport certificates, mainly into the DAT, enables the client to relate the transport layer security with the IDS interactions."@en .

ids:DatPayload  rdf:type  owl:Class ;
        rdfs:subClassOf  ids:JwtPayload ;
        rdfs:label       "DAT Payload"@en ;
        rdfs:comment     "The Dynamic Attribute Token (DAT) Payload is the JSON Element of any DAT containing the claims of the token bearer. This payload itself is a JSON-LD encoded RDF class with a defined set of attributes. These attributes are either defined by RFC 7519 or by the IDS Information Model. As a direct consequence of regarding the DAT Payload as JSON-LD, *all* DAT Payloads must have exactly one \"@context\" attribute with the IDS context URI as its value and a \"@type\" with ids:DatPayload as its value."@en ;
        rdfs:seeAlso     <https://tools.ietf.org/html/rfc7519> .

ids:DatRequestPayload
        rdf:type         owl:Class ;
        rdfs:subClassOf  ids:JwtPayload ;
        rdfs:label       "DAT Request Payload"@en ;
        rdfs:comment     "The Dynamic Attribute Token (DAT) *Request* Payload is the JSON Element of any DAT containing the claims of the token bearer. This payload itself is a JSON-LD encoded RDF class with a defined set of attributes. These attributes are either defined by RFC 7519 or by the IDS Information Model. As a direct consequence of regarding the DAT Payload as JSON-LD, *all* DAT Payloads must have exactly one \"@context\" attribute with the IDS context URI as its value and a \"@type\" with ids:DatPayload as its value. Note that, different to the DatPayload, the DatRequestPayload contains the *self-claims* of a connector and is not yet signed by any DAPS. Consequently, no other connector must accept a DatRequest object as a DAT. A DatRequest and its contained DatRequestPayload is *only* intended for interactions with a DAPS and *nothing else*!"@en ;
        rdfs:seeAlso     <https://tools.ietf.org/html/rfc7519> .

ids:Audience  rdf:type  owl:Class ;
        rdfs:label    "Audience"@en ;
        rdfs:comment  "The class of audiences (recipients) used in the JWT. "@en ;
        rdfs:seeAlso  <https://tools.ietf.org/html/rfc7519> .

ids:aud  rdf:type     owl:ObjectProperty ;
        rdfs:label    "aud"@en ;
        rdfs:domain   ids:JwtPayload ;
        rdfs:range    ids:Audience ;
        rdfs:seeAlso  <https://tools.ietf.org/html/rfc7519#section-4.1.3> ;
        rdfs:comment  "The 'aud' (audience) claim identifies the recipients that the JWT is intended for."@en .

ids:exp  rdf:type     owl:DatatypeProperty ;
        rdfs:label    "exp"@en ;
        rdfs:domain   ids:JwtPayload ;
        rdfs:range    xsd:integer ;
        rdfs:seeAlso  <https://tools.ietf.org/html/rfc7519#section-4.1.4> ;
        rdfs:comment  "The 'exp' (expiration time) claim identifies the expiration time on or after which the JWT MUST NOT be accepted for processing."@en .

ids:iat  rdf:type     owl:DatatypeProperty ;
        rdfs:label    "iat"@en ;
        rdfs:domain   ids:JwtPayload ;
        rdfs:range    xsd:integer ;
        rdfs:comment  "The 'iat' (issued at) claim contains the point in time when the JWT was created."@en .

ids:iss  rdf:type     owl:DatatypeProperty ;
        rdfs:label    "iss"@en ;
        rdfs:domain   ids:JwtPayload ;
        rdfs:range    xsd:string ;
        rdfs:seeAlso  <https://tools.ietf.org/html/rfc7519#section-4.1.1> ;
        rdfs:comment  "The 'iss' (issuer) claim identifies the principal that issued the JWT."@en .

ids:nbf  rdf:type     owl:DatatypeProperty ;
        rdfs:label    "nbf"@en ;
        rdfs:domain   ids:JwtPayload ;
        rdfs:range    xsd:integer ;
        rdfs:seeAlso  <https://tools.ietf.org/html/rfc7519#section-4.1.5> ;
        rdfs:comment  "The 'aud' (audience) claim identifies the recipients that the JWT is intended for."@en .

ids:referringConnector
        rdf:type      owl:DatatypeProperty ;
        rdfs:label    "referringConnector"@en ;
        rdfs:domain   ids:JwtPayload ;
        rdfs:range    ids:Connector ;
        rdfs:comment  "The RDF connector entity as referred to by the DAT, with its URI included as the value. The value MUST be its accessible URI."@en .

ids:scope  rdf:type   owl:DatatypeProperty ;
        rdfs:label    "scope"@en ;
        rdfs:domain   ids:JwtPayload ;
        rdfs:range    xsd:string ;
        rdfs:seeAlso  <https://tools.ietf.org/html/rfc7519#section-4.1.2> ;
        rdfs:comment  "Currently, the scope is limited to 'Connector' but can be used for scoping purposes in the future. Scope is currently fixed to 'https://w3id.org/idsa/core/Connector'."@en .

ids:sub  rdf:type     owl:DatatypeProperty ;
        rdfs:label    "sub"@en ;
        rdfs:domain   ids:JwtPayload ;
        rdfs:range    xsd:string ;
        rdfs:seeAlso  <https://tools.ietf.org/html/rfc7519#section-4.1.2> ;
        rdfs:comment  "The 'sub' (subject) claim identifies the principal that is the subject of the JWT."@en .

ids:tokenValue  rdf:type  owl:DatatypeProperty ;
        rdfs:label    "tokenValue"@en ;
        rdfs:domain   ids:Token ;
        rdfs:range    xsd:string ;
        rdfs:comment  "An authentication token value like JSON Web Token."@en .

ids:tokenFormat  rdf:type  owl:ObjectProperty ;
        rdfs:label    "tokenFormat"@en ;
        rdfs:domain   ids:Token ;
        rdfs:range    ids:TokenFormat ;
        rdfs:comment  "Describes the format of the authentication token."@en .
@prefix owl:   <http://www.w3.org/2002/07/owl#> .
@prefix rdfs:  <http://www.w3.org/2000/01/rdf-schema#> .
@prefix dct:   <http://purl.org/dc/terms/> .
@prefix xsd:   <http://www.w3.org/2001/XMLSchema#> .
@prefix ids:   <https://w3id.org/idsa/core/> .

ids:UserAuthentication
        rdf:type      owl:Class ;
        rdfs:label    "User Authentication"@en ;
        rdfs:comment  "Holds User authentication information. Differs from ids:AuthInfo. This class refers to user authentication methods that are not intended for direct data exchange with a connector."@en .

ids:authUsername  rdf:type  owl:DatatypeProperty ;
        rdfs:domain   ids:UserAuthentication ;
        rdfs:range    xsd:string ;
        rdfs:label    "auth username"@en ;
        rdfs:comment  "Username / ID used for authentication."@en .

ids:BasicAuthentication
        rdf:type         owl:Class ;
        rdfs:subClassOf  ids:UserAuthentication ;
        rdfs:label       "User Authentication"@en ;
        rdfs:comment     "Basic authentication using username / password "@en ;
        rdfs:seeAlso     <https://tools.ietf.org/html/rfc7617> .

ids:authPassword  rdf:type  owl:DatatypeProperty ;
        rdfs:domain   ids:BasicAuthentication ;
        rdfs:range    xsd:string ;
        rdfs:label    "auth password" ;
        rdfs:comment  "Username / ID used for authentication." .

ids:HTTPAuthentication
        rdf:type         owl:Class ;
        rdfs:subClassOf  ids:BasicAuthentication ;
        rdfs:label       "HTTP Authentication"@en ;
        rdfs:comment     "HTTP authentication."@en .

ids:httpAuthURI  rdf:type  owl:DatatypeProperty ;
        rdfs:domain   ids:HTTPAuthentication ;
        rdfs:range    xsd:anyURI ;
        rdfs:label    "http auth URI"@en ;
        rdfs:comment  "HTTP authentication URI."@en ;
        rdfs:seeAlso  <https://tools.ietf.org/html/rfc7235> .
@prefix owl:   <http://www.w3.org/2002/07/owl#> .
@prefix dct:   <http://purl.org/dc/terms/> .
@prefix rdfs:  <http://www.w3.org/2000/01/rdf-schema#> .
@prefix odrl:  <http://www.w3.org/ns/odrl/2/> .
@prefix xsd:   <http://www.w3.org/2001/XMLSchema#> .
@prefix ids:   <https://w3id.org/idsa/core/> .

ids:EvaluationFacility
        rdf:type      owl:Class ;
        rdfs:label    "Evaluation Facility"@en ;
        rdfs:comment  "Evaluation Facilities carry out the evaluation work during a certification process and issue the corresponding Certifications."@en .

ids:Certification  rdf:type  owl:Class ;
        rdfs:subClassOf  ids:ManagedEntity ;
        rdfs:label       "Certification"@en ;
        rdfs:comment     "Abstract certification of compliance according to given Certification Scheme."@en .

ids:CertificationLevel
        rdf:type      owl:Class ;
        rdfs:label    "Certification Level"@en ;
        rdfs:comment  "Level of Certification"@en .

ids:includedCertificationLevel
        rdf:type            owl:ObjectProperty ;
        rdfs:subPropertyOf  dct:isPartOf ;
        rdfs:seeAlso        <https://www.w3.org/TR/odrl-vocab/#term-includedIn> ;
        rdfs:label          "included certification level"@en ;
        rdfs:domain         ids:CertificationLevel ;
        rdfs:range          ids:CertificationLevel ;
        rdfs:comment        "Certification Level transitively implied by given Certification Level of same root type."@en .

ids:certificationLevel
        rdf:type      owl:ObjectProperty ;
        rdfs:label    "certification level"@en ;
        rdfs:domain   ids:Certification ;
        rdfs:range    ids:CertificationLevel ;
        rdfs:comment  "Level of certification (based on a combination of requierements, evaluation method etc.)"@en .

ids:lastValidDate  rdf:type  owl:DatatypeProperty ;
        rdfs:label    "last valid date"@en ;
        rdfs:domain   ids:Certification ;
        rdfs:range    xsd:dateTimeStamp ;
        rdfs:comment  "Last date (as xsd:dateTimeStamp) the given Certification is considered valid."@en .

ids:evaluationFacility
        rdf:type      owl:ObjectProperty ;
        rdfs:label    "evaluation facility"@en ;
        rdfs:domain   ids:Certification ;
        rdfs:range    ids:EvaluationFacility ;
        rdfs:comment  "Evaluation Facility that performed and issued given Certification"@en .
@prefix dc:    <http://purl.org/dc/elements/1.1/> .
@prefix dct:   <http://purl.org/dc/terms/> .
@prefix ids:   <https://w3id.org/idsa/core/> .
@prefix owl:   <http://www.w3.org/2002/07/owl#> .
@prefix rdf:   <http://www.w3.org/1999/02/22-rdf-syntax-ns#> .
@prefix rdfs:  <http://www.w3.org/2000/01/rdf-schema#> .
@prefix skos:  <http://www.w3.org/2004/02/skos/core#> .
@prefix xsd:   <http://www.w3.org/2001/XMLSchema#> .

ids:Described  rdf:type  owl:Class ;
        rdfs:label    "described"@en ;
        rdfs:comment  "Entity described by a minimal textual annotation, i.e. a title and description."@en .
@prefix dc:    <http://purl.org/dc/elements/1.1/> .
@prefix dct:   <http://purl.org/dc/terms/> .
@prefix ids:   <https://w3id.org/idsa/core/> .
@prefix owl:   <http://www.w3.org/2002/07/owl#> .
@prefix rdf:   <http://www.w3.org/1999/02/22-rdf-syntax-ns#> .
@prefix rdfs:  <http://www.w3.org/2000/01/rdf-schema#> .
@prefix skos:  <http://www.w3.org/2004/02/skos/core#> .
@prefix xsd:   <http://www.w3.org/2001/XMLSchema#> .
@prefix sh:    <http://www.w3.org/ns/shacl#> .
@prefix void:  <http://rdfs.org/ns/void#> .

ids:DescribedSemantically
        rdf:type      owl:Class ;
        rdfs:label    "DescribedSemantically"@en ;
        rdfs:comment  "Entity described semantically."@en .
@prefix dc:    <http://purl.org/dc/elements/1.1/> .
@prefix dct:   <http://purl.org/dc/terms/> .
@prefix ids:   <https://w3id.org/idsa/core/> .
@prefix owl:   <http://www.w3.org/2002/07/owl#> .
@prefix rdf:   <http://www.w3.org/1999/02/22-rdf-syntax-ns#> .
@prefix rdfs:  <http://www.w3.org/2000/01/rdf-schema#> .
@prefix skos:  <http://www.w3.org/2004/02/skos/core#> .
@prefix xsd:   <http://www.w3.org/2001/XMLSchema#> .

ids:Named  rdf:type  owl:Class .

_:b2    rdf:type         owl:Restriction ;
        owl:onProperty   ids:name ;
        owl:cardinality  "1"^^xsd:nonNegativeInteger .

ids:Named  owl:equivalentClass  _:b2 ;
        rdfs:label           "Named"@en ;
        rdfs:comment         "Entity that is identifiable within a context by means of a name."@en .

ids:name  rdf:type    owl:DatatypeProperty ;
        rdf:type      owl:FunctionalProperty ;
        rdfs:label    "name"@en ;
        rdfs:domain   ids:Named ;
        rdfs:range    xsd:string ;
        rdfs:comment  "Entity name unique within a specified context."@en .
@prefix owl:   <http://www.w3.org/2002/07/owl#> .
@prefix rdfs:  <http://www.w3.org/2000/01/rdf-schema#> .
@prefix dct:   <http://purl.org/dc/terms/> .
@prefix xsd:   <http://www.w3.org/2001/XMLSchema#> .
@prefix locn:  <http://www.w3.org/ns/locn#> .
@prefix gn:    <http://www.geonames.org/ontology#> .
@prefix wgs84: <http://www.w3.org/2003/01/geo/wgs84_pos#> .
@prefix geo:   <http://www.opengis.net/def/function/geosparql/> .
@prefix ids:   <https://w3id.org/idsa/core/> .
@prefix idsc:  <https://w3id.org/idsa/code/> .

ids:Location  rdf:type   owl:Class ;
        rdfs:subClassOf  dct:Location ;
        rdfs:subClassOf  wgs84:SpatialThing ;
        rdfs:label       "Location"@en ;
        rdfs:comment     "Class of all locations."@en .

ids:GeoPoint  rdfs:subClassOf  ids:Location ;
        rdf:type         owl:Class ;
        rdfs:label       "GeoPoint"@en ;
        rdfs:comment     "A location identified by geo coordinates."@en .

ids:GeoFeature  rdf:type  owl:Class ;
        rdfs:subClassOf  gn:Feature ;
        rdfs:subClassOf  ids:Location ;
        rdfs:label       "GeoFeature"@en ;
        rdfs:comment     "A location identified by a geonames URL."@en .

ids:Geometry  rdfs:subClassOf  locn:Geometry ;
        rdfs:subClassOf  ids:Location ;
        rdf:type         owl:Class ;
        rdfs:label       "Geometry"@en ;
        rdfs:comment     "Geometrical shape indicating a spatial area of interest."@en .

ids:BoundingPolygon  rdfs:subClassOf  ids:Geometry ;
        rdf:type         owl:Class ;
        rdfs:label       "BoundingPolygon"@en ;
        rdfs:comment     "Defines an area of interest as a set of connected points."@en .

ids:latitude  rdfs:subPropertyOf  wgs84:lat ;
        rdf:type            owl:DatatypeProperty ;
        rdfs:domain         ids:GeoPoint ;
        rdfs:range          xsd:float ;
        rdfs:label          "latitude"@en ;
        rdfs:comment        "Latitude of a GeoPoint (decimal degrees)."@en .

ids:longitude  rdfs:subPropertyOf  wgs84:long ;
        rdf:type            owl:DatatypeProperty ;
        rdfs:domain         ids:GeoPoint ;
        rdfs:range          xsd:float ;
        rdfs:label          "longitude"@en ;
        rdfs:comment        "Longitude of a GeoPoint (decimal degrees)."@en .

ids:geoPoint  rdf:type  owl:ObjectProperty ;
        rdfs:domain   ids:BoundingPolygon ;
        rdfs:range    ids:GeoPoint ;
        rdfs:label    "geoPoint"@en ;
        rdfs:comment  "Refers to a GeoPoint that is member of a BoundingPolygon."@en .
@prefix owl:   <http://www.w3.org/2002/07/owl#> .
@prefix rdfs:  <http://www.w3.org/2000/01/rdf-schema#> .
@prefix skos:  <http://www.w3.org/2004/02/skos/core#> .
@prefix dct:   <http://purl.org/dc/terms/> .
@prefix time:  <http://www.w3.org/2006/time#> .
@prefix xsd:   <http://www.w3.org/2001/XMLSchema#> .
@prefix ids:   <https://w3id.org/idsa/core/> .
@prefix idsc:  <https://w3id.org/idsa/code/> .
@prefix greg:  <http://www.w3.org/ns/time/gregorian#> .

ids:DurationEntity  rdf:type  owl:Class ;
        rdfs:subClassOf  time:TemporalEntity ;
        rdfs:label       "Duration"@en ;
        rdfs:comment     "A relative temporal entity of a certain length. Different to time:Interval, the starting point is not (yet) defined. Specifying a starting or ending point automatically transformes an instance of ids:DurationEntity to an time:Interval."@en .

ids:Frequency  rdf:type      owl:Class ;
        owl:equivalentClass  dct:Frequency ;
        rdfs:label           "Frequency"@en ;
        rdfs:comment         "Class of all frequencies."@en .

ids:hasDuration  rdf:type  owl:DatatypeProperty ;
        rdfs:seeAlso  time:hasDuration ;
        rdfs:domain   time:TemporalEntity ;
        rdfs:range    xsd:duration ;
        rdfs:label    "has duration"@en ;
        rdfs:comment  "Duration (relative time interval) of a temporal specification. Different to the TIME Ontology, durations are expressed using the xsd:duration datatype. In case it is used with a instance of time:Instant, the value must be 'P0Y0M0DT0H0M0S'^^xsd:duration."@en .
@prefix owl:   <http://www.w3.org/2002/07/owl#> .
@prefix rdfs:  <http://www.w3.org/2000/01/rdf-schema#> .
@prefix ids:   <https://w3id.org/idsa/core/> .

ids:AppStore  rdf:type   owl:Class ;
        rdfs:subClassOf  ids:Connector ;
        rdfs:label       "App Store"@en ;
        rdfs:comment     "Secure platform for distributing Data Apps."@en .
@prefix owl:   <http://www.w3.org/2002/07/owl#> .
@prefix rdfs:  <http://www.w3.org/2000/01/rdf-schema#> .
@prefix ids:   <https://w3id.org/idsa/core/> .
@prefix dct:   <http://purl.org/dc/terms/> .

ids:Broker  rdf:type     owl:Class ;
        rdfs:subClassOf  ids:Connector ;
        rdfs:label       "Broker"@en ;
        rdfs:comment     "Broker holding an index of published data endpoints."@en .

ids:connectorCatalog  rdf:type  owl:ObjectProperty ;
        rdfs:label    "connector Catalog"@en ;
        rdfs:domain   ids:Broker ;
        rdfs:range    ids:ConnectorCatalog ;
        rdfs:comment  "Reference to catalog of Connectors, which are listed in the Broker."@en .
@prefix rdf:   <http://www.w3.org/1999/02/22-rdf-syntax-ns#> .
@prefix owl:   <http://www.w3.org/2002/07/owl#> .
@prefix rdfs:  <http://www.w3.org/2000/01/rdf-schema#> .
@prefix xsd:   <http://www.w3.org/2001/XMLSchema#> .
@prefix dcat:  <http://www.w3.org/ns/dcat#> .
@prefix ids:   <https://w3id.org/idsa/core/> .
@prefix odrl:  <http://www.w3.org/ns/odrl/2/> .

ids:ResourceCatalog  rdf:type  owl:Class ;
        rdfs:subClassOf  dcat:Catalog ;
        rdfs:subClassOf  odrl:AssetCollection ;
        rdfs:label       "Resource Catalog"@en ;
        rdfs:comment     "Class that aggregates Resources from a (distributable) Catalog."@en .

ids:ParticipantCatalog
        rdf:type         owl:Class ;
        rdfs:subClassOf  dcat:Catalog ;
        rdfs:subClassOf  odrl:AssetCollection ;
        rdfs:label       "Participant Catalog"@en ;
        rdfs:comment     "Class that aggregates Participants from a (distributable) Catalog."@en .

ids:ConnectorCatalog  rdf:type  owl:Class ;
        rdfs:subClassOf  dcat:Catalog ;
        rdfs:subClassOf  odrl:AssetCollection ;
        rdfs:label       "Connector Catalog"@en ;
        rdfs:comment     "Class that aggregates Connectors from a (distributable) Catalog."@en .

ids:BrokerCatalog  rdf:type  owl:Class ;
        rdfs:subClassOf  ids:ConnectorCatalog ;
        rdfs:label       "Broker Catalog"@en ;
        rdfs:comment     "Class that aggregates Brokers from a (distributable) Catalog."@en .

ids:AppStoreCatalog  rdf:type  owl:Class ;
        rdfs:subClassOf  ids:ConnectorCatalog ;
        rdfs:label       "AppStore Catalog"@en ;
        rdfs:comment     "Class that aggregates AppStores from a (distributable) Catalog."@en .

ids:AppResourceCatalog
        rdf:type         owl:Class ;
        rdfs:subClassOf  dcat:Catalog ;
        rdfs:subClassOf  odrl:AssetCollection ;
        rdfs:label       "App Resource Catalog"@en ;
        rdfs:comment     "Class that aggregates App Resources from a (distributable) Catalog. May be used to list installed apps in a component."@en .

ids:ClearingHouseCatalog
        rdfs:subClassOf  dcat:Catalog ;
        rdfs:subClassOf  odrl:AssetCollection ;
        rdf:type         owl:Class ;
        rdfs:label       "Clearing House Catalog"@en ;
        rdfs:comment     "Class that aggregates Clearing Houses from a (distributable) Catalog."@en .

ids:offeredResource  rdf:type  owl:ObjectProperty ;
        rdfs:subPropertyOf  dcat:dataset ;
        rdfs:domain         ids:ResourceCatalog ;
        rdfs:range          ids:Resource ;
        rdfs:label          "offered resource"@en ;
        rdfs:comment        "A Resource that is part of a resource catalog, indicating an offering (of, e.g., data)."@en .

ids:requestedResource
        rdf:type            owl:ObjectProperty ;
        rdfs:subPropertyOf  dcat:dataset ;
        rdfs:domain         ids:ResourceCatalog ;
        rdfs:range          ids:Resource ;
        rdfs:label          "requested resource"@en ;
        rdfs:comment        "A Resource that is part of a resource catalog, indicating a request (of, e.g., data, software, …)."@en .

ids:member  rdf:type        owl:ObjectProperty ;
        rdfs:subPropertyOf  dcat:dataset ;
        rdfs:domain         ids:ParticipantCatalog ;
        rdfs:range          ids:Participant ;
        rdfs:label          "member"@en ;
        rdfs:comment        "A Participant that is part of a participant catalog."@en .

ids:listedConnector  rdf:type  owl:ObjectProperty ;
        rdfs:subPropertyOf  dcat:dataset ;
        rdfs:domain         ids:ConnectorCatalog ;
        rdfs:range          ids:Connector ;
        rdfs:label          "listed Connector"@en ;
        rdfs:comment        "A Connector that is part of a Connector catalog."@en .

ids:listedClearingHouse
        rdf:type            owl:ObjectProperty ;
        rdfs:subPropertyOf  dcat:dataset ;
        rdfs:domain         ids:ClearingHouseCatalog ;
        rdfs:range          ids:ClearingHouse ;
        rdfs:label          "listed Clearing House"@en ;
        rdfs:comment        "A Clearing House that is part of a Clearing House catalog."@en .

ids:listedAppResource
        rdf:type            owl:ObjectProperty ;
        rdfs:subPropertyOf  dcat:dataset ;
        rdfs:domain         ids:AppResourceCatalog ;
        rdfs:range          ids:AppResource ;
        rdfs:label          "listed AppResource"@en ;
        rdfs:comment        "An AppResource that is part of an AppResourceCatalog."@en .
@prefix owl:   <http://www.w3.org/2002/07/owl#> .
@prefix rdfs:  <http://www.w3.org/2000/01/rdf-schema#> .
@prefix ids:   <https://w3id.org/idsa/core/> .
@prefix dct:   <http://purl.org/dc/terms/> .

ids:ClearingHouse  rdf:type  owl:Class ;
        rdfs:subClassOf  ids:InfrastructureComponent ;
        rdfs:label       "Clearing House"@en ;
        rdfs:comment     "The Clearing House provides clearing and settlement services B2B interactions within the International Data Spaces."@en .
@prefix owl:   <http://www.w3.org/2002/07/owl#> .
@prefix rdfs:  <http://www.w3.org/2000/01/rdf-schema#> .
@prefix xsd:   <http://www.w3.org/2001/XMLSchema#> .
@prefix ids:   <https://w3id.org/idsa/core/> .

ids:ConfigurationModel
        rdf:type      owl:Class ;
        rdfs:label    "Configuration Model"@en ;
        rdfs:comment  "Configuration Model is used for Connector deployment."@en .

ids:userAuthentication
        rdf:type      owl:ObjectProperty ;
        rdfs:label    "user authentication"@en ;
        rdfs:comment  "authentication methods allowed in a Configuration Model"@en ;
        rdfs:domain   ids:ConfigurationModel ;
        rdfs:range    ids:UserAuthentication .

ids:configurationModelLogLevel
        rdf:type      owl:ObjectProperty ;
        rdfs:label    "configuration model log level"@en ;
        rdfs:comment  "Log level configuration for a Connector which is deployed using the Configuration Model"@en ;
        rdfs:domain   ids:ConfigurationModel ;
        rdfs:range    ids:LogLevel .

ids:connectorStatus  rdf:type  owl:ObjectProperty ;
        rdfs:label    "Connector Status"@en ;
        rdfs:comment  "Status of a Connector deployed by the Configuration Model"@en ;
        rdfs:domain   ids:ConfigurationModel ;
        rdfs:range    ids:ConnectorStatus .

ids:connectorDeployMode
        rdf:type      owl:ObjectProperty ;
        rdfs:label    "connector deploy mode"@en ;
        rdfs:comment  "Deply mode of a Connector in the Configuration Model"@en ;
        rdfs:domain   ids:ConfigurationModel ;
        rdfs:range    ids:ConnectorDeployMode .

ids:connectorDescription
        rdf:type      owl:ObjectProperty ;
        rdfs:label    "Connector description"@en ;
        rdfs:comment  "References to Connector which is deployed / maintained in the Configuration Model"@en ;
        rdfs:domain   ids:ConfigurationModel ;
        rdfs:range    ids:Connector .

ids:connectorProxy  rdf:type  owl:ObjectProperty ;
        rdfs:label    "Connector proxy"@en ;
        rdfs:comment  "Proxies for a Connector which is deployed using the Configuration Model"@en ;
        rdfs:domain   ids:ConfigurationModel ;
        rdfs:range    ids:Proxy .

ids:trustStore  rdf:type  owl:DatatypeProperty ;
        rdfs:domain   ids:ConfigurationModel ;
        rdfs:range    xsd:anyURI ;
        rdfs:label    "trust store"@en ;
        rdfs:comment  "URI of the trust store server."@en .

ids:trustStoreAlias  rdf:type  owl:DatatypeProperty ;
        rdfs:domain   ids:ConfigurationModel ;
        rdfs:range    xsd:string ;
        rdfs:label    "trust store alias"@en ;
        rdfs:comment  "alias for the trust store."@en .

ids:trustStorePassword
        rdf:type      owl:DatatypeProperty ;
        rdfs:domain   ids:ConfigurationModel ;
        rdfs:range    xsd:string ;
        rdfs:label    "trust store password"@en ;
        rdfs:comment  "Password of the trust store server."@en .

ids:keyStore  rdf:type  owl:DatatypeProperty ;
        rdfs:domain   ids:ConfigurationModel ;
        rdfs:range    xsd:anyURI ;
        rdfs:label    "key store"@en ;
        rdfs:comment  "URI of the key store server."@en .

ids:keyStoreAlias  rdf:type  owl:DatatypeProperty ;
        rdfs:domain   ids:ConfigurationModel ;
        rdfs:range    xsd:string ;
        rdfs:label    "key store alias"@en ;
        rdfs:comment  "alias for the key store."@en .

ids:keyStorePassword  rdf:type  owl:DatatypeProperty ;
        rdfs:domain   ids:ConfigurationModel ;
        rdfs:range    xsd:string ;
        rdfs:label    "key store password"@en ;
        rdfs:comment  "Password of the key store server."@en .

ids:configuredBroker  rdf:type  owl:ObjectProperty ;
        rdfs:domain   ids:ConfigurationModel ;
        rdfs:range    ids:BrokerCatalog ;
        rdfs:label    "configured broker"@en ;
        rdfs:comment  "Catalog of Brokers to which the ids:Connector that we are configuring (cf. ids:connectorDescription) may want to talk."@en .

ids:appRoute  rdf:type  owl:ObjectProperty ;
        rdfs:label   "app route" ;
        rdfs:domain  ids:ConfigurationModel ;
        rdfs:range   ids:AppRoute .

ids:configuredAppStore
        rdf:type      owl:ObjectProperty ;
        rdfs:domain   ids:ConfigurationModel ;
        rdfs:range    ids:AppStoreCatalog ;
        rdfs:label    "configured appstore"@en ;
        rdfs:comment  "One or more app stores to which the ids:Connector that we are configuring (cf. ids:connectorDescription) may want to talk, e.g., to retrieve apps from them."@en .

ids:configuredAppResource
        rdf:type      owl:ObjectProperty ;
        rdfs:domain   ids:ConfigurationModel ;
        rdfs:range    ids:AppResourceCatalog ;
        rdfs:label    "configured app resources"@en ;
        rdfs:comment  "Catalog of app resources for a given Configuration Model. Used to persist configured / installed apps."@en .

ids:configuredClearingHouse
        rdf:type      owl:ObjectProperty ;
        rdfs:domain   ids:ConfigurationModel ;
        rdfs:range    ids:ClearingHouseCatalog ;
        rdfs:label    "configured clearing house"@en ;
        rdfs:comment  "Catalog of clearing houses for a given Configuration Model."@en .
@prefix rdf:   <http://www.w3.org/1999/02/22-rdf-syntax-ns#> .
@prefix owl:   <http://www.w3.org/2002/07/owl#> .
@prefix rdfs:  <http://www.w3.org/2000/01/rdf-schema#> .
@prefix foaf:  <http://xmlns.com/foaf/0.1/> .
@prefix xsd:   <http://www.w3.org/2001/XMLSchema#> .
@prefix ids:   <https://w3id.org/idsa/core/> .

ids:Connector  rdfs:subClassOf  ids:InfrastructureComponent ;
        rdf:type         owl:Class ;
        rdfs:label       "Connector"@en ;
        rdfs:comment     "Dedicated communication server for sending and receiving data in compliance with the Connector specification. There are different types of Connectors according to provided capabilities."@en .

ids:BaseConnector  rdfs:subClassOf  ids:Connector ;
        rdf:type         owl:Class ;
        rdfs:label       "Base Connector"@en ;
        rdfs:comment     "Implementation of the Connector specification providing only restricted security capabilities."@en .

ids:TrustedConnector  rdfs:subClassOf  ids:Connector ;
        rdf:type         owl:Class ;
        rdfs:label       "Trusted Connector"@en ;
        rdfs:comment     "Hardened implementation of the Connector specification providing enhanced security capabilities."@en .

ids:hasDefaultEndpoint
        rdf:type      owl:ObjectProperty ;
        rdfs:label    "has default endpoint"@en ;
        rdfs:domain   ids:Connector ;
        rdfs:range    ids:ConnectorEndpoint ;
        rdfs:comment  "Indicates the default endpoint that should be used for basic infrastructure interactions, e.g., providing the self description."@en .

ids:hasEndpoint  rdf:type  owl:ObjectProperty ;
        rdfs:label    "has endpoint"@en ;
        rdfs:domain   ids:Connector ;
        rdfs:range    ids:ConnectorEndpoint ;
        rdfs:comment  "Reference to the Endpoints that serve the resource's content or let you exchange messages with an IDS Connector."@en .

ids:securityProfile  rdf:type  owl:ObjectProperty .

_:b3    rdf:type  owl:Class .

_:b4    rdf:first  ids:Connector ;
        rdf:rest   _:b5 .

_:b5    rdf:first  ids:JwtPayload ;
        rdf:rest   rdf:nil .

_:b3    owl:unionOf  _:b4 .

ids:securityProfile  rdfs:domain  _:b3 ;
        rdfs:range    ids:SecurityProfile ;
        rdfs:label    "securityProfile"@en ;
        rdfs:comment  "The SecurityProfile supported by the Connector."@en .

ids:extendedGuarantee
        rdf:type  owl:ObjectProperty .

_:b6    rdf:type  owl:Class .

_:b7    rdf:first  ids:Connector ;
        rdf:rest   _:b8 .

_:b8    rdf:first  ids:DatPayload ;
        rdf:rest   rdf:nil .

_:b6    owl:unionOf  _:b7 .

ids:extendedGuarantee
        rdfs:domain   _:b6 ;
        rdfs:range    ids:SecurityGuarantee ;
        rdfs:label    "extended guarantee"@en ;
        rdfs:comment  "Reference to a security guarantee that, if used in combination with a security profile instance, overrides the respective guarantee of the given predefined instance."@en .

ids:authInfo  rdf:type  owl:ObjectProperty ;
        rdfs:domain   ids:Connector ;
        rdfs:range    ids:AuthInfo ;
        rdfs:label    "authInfo"@en ;
        rdfs:comment  "Information of the authentication service used by the Connector."@en .

ids:resourceCatalog  rdf:type  owl:ObjectProperty ;
        rdfs:domain   ids:Connector ;
        rdfs:range    ids:ResourceCatalog ;
        rdfs:label    "resource catalog"@en ;
        rdfs:comment  "References the Catalog of published or requested resource by this Connector."@en .

ids:hasAgent  rdf:type  owl:ObjectProperty ;
        rdfs:label    "has Agent"@en ;
        rdfs:domain   ids:Connector ;
        rdfs:range    foaf:Agent ;
        rdfs:comment  "The Agents for which this Connector may initiate and receive Messages."@en .
@prefix owl:   <http://www.w3.org/2002/07/owl#> .
@prefix rdfs:  <http://www.w3.org/2000/01/rdf-schema#> .
@prefix ids:   <https://w3id.org/idsa/core/> .
@prefix dct:   <http://purl.org/dc/terms/> .

ids:DAPS  rdf:type       owl:Class ;
        rdfs:subClassOf  ids:InfrastructureComponent ;
        rdfs:label       "Dynamic Attribute Provisioning Service"@en ;
        rdfs:comment     "The Dynamic Attribute Provisioning Service (DAPS) is a component of the Identity Provider and manages and issues the Dynamic Attribute Tokens (DAT), acting as digtial proofs for dynamic attributes of both connectors and participants."@en .
@prefix owl:   <http://www.w3.org/2002/07/owl#> .
@prefix rdfs:  <http://www.w3.org/2000/01/rdf-schema#> .
@prefix ids:   <https://w3id.org/idsa/core/> .
@prefix dct:   <http://purl.org/dc/terms/> .

ids:IdentityProvider  rdf:type  owl:Class ;
        rdfs:subClassOf  ids:InfrastructureComponent ;
        rdfs:label       "Identity provider"@en ;
        rdfs:comment     "The Identity Provider manages and validates the digital identity of International Data Spaces Participants."@en .
@prefix owl:   <http://www.w3.org/2002/07/owl#> .
@prefix dct:   <http://purl.org/dc/terms/> .
@prefix rdfs:  <http://www.w3.org/2000/01/rdf-schema#> .
@prefix prov:  <http://www.w3.org/ns/prov#> .
@prefix rdf:   <http://www.w3.org/1999/02/22-rdf-syntax-ns#> .
@prefix xsd:   <http://www.w3.org/2001/XMLSchema#> .
@prefix ids:   <https://w3id.org/idsa/core/> .

ids:InfrastructureComponent
        rdfs:subClassOf  ids:ManagedEntity ;
        rdf:type         owl:Class ;
        rdfs:label       "InfrastructureComponent"@en ;
        rdfs:comment     "The class of all infrastructure components of the IDS."@en .

ids:maintainer  rdf:type  owl:ObjectProperty ;
        rdfs:domain   ids:InfrastructureComponent ;
        rdfs:range    ids:Participant ;
        rdfs:label    "maintainer"@en ;
        rdfs:comment  "Participant responsible for technical maintenance of the InfrastructureComponent."@en .

ids:curator  rdf:type       owl:ObjectProperty ;
        rdfs:subPropertyOf  dct:publisher ;
        rdfs:domain         ids:InfrastructureComponent ;
        rdfs:range          ids:Participant ;
        rdfs:label          "curator"@en ;
        rdfs:comment        "Participant responsible for the correctness of the content offered by the InfrastructureComponent."@en .

ids:physicalLocation  rdf:type  owl:ObjectProperty ;
        rdfs:label    "physicalLocation"@en ;
        rdfs:domain   ids:InfrastructureComponent ;
        rdfs:range    ids:Location ;
        rdfs:comment  "The location where the Connector is physically deployed."@en .

ids:inboundModelVersion
        rdf:type      owl:DatatypeProperty ;
        rdfs:label    "inboundModelVersion"@en ;
        rdfs:domain   ids:InfrastructureComponent ;
        rdfs:range    xsd:string ;
        rdfs:comment  "Information Model version that the InfrastructureComponent is capable of reading/processing."@en .

ids:outboundModelVersion
        rdf:type      owl:DatatypeProperty ;
        rdfs:label    "outbound model version"@en ;
        rdfs:domain   ids:InfrastructureComponent ;
        rdfs:range    xsd:string ;
        rdfs:comment  "Information Model version being produced by the InfrastructureComponent."@en .

ids:componentCertification
        rdf:type      owl:ObjectProperty ;
        rdfs:label    "component certification"@en ;
        rdfs:domain   ids:InfrastructureComponent ;
        rdfs:range    ids:ComponentCertification ;
        rdfs:comment  "Certification issued for the given Infrastructure Component."@en .

ids:publicKey  rdf:type  owl:ObjectProperty ;
        rdfs:label    "Public Key"@en ;
        rdfs:domain   ids:InfrastructureComponent ;
        rdfs:range    ids:PublicKey ;
        rdfs:comment  "Public Key that has been created for the Component."@en .
@prefix owl:   <http://www.w3.org/2002/07/owl#> .
@prefix rdfs:  <http://www.w3.org/2000/01/rdf-schema#> .
@prefix ids:   <https://w3id.org/idsa/core/> .
@prefix dct:   <http://purl.org/dc/terms/> .

ids:ParIS  rdf:type      owl:Class ;
        rdfs:subClassOf  ids:Connector ;
        rdfs:label       "Participant Information Service"@en ;
        rdfs:comment     "The Participant Information Service (ParIS) provides metadata and relevant information about participants (humans and organizations) in the International Data Spaces."@en .

ids:participantCatalog
        rdf:type      owl:ObjectProperty ;
        rdfs:domain   ids:ParIS ;
        rdfs:range    ids:ParticipantCatalog ;
        rdfs:label    "participant catalog"@en ;
        rdfs:comment  "List of participants a ParIS may expose."@en .
@prefix owl:   <http://www.w3.org/2002/07/owl#> .
@prefix rdfs:  <http://www.w3.org/2000/01/rdf-schema#> .
@prefix ids:   <https://w3id.org/idsa/core/> .
@prefix xsd:   <http://www.w3.org/2001/XMLSchema#> .

ids:PublicKey  rdf:type  owl:Class ;
        rdfs:label    "Public Key"@en ;
        rdfs:comment  "Public key as used in asymmetric cryptography."@en .

ids:KeyType  rdf:type  owl:Class ;
        rdfs:label    "Key Type"@en ;
        rdfs:comment  "Cryptographic Key Type."@en .

ids:keyType  rdf:type  owl:ObjectProperty ;
        rdfs:domain   ids:PublicKey ;
        rdfs:range    ids:KeyType ;
        rdfs:label    "Key Type"@en ;
        rdfs:comment  "Type of the public key."@en .

ids:keyValue  rdf:type  owl:DatatypeProperty ;
        rdfs:label    "Key Value"@en ;
        rdfs:comment  "Binary representation of the key."@en ;
        rdfs:domain   ids:PublicKey ;
        rdfs:range    xsd:base64Binary .
@prefix owl:   <http://www.w3.org/2002/07/owl#> .
@prefix rdfs:  <http://www.w3.org/2000/01/rdf-schema#> .
@prefix xsd:   <http://www.w3.org/2001/XMLSchema#> .
@prefix ids:   <https://w3id.org/idsa/core/> .

ids:ConnectorDeployMode
        rdf:type      owl:Class ;
        rdfs:label    "Connector Deploy Mode"@en ;
        rdfs:comment  "Deploy mode of a Connector. Used mainly to capture a Connectors deployment type in the Configuration Model."@en .
@prefix owl:   <http://www.w3.org/2002/07/owl#> .
@prefix rdfs:  <http://www.w3.org/2000/01/rdf-schema#> .
@prefix xsd:   <http://www.w3.org/2001/XMLSchema#> .
@prefix ids:   <https://w3id.org/idsa/core/> .

ids:ConnectorStatus  rdf:type  owl:Class ;
        rdfs:label    "Connector Status"@en ;
        rdfs:comment  "Connector Status is used to represent a Connectors current state inside the Configuration Model."@en .
@prefix owl:   <http://www.w3.org/2002/07/owl#> .
@prefix rdfs:  <http://www.w3.org/2000/01/rdf-schema#> .
@prefix ids:   <https://w3id.org/idsa/core/> .

ids:LogLevel  rdf:type  owl:Class ;
        rdfs:label    "Log Level"@en ;
        rdfs:comment  "Instances of ids:LogLevel can be used to specify a log level. Currently this is only used by the Configuration Model."@en .
@prefix owl:   <http://www.w3.org/2002/07/owl#> .
@prefix dct:   <http://purl.org/dc/terms/> .
@prefix rdfs:  <http://www.w3.org/2000/01/rdf-schema#> .
@prefix prov:  <http://www.w3.org/ns/prov#> .
@prefix rdf:   <http://www.w3.org/1999/02/22-rdf-syntax-ns#> .
@prefix xsd:   <http://www.w3.org/2001/XMLSchema#> .
@prefix ids:   <https://w3id.org/idsa/core/> .

ids:ManagedEntity  rdf:type  owl:Class ;
        rdfs:subClassOf  ids:Described ;
        rdfs:label       "Managed entity"@en ;
        rdfs:comment     "The class of mutable individuals."@en .
@prefix owl:   <http://www.w3.org/2002/07/owl#> .
@prefix rdfs:  <http://www.w3.org/2000/01/rdf-schema#> .
@prefix dct:   <http://purl.org/dc/terms/> .
@prefix xsd:   <http://www.w3.org/2001/XMLSchema#> .
@prefix ids:   <https://w3id.org/idsa/core/> .
@prefix idsc:  <https://w3id.org/idsa/code/> .
@prefix skos:  <http://www.w3.org/2004/02/skos/core#> .
@prefix odrl:  <http://www.w3.org/ns/odrl/2/> .

idsc:ANONYMIZE  rdf:type  odrl:Action ;
        rdfs:comment     "To anonymize all, parts or certain attributes of the resource."@en ;
        rdfs:label       "anonymize"@en ;
        skos:broader     odrl:anonymize ;
        odrl:includedIn  idsc:USE ;
        skos:note        "This action is always evaluated at the provider side."@en .

idsc:AGGREGATE_BY_CONSUMER
        rdf:type         odrl:Action ;
        rdfs:comment     "Data will be part of another piece of data so that it is not distinguishable anymore."@en ;
        rdfs:label       "aggregate by consumer"@en ;
        skos:broader     odrl:aggregate ;
        odrl:includedIn  idsc:USE ;
        skos:note        "This action is always evaluated at the consumer side."@en .

idsc:AGGREGATE_BY_PROVIDER
        rdf:type         odrl:Action ;
        rdfs:comment     "Data will be part of another piece of data so that it is not distinguishable anymore."@en ;
        rdfs:label       "aggregate by provider"@en ;
        skos:broader     odrl:aggregate ;
        odrl:includedIn  idsc:AGGREGATE_BY_CONSUMER ;
        skos:note        "This action is always evaluated at the provider side."@en .

idsc:ADD  rdf:type    odrl:Action ;
        rdfs:comment  "This action modifies a number by adding a given value to it."@en ;
        rdfs:label    "add"@en ;
        skos:note     "This action modifies a number by adding a given value to it. The field to be modified and the given value are specified in the policy as idsc:JSONPATH/idsc:XPATH and idsc:OPERAND, respectively."@en .

idsc:COMPENSATE  rdf:type  odrl:Action ;
        rdfs:label       "compensate"@en ;
        rdfs:comment     "To pay a certain amount of money in order to use a resource."@en ;
        skos:broader     odrl:compensate ;
        odrl:includedIn  idsc:USE ;
        skos:note        "This action must be evaluated both at the consumer and provider side. A compensation might be required before access is granted (provider-side), or each time the usage action is performed (consumer-side)."@en .

idsc:DIVIDE  rdf:type  odrl:Action ;
        rdfs:comment  "This action modifies dividing something by something else."@en ;
        rdfs:label    "divide"@en ;
        skos:note     "This action modifies dividing something by something else. The field to be modified and the given value are specified in the policy as idsc:JSONPATH/idsc:XPATH and idsc:OPERAND, respectively."@en .

idsc:DELETE  rdf:type    odrl:Action ;
        rdfs:label       "delete"@en ;
        rdfs:comment     "To remove a resource or inhibit any further access with reasonable measures."@en ;
        skos:broader     odrl:delete ;
        odrl:includedIn  idsc:WRITE ;
        skos:note        "This action is evaluated at the consumer side if used in a duty clause. A provider cannot be forced to delete its data resources. If used in a permission clause, it is effecting the data provider as it allows the consumer to delete the provider's resource remotely."@en .

idsc:DISTRIBUTE  rdf:type  odrl:Action ;
        rdfs:label       "distribute"@en ;
        rdfs:comment     "To forward or supply a resource to a third-party."@en ;
        skos:broader     odrl:distribute ;
        odrl:includedIn  idsc:USE ;
        skos:note        "This action is always evaluated at the consumer side and allows it to become a data provider of this resource."@en .

idsc:GRANT_USE  rdf:type  odrl:Action ;
        rdfs:label       "grant use"@en ;
        rdfs:comment     "To grant use of a resource to another party. Does *not* imply any other usage rights."@en ;
        skos:broader     odrl:grantUse ;
        odrl:includedIn  idsc:USE ;
        skos:note        "This action is always evaluated at the consumer side, at the moment a third party intends to access the resource as received by the original consumer."@en .

idsc:HASH  rdf:type   odrl:Action ;
        rdfs:comment  "This action modifies a value by replacing it with a hash of the value."@en ;
        rdfs:label    "hash"@en ;
        skos:note     "This action modifies a value by replacing it with a hash of the value. The field to be modified and the hash algorithm are specified in the policy as idsc:JSONPATH/idsc:XPATH and idsc:HASH_ALGORITHM (eg. SHA256), respectively."@en .

idsc:INCREMENT_COUNTER
        rdf:type      odrl:Action ;
        rdfs:label    "increment counter"@en ;
        rdfs:comment  "An action to be used in the count usage policy where the idsc:COUNT left operand is used."@en .

idsc:ENCRYPT  rdf:type   odrl:Action ;
        rdfs:comment     "The data artifact or parts of it are encrypted and can not be read by neither the ids:DataConsumer nor any other third party. The encryption algorithm might be specified by a constraint."@en ;
        rdfs:label       "encrypt"@en ;
        odrl:includedIn  idsc:USE ;
        skos:note        "This action is always evaluated at the provider side."@en .

idsc:LOG  rdf:type       odrl:Action ;
        rdfs:comment     "To log information or store information about incidents in a local file or database. Is not necessarily available to external parties but can be used to create transparency on happened events."@en ;
        rdfs:label       "log"@en ;
        odrl:includedIn  idsc:USE ;
        skos:note        "This action is always evaluated at the consumer side."@en .

idsc:MODIFY  rdf:type    odrl:Action ;
        rdfs:comment     "To change a resource locally."@en ;
        rdfs:label       "modify"@en ;
        skos:broader     odrl:modify ;
        odrl:includedIn  idsc:WRITE ;
        skos:note        "This action is always evaluated at the consumer side. It corresponds to 'allow changes of the copied resource'."@en .

idsc:MULTIPLY  rdf:type  odrl:Action ;
        rdfs:comment  "This action modifies a number by multiplying it to a given value."@en ;
        rdfs:label    "multiply"@en ;
        skos:note     "This action modifies a number by multiplying it to a given value. The field to be modified and the given value are specified in the policy as idsc:JSONPATH/idsc:XPATH and idsc:OPERAND, respectively."@en .

idsc:NEXT_POLICY  rdf:type  odrl:Action ;
        rdfs:comment     "To forward the resource under the same policy. Implies a permission to distribute."@en ;
        rdfs:label       "next policy"@en ;
        skos:broader     odrl:nextPolicy ;
        odrl:includedIn  idsc:DISTRIBUTE ;
        skos:note        "This action is always evaluated at the consumer side."@en .

idsc:NOTIFY  rdf:type    odrl:Action ;
        rdfs:comment     "To log information or notify an instance about incidents. Can be used to define Clearing House interactions."@en ;
        rdfs:label       "notify"@en ;
        skos:broader     odrl:inform ;
        odrl:includedIn  idsc:LOG ;
        skos:note        "This action can target the consumer and the data provider of the resource."@en .

idsc:READ  rdf:type      odrl:Action ;
        rdfs:comment     "To obtain data from the resource."@en ;
        rdfs:label       "read"@en ;
        skos:broader     odrl:read ;
        odrl:includedIn  idsc:MODIFY ;
        skos:note        "This action is always evaluated at the provider side. It corresponds to 'give access to a resource'."@en .

idsc:REPLACE  rdf:type  odrl:Action ;
        rdfs:comment  "To replace some value."@en ;
        rdfs:label    "replace"@en ;
        skos:note     "This action modifies a value by replacing it with a given value. The field to be modified and the given value are specified in the policy as idsc:JSONPATH/idsc:XPATH and idsc:REPLACE_WITH, respectively."@en .

idsc:SHUFFLE  rdf:type  odrl:Action ;
        rdfs:comment  "This action modifies a value by replacing it with an anagram of the value."@en ;
        rdfs:label    "shuffle"@en ;
        skos:note     "This action modifies a value by replacing it with an anagram of the value. The field to be modified is specified in the policy as idsc:JSONPATH/idsc:XPATH."@en .

idsc:TRACK_PROVENANCE
        rdf:type         odrl:Action ;
        rdfs:comment     "To accept that the use of the Asset may be tracked."@en ;
        rdfs:label       "track provenance"@en ;
        odrl:includedIn  idsc:NOTIFY ;
        skos:note        "This action is always evaluated at the consumer side."@en .

idsc:USE  rdf:type    odrl:Action ;
        rdfs:label    "use"@en ;
        rdfs:comment  "To use a resource in any possible way. Includes all other actions."@en ;
        skos:broader  odrl:use ;
        skos:note     "This action is always evaluated at the consumer side."@en .

idsc:WRITE  rdf:type     odrl:Action ;
        rdfs:comment     "To change a remote resource."@en ;
        rdfs:label       "write"@en ;
        odrl:includedIn  idsc:USE ;
        skos:note        "This action is always evaluated at the provider side. It corresponds to 'allow changes of a resource' but *not* including its deletion."@en .
@prefix owl:   <http://www.w3.org/2002/07/owl#> .
@prefix rdfs:  <http://www.w3.org/2000/01/rdf-schema#> .
@prefix ids:   <https://w3id.org/idsa/core/> .
@prefix idsc:  <https://w3id.org/idsa/code/> .

idsc:INPUT_ENDPOINT  rdf:type  ids:AppEndpointType ;
        rdfs:label    "Input endpoint"@en ;
        rdfs:comment  "Endpoint is used for data input."@en .

idsc:OUTPUT_ENDPOINT  rdf:type  ids:AppEndpointType ;
        rdfs:label    "Output endpoint"@en ;
        rdfs:comment  "Endpoint is used for data output."@en .

idsc:STATUS_ENDPOINT  rdf:type  ids:AppEndpointType ;
        rdfs:label    "Status endpoint"@en ;
        rdfs:comment  "Endpoint is used to get app health / lifecycle status."@en .

idsc:CONFIG_ENDPOINT  rdf:type  ids:AppEndpointType ;
        rdfs:label    "Config endpoint"@en ;
        rdfs:comment  "Endpoint is used for runtime-related app configurations and app parameters."@en .

idsc:PROCESS_ENDPOINT
        rdf:type      ids:AppEndpointType ;
        rdfs:label    "Process endpoint"@en ;
        rdfs:comment  "Endpoint is used to start (or control) app processing."@en .

idsc:USAGE_POLICY_ENDPOINT
        rdf:type      ids:AppEndpointType ;
        rdfs:label    "Usage policy endpoint"@en ;
        rdfs:comment  "Endpoint is used for usage policy / usage control related scenarios."@en .

idsc:SELF_DESCRIPTION_ENDPOINT
        rdf:type      ids:AppEndpointType ;
        rdfs:label    "Self-description endpoint"@en ;
        rdfs:comment  "Pre-defined endpoint used to return the corresponding self-description of the data app."@en .
@prefix owl:   <http://www.w3.org/2002/07/owl#> .
@prefix rdfs:  <http://www.w3.org/2000/01/rdf-schema#> .
@prefix skos:  <http://www.w3.org/2004/02/skos/core#> .
@prefix dct:   <http://purl.org/dc/terms/> .
@prefix xsd:   <http://www.w3.org/2001/XMLSchema#> .
@prefix geo:   <http://www.opengis.net/ont/geosparql#> .
@prefix wgs84: <https://www.w3.org/2003/01/geo/wgs84_pos#> .
@prefix odrl:  <http://www.w3.org/ns/odrl/2/> .
@prefix time:  <http://www.w3.org/2006/time#> .
@prefix org:   <http://www.w3.org/ns/org#> .
@prefix ids:   <https://w3id.org/idsa/core/> .
@prefix idsc:  <https://w3id.org/idsa/code/> .

idsc:ANONYMIZED  rdf:type  ids:ArtifactState ;
        rdfs:label    "is anonymized"@en ;
        rdfs:comment  "The artifact is anonymized so the data source can not be recognized by any further user."@en .

idsc:PSEUDONYMIZED  rdf:type  ids:ArtifactState ;
        rdfs:label    "is pseudonymized"@en ;
        rdfs:comment  "The artifact is pseudo pseudonymized."@en .

idsc:ENCRYPTED  rdf:type  ids:ArtifactState ;
        rdfs:label    "is encrypted"@en ;
        rdfs:comment  "The artifact is encrypted so the data itself cannot be read by any user without having the corresponding key."@en .

idsc:COMBINED  rdf:type  ids:ArtifactState ;
        rdfs:label    "is combined"@en ;
        rdfs:comment  "The artifact is a collection of smaller artifacts and can be split into parts when necessary."@en .
@prefix rdfs:  <http://www.w3.org/2000/01/rdf-schema#> .
@prefix owl:   <http://www.w3.org/2002/07/owl#> .
@prefix ids:   <https://w3id.org/idsa/core/> .
@prefix idsc:  <https://w3id.org/idsa/code/> .

idsc:IDS_CONNECTOR_ATTRIBUTES_ALL
        rdf:type      ids:Audience ;
        rdfs:label    "all IDS Connectors" ;
        rdfs:comment  "Every IDS Connector is in the intended audience for the DAT with this 'scope' property."@en .
@prefix owl:   <http://www.w3.org/2002/07/owl#> .
@prefix rdfs:  <http://www.w3.org/2000/01/rdf-schema#> .
@prefix skos:  <http://www.w3.org/2004/02/skos/core#> .
@prefix dct:   <http://purl.org/dc/terms/> .
@prefix xsd:   <http://www.w3.org/2001/XMLSchema#> .
@prefix geo:   <http://www.opengis.net/ont/geosparql#> .
@prefix wgs84: <https://www.w3.org/2003/01/geo/wgs84_pos#> .
@prefix odrl:  <http://www.w3.org/ns/odrl/2/> .
@prefix time:  <http://www.w3.org/2006/time#> .
@prefix org:   <http://www.w3.org/ns/org#> .
@prefix ids:   <https://w3id.org/idsa/core/> .
@prefix idsc:  <https://w3id.org/idsa/code/> .

idsc:EQUALS  rdf:type  ids:BinaryOperator ;
        skos:broader  odrl:eq ;
        rdfs:label    "equals"@en ;
        rdfs:comment  "Logical equals operator (true = true)."@en .

idsc:SAME_AS  rdf:type  ids:BinaryOperator ;
        rdfs:seeAlso  owl:sameAs ;
        rdfs:label    "is same as"@en ;
        rdfs:comment  "Logical equals operator comparing two RDF URIs. Is true if at least one owl:sameAs relation exists."@en ;
        skos:note     "A owl:sameAs A is always true."@en .

idsc:NOT  rdf:type    ids:BinaryOperator ;
        skos:broader  odrl:neq ;
        rdfs:label    "not equals"@en ;
        rdfs:comment  "Logical difference operator (false != true)."@en .

idsc:HAS_STATE  rdf:type  ids:BinaryOperator ;
        rdfs:label    "has state"@en ;
        rdfs:comment  "Operator examining if the target resource has a certain state at the moment, for instance is anonymized (idsc:ANONYMIZED)."@en .

idsc:GTEQ  rdf:type   ids:BinaryOperator ;
        skos:broader  odrl:gteq ;
        rdfs:label    "greater than or equals"@en ;
        rdfs:comment  "Greater-than-or-equals operator. Can be used for numeric (5 idsc:GTEQ 2) comparisons."@en .

idsc:GT  rdf:type     ids:BinaryOperator ;
        skos:broader  odrl:gt ;
        rdfs:label    "greater than"@en ;
        rdfs:comment  "Greater-than operator. Can be used for numeric (5 idsc:GT 2) comparisons."@en .

idsc:EQ  rdf:type     ids:BinaryOperator ;
        skos:broader  odrl:eq ;
        rdfs:label    "equals"@en ;
        rdfs:comment  "Arithmetic equals operator (5 = 5)."@en .

idsc:LTEQ  rdf:type   ids:BinaryOperator ;
        skos:broader  odrl:lteq ;
        rdfs:label    "less than or equals"@en ;
        rdfs:comment  "Less-than-or-equals operator. Can be used for numeric (2 idsc:LTEQ 5) comparisons."@en .

idsc:LT  rdf:type     ids:BinaryOperator ;
        skos:broader  odrl:lt ;
        rdfs:label    "less than"@en ;
        rdfs:comment  "Less-than operator. Can be used for numeric (2 idsc:LT 5) comparisons."@en ;
        skos:note     "Do not confuse with idsc:LT (which is a language)."@en .

idsc:IN  rdf:type     ids:BinaryOperator ;
        skos:broader  odrl:isAnyOf ;
        skos:broader  <https://postgis.net/docs/ST_Within.html> ;
        rdfs:label    "in"@en ;
        rdfs:comment  "Element-of operator. Allowed RightOperands are RDF collections('(A B C)')."@en .

idsc:STRING_EQ  rdf:type  ids:BinaryOperator ;
        rdfs:label    "string equals"@en ;
        rdfs:comment  "Equals operator for strings. Evaluates to true iff all characters and their sequence is the same."@en .

idsc:STRING_CONTAINS  rdf:type  ids:BinaryOperator ;
        rdfs:label    "string contains"@en ;
        rdfs:comment  "Contains operator for strings. Evaluates to true iff the LeftOperand contains the complete RightOperand."@en .

idsc:STRING_IS_CONTAINED
        rdf:type      ids:BinaryOperator ;
        rdfs:label    "string is contained in"@en ;
        rdfs:comment  "Contained in operator for strings. Evaluates to true iff the LeftOperand is contained completely by the RightOperand."@en .

idsc:MATCHES  rdf:type  ids:BinaryOperator ;
        rdfs:label    "matches"@en ;
        rdfs:comment  "Regex operator for strings. Evaluates to true iff the regex pattern of the RightOperand matches the LeftOperand."@en .

idsc:AFTER  rdf:type  ids:BinaryOperator ;
        rdfs:seeAlso  time:after ;
        rdfs:label    "after"@en ;
        rdfs:comment  "If a temporal entity T1 is after another temporal entity T2, then the beginning of T1 is after the end of T2 and the beginning of T1 is different to the ending of T2. Temporal entities can either be a xsd:dateTimeStamp or a time:TemporalEntity."@en .

idsc:BEFORE  rdf:type  ids:BinaryOperator ;
        rdfs:seeAlso  time:before ;
        rdfs:label    "before"@en ;
        skos:note     "Compares an instance of time:TemporalEntity or a Literal of xsd:dateTimeStamp to an instance of time:TemporalEntity or a Literal of xsd:dateTimeStamp."@en ;
        rdfs:comment  "If a temporal entity T1 is before another temporal entity T2, then the ending of T1 is before the end of T2 and the ending of T1 is different to the beginning of T2. Temporal entities can either be a xsd:dateTimeStamp or a time:TemporalEntity."@en .

idsc:CONTAINS  rdf:type  ids:BinaryOperator ;
        rdfs:seeAlso  time:inside ;
        rdfs:seeAlso  time:intervalContains ;
        rdfs:label    "contains"@en ;
        rdfs:comment  "If a TemporalEntity (or xsd:dateTimeStamp) T1 contains another time:TemporalEntity T2, then the beginning of T1 is idsc:AFTER the beginning of T2 and the ending of T1 is idsc:BEFORE the ending of T2. An Instant (or xsd:dateTimeStamp) cannot contain another Instant (or xsd:dateTimeStamp), neihter contains itself."@en ;
        skos:note     "Compares an instance of time:Instant, time:Interval or xsd:dateTimeStamp with an instance of time:Interval. Evaluates to false if compared to a non time:Interval."@en .

idsc:TEMPORAL_DISJOINT
        rdf:type      ids:BinaryOperator ;
        rdfs:seeAlso  time:intervalDisjoint ;
        rdfs:label    "disjoint"@en ;
        rdfs:comment  "If a TemporalEntity (or xsd:dateTimeStamp) T1 is disjoint with another time:TemporalEntity (or xsd:dateTimeStamp) T2, then T1 is idsc:BEFORE or idsc:AFTER to T2."@en ;
        skos:note     "Compares an instance of time:TemporalEntity or xsd:dateTimeStamp Literal to an instance of time:TemporalEntity or xsd:dateTimeStamp Literal."@en .

idsc:DURING  rdf:type  ids:BinaryOperator ;
        rdfs:seeAlso  time:intervalDuring ;
        rdfs:label    "during"@en ;
        rdfs:comment  "If a TemporalEntity T1 is during another TemporalEntity T2, then the beginning of T1 is after the beginning of T2, and the end of T1 is before the end of T2."@en ;
        skos:note     "Compares an instance of time:Instant, time:Interval or xsd:dateTimeStamp with an instance of time:Interval. Evaluates to false if compared to a non time:Interval."@en .

idsc:TEMPORAL_EQUALS  rdf:type  ids:BinaryOperator ;
        rdfs:seeAlso  time:intervalEquals ;
        rdfs:label    "interval equals"@en ;
        rdfs:comment  "If a TemporalEntity (or xsd:dateTimeStamp Literal) T1 is equals another TemporalEntity (or xsd:dateTimeStamp Literal) T2, then the beginning of T1 is coincident with the beginning of T2, and the end of T1 is coincident with the end of T2. The beginning and ending is the same for instances of time:Instant (or xsd:dateTimeStamp Literal)."@en ;
        skos:note     "Compares an instance of TemporalEntity or xsd:dateTimeStamp Literal to another TemporalEntity or xsd:dateTimeStamp. Evaluates to false if a DurationEntity is involved."@en .

idsc:FINISHED_BY  rdf:type  ids:BinaryOperator ;
        rdfs:seeAlso  time:intervalFinishedBy ;
        rdfs:label    "finished by"@en ;
        rdfs:comment  "If an interval T1 is finished by another interval T2, then the beginning of T1 is before the beginning of T2, and the end of T1 is coincident with the end of T2."@en ;
        skos:note     "Compares an instance of time:Interval to another instance of time:Interval. Evaluates to false if compared to a non time:Interval or one interval is empty."@en .

idsc:FINISHES  rdf:type  ids:BinaryOperator ;
        rdfs:seeAlso  time:intervalFinishes ;
        rdfs:seeAlso  ids:intervalIn ;
        rdfs:label    "finishes"@en ;
        rdfs:comment  "If an Interval T1 finishes another interval T2, then the beginning of T1 is after the beginning of T2, and the end of T1 is coincident with the end of T2."@en ;
        skos:note     "Compares an instance of time:Interval to another instance of time:Interval. Evaluates to false if compared to a non time:Interval or one interval is empty."@en .

idsc:MEETS  rdf:type  ids:BinaryOperator ;
        rdfs:seeAlso  time:intervalMeets ;
        rdfs:label    "meets"@en ;
        rdfs:comment  "If a TemporalEntity or (xsd:dateTimeStamp Literal) T1 meets another TemporalEntity (or xsd:dateTimeStamp Literal) T2, then the end of T1 is coincident with the beginning of T2."@en ;
        skos:note     "Compares an instance of TemporalEntity or xsd:dateTimeStamp Literal to another instance of TemporalEntity or xsd:dateTimeStamp Literal. Evaluates to true if T1 or T2 are Instants (or xsd:dateTimeStamp Literal) and the condition in the comment holds."@en .

idsc:MET_BY  rdf:type  ids:BinaryOperator ;
        rdfs:seeAlso  time:intervalMetBy ;
        rdfs:label    "met by"@en ;
        rdfs:comment  "If a TemporalEntity or (xsd:dateTimeStamp Literal) T1 is met by another TemporalEntity or (xsd:dateTimeStamp Literal) T2, then the beginning of T1 is coincident with the end of T2."@en ;
        skos:note     "Compares an instance of TemporalEntity (or xsd:dateTimeStamp Literal) to another instance of TemporalEntity (or xsd:dateTimeStamp Literal). Evaluates to true if T1 or T2 are Instants (or xsd:dateTimeStamp Literal) and the condition in the comment holds."@en .

idsc:OVERLAPS  rdf:type  ids:BinaryOperator ;
        rdfs:seeAlso  time:intervalOverlaps ;
        rdfs:label    "overlaps"@en ;
        rdfs:comment  "If a time:Interval T1 overlapps another time:Interval T2, then the beginning of T1 is after the beginning of T2, the beginning of T1 is before the end of T2, and the end of T1 is after the end of T2."@en ;
        skos:note     "Compares an instance of time:Interval to another instance of time:Interval. Evaluates to false if compared to a non time:Interval or one interval is empty."@en .

idsc:OVERLAPPED_BY  rdf:type  ids:BinaryOperator ;
        rdfs:seeAlso  time:intervalOverlappedBy ;
        rdfs:label    "overlapped by"@en ;
        rdfs:comment  "If a interval T1 is overlapped another proper interval T2, then the beginning of T1 is before the beginning of T2, the end of T1 is after the beginning of T2, and the end of T1 is before the end of T2."@en ;
        skos:note     "Compares an instance of time:Interval to another instance of time:Interval. Evaluates to false if compared to a non time:Interval or one interval is empty."@en .

idsc:STARTS  rdf:type  ids:BinaryOperator ;
        rdfs:seeAlso  time:intervalStarts ;
        rdfs:label    "starts"@en ;
        rdfs:comment  "If an interval T1 starts with a TemporalEntity T2, then the beginning of T1 is coincident with the beginning of T2, and the end of T1 is before the end of T2."@en ;
        skos:note     "Compares an instance of time:Interval to another instance of TemporalEntity (or xsd:dateTimeStamp Literal). Evaluates to false if T2 is not a time:Interval as then the end of T1 can never be idsc:BEFORE the end of T2"@en .

idsc:STARTED_BY  rdf:type  ids:BinaryOperator ;
        rdfs:seeAlso  time:intervalStartedBy ;
        rdfs:label    "started by"@en ;
        rdfs:comment  "If a TemporalEntity T1 is started by another proper interval T2, then the beginning of T1 is coincident with the beginning of T2, and the end of T1 is after the end of T2."@en ;
        skos:note     "Compares an instance of TemporalEntity (or xsd:dateTimeStamp Literal) to instance of time:Interval. Evaluates to false if T1 is an Instant (or xsd:dateTimeStamp Literal) as the end of T1 can then not be idsc:AFTER the end of T2."@en .

idsc:DURATION_EQ  rdf:type  ids:BinaryOperator ;
        rdfs:seeAlso  time:hasTemporalDuration ;
        rdfs:label    "has same duration"@en ;
        rdfs:comment  "If a temporal entity T1 has the same duration as another temporal entity T2, then their length or their duration is equal. Instants and xsd:dateTimeStamp Literals have always the duration 'P0Y0M0DT0H0M0S'^^xsd:duration and therefore have always the same duration."@en ;
        skos:note     "Compares an instance of time:TemporalEntity with an instance of time:TemporalEntity."@en .

idsc:LONGER  rdf:type  ids:BinaryOperator ;
        rdfs:label    "longer"@en ;
        rdfs:comment  "If a temporal entity T1 is longer than another temporal entity T2, then the length or duration of T1 is bigger. Instants and xsd:dateTimeStamp Literals have always the duration 'P0Y0M0DT0H0M0S'^^xsd:duration and therefore have always the same duration."@en ;
        skos:note     "Compares an instance of time:TemporalEntity with an instance of xsd:duration."@en .

idsc:LONGER_EQ  rdf:type  ids:BinaryOperator ;
        rdfs:label    "longer or equals"@en ;
        rdfs:comment  "If temporal entity T1 is longer or equals than another temporal entity T2, then the length or duration of T1 is bigger or their length or their duration is equal. Instants and xsd:dateTimeStamp Literals have always the duration 'P0Y0M0DT0H0M0S'^^xsd:duration and therefore have always the same duration."@en ;
        skos:note     "Compares an instance of time:TemporalEntity with an instance of xsd:duration."@en .

idsc:SHORTER_EQ  rdf:type  ids:BinaryOperator ;
        rdfs:label    "shorter or equals"@en ;
        rdfs:comment  "If a temporal entity T1 is shorter or equals than another temporal entity T2, then the length or duration of T1 is shorter or their length or their duration is equal. Instants and xsd:dateTimeStamp Literals have always the duration 'P0Y0M0DT0H0M0S'^^xsd:duration and therefore have always the same duration."@en ;
        skos:note     "Compares an instance of time:TemporalEntity with an instance of xsd:duration."@en .

idsc:SHORTER  rdf:type  ids:BinaryOperator ;
        rdfs:label    "shorter"@en ;
        rdfs:comment  "If a temporal entity T1 is shorter than another temporal entity T2, then the length or duration of T1 is shorter. Instants and xsd:dateTimeStamp Literals have always the duration 'P0Y0M0DT0H0M0S'^^xsd:duration and therefore have always the same duration."@en ;
        skos:note     "Compares an instance of time:TemporalEntity with an instance of xsd:duration."@en .

idsc:COVERED_BY  rdf:type  ids:BinaryOperator ;
        rdfs:seeAlso  geo:ehCoveredBy ;
        rdfs:comment  "Spatial operator 'covered by' as defined by the Egenhofer Topological Relations family: An object A is covered_by another object B if both objects share common bounding and interior faces; if A has interior faces which are bounding faces of B; and if none of B's interior faces are part of A's boundary. (https://doi.org/10.1007/3-540-51295-0_148 Definition 7)"@en ;
        rdfs:label    "covered by"@en .

idsc:COVERS  rdf:type  ids:BinaryOperator ;
        rdfs:seeAlso  geo:ehCovers ;
        rdfs:comment  "Spatial operator 'covers' as defined by the Egenhofer Topological Relations family: An object A covers another object B if both objects share common bounding and interior faces; if B has interior faces which are bounding faces of A; and if none of A's interior faces are part of B's boundary. (https://doi.org/10.1007/3-540-51295-0_148 Definition 6)"@en ;
        rdfs:label    "covers"@en .

idsc:INSIDE  rdf:type  ids:BinaryOperator ;
        rdfs:seeAlso  geo:ehInside ;
        rdfs:comment  "Spatial operator 'inside' as defined by the Egenhofer Topological Relations family: An object A is inside of another object B if (1) A and B share interior, but not bounding faces, (2) if A has bounding faces which are interior faces of B, and (3) none of B's bounding faces coincides with any of A's interior faces. (https://doi.org/10.1007/3-540-51295-0_148 Definition 4)"@en ;
        skos:note     "In addition, a point is inside a polygom iff the point is in the polygom's interior (the point itself has no interior)."@en ;
        rdfs:label    "inside"@en .

idsc:SPATIAL_CONTAINS
        rdf:type      ids:BinaryOperator ;
        rdfs:seeAlso  geo:ehContains ;
        rdfs:comment  "Spatial operator 'contains' as defined by the Egenhofer Topological Relations family: An object A contains another object B if A and B share interior but no bounding faces; if B has bounding faces which are interior faces of , and none of A's bounding faces coincides with any of B's interior faces. (https://doi.org/10.1007/3-540-51295-0_148 Definition 5)"@en ;
        skos:note     "In addition, a polygom contains a point iff the point is in the polygom's interior (the point itself has no interior)."@en ;
        rdfs:label    "contains"@en .

idsc:SPATIAL_EQUALS  rdf:type  ids:BinaryOperator ;
        rdfs:seeAlso  geo:ehEquals ;
        rdfs:comment  "Spatial operator 'equals' as defined by the Egenhofer Topological Relations family: Two objects are equal if both intersections of bounding and interior faces are not empty while the two boundary-interior intersections are empty. (https://doi.org/10.1007/3-540-51295-0_148 Definition 3)"@en ;
        skos:note     "In addition, two spatial points are equal iff both coordinates are equal (points have no interior)."@en ;
        rdfs:label    "equals"@en .

idsc:SPATIAL_OVERLAP  rdf:type  ids:BinaryOperator ;
        rdfs:seeAlso  geo:ehOverlap ;
        rdfs:comment  "Spatial operator 'overlap' as defined by the Egenhofer Topological Relations family: Two objects overlap if they have common interior faces and the bounding faces have common parts with the opposite interior faces. (https://doi.org/10.1007/3-540-51295-0_148 Definition 8)"@en ;
        rdfs:label    "overlap"@en .

idsc:SPATIAL_MEET  rdf:type  ids:BinaryOperator ;
        rdfs:seeAlso  geo:ehMeet ;
        rdfs:comment  "Spatial operator 'meet' as defined by the Egenhofer Topological Relations family: If the intersection among the bounding faces is not empty, whereas all other 3 intersections are empty, then the two objects meet. (https://doi.org/10.1007/3-540-51295-0_148 Definition 2)"@en ;
        rdfs:label    "meet"@en .

idsc:DISJOINT  rdf:type  ids:BinaryOperator ;
        rdfs:seeAlso  geo:ehDisjoint ;
        rdfs:comment  "Spatial operator 'disjoint' as defined by the Egenhofer Topological Relations family: If all four intersections among all object parts are empty, then the two objects are disjoint. (https://doi.org/10.1007/3-540-51295-0_148 Definition 1)"@en ;
        rdfs:label    "disjoint"@en .

idsc:MEMBER_OF  rdf:type  ids:BinaryOperator ;
        rdfs:seeAlso  org:memberOf ;
        rdfs:label    "memberOf"@en ;
        rdfs:comment  "If a user is part of a certain organisation required for accessing a resource. Should be used together with a RightOperand pointing to an accessible endpoint providing this information."@en .

idsc:HAS_MEMBERSHIP  rdf:type  ids:BinaryOperator ;
        rdfs:seeAlso  org:hasMember ;
        rdfs:label    "has Member"@en ;
        rdfs:comment  "If a user has a specific membership required for accessing a resource. A membership includes always a role and a related organisation (see also org:). Should be used together with a RightOperand pointing to an accessible endpoint providing this information."@en .

idsc:HAS_SITE  rdf:type  ids:BinaryOperator ;
        rdfs:seeAlso  org:basedAt ;
        rdfs:label    "has site"@en ;
        rdfs:comment  "If a user needs to be located at a certain site required for accessing a resource. A 'HAS_SITE' relation includes always a membership (role and related organisation) corresponding to the site. Should be used together with a RightOperand pointing to an accessible endpoint providing this information."@en .

idsc:INSIDE_NETWORK  rdf:type  ids:BinaryOperator ;
        rdfs:label    "inside network"@en ;
        rdfs:comment  "Is satisfied if a system is inside a specified target network or network range."@en .

idsc:DEFINES_AS  rdf:type  ids:BinaryOperator ;
        rdfs:label    "defines as"@en ;
        rdfs:comment  "Allows assignments similar to 'var x := {RightOperand}'."@en ;
        skos:note     "Different to the other ids:BinaryOperator, idsc:DEFINES_AS does *not* compare a feature but tells the interpreter where to *find* one. Therefore, the constraint is not evaluated in the same way as with other operators."@en .
@prefix owl:   <http://www.w3.org/2002/07/owl#> .
@prefix rdfs:  <http://www.w3.org/2000/01/rdf-schema#> .
@prefix dct:   <http://purl.org/dc/terms/> .
@prefix xsd:   <http://www.w3.org/2001/XMLSchema#> .
@prefix ids:   <https://w3id.org/idsa/core/> .
@prefix idsc:  <https://w3id.org/idsa/code/> .
@prefix skos:  <http://www.w3.org/2004/02/skos/core#> .

idsc:PARTICIPANT_ENTRY_LEVEL_SELF_ASSESSMENT
        rdf:type    ids:ParticipantCertificationLevel ;
        rdfs:label  "Entry Level Self-Assessment Certification of Participants"@en .

idsc:PARTICIPANT_ENTRY_LEVEL_MANAGEMENT_SYSTEM
        rdf:type                        ids:ParticipantCertificationLevel ;
        rdfs:label                      "Entry Level Management System Certification of Participants"@en ;
        ids:includedCertificationLevel  idsc:PARTICIPANT_ENTRY_LEVEL_SELF_ASSESSMENT .

idsc:PARTICIPANT_MEMBER_LEVEL_MANAGEMENT_SYSTEM
        rdf:type                        ids:ParticipantCertificationLevel ;
        rdfs:label                      "Member Level Management System Certification of Participants"@en ;
        ids:includedCertificationLevel  idsc:PARTICIPANT_MEMBER_LEVEL_MANAGEMENT_SYSTEM .

idsc:PARTICIPANT_MEMBER_LEVEL_CONTROL_FRAMEWORK
        rdf:type                        ids:ParticipantCertificationLevel ;
        rdfs:label                      "Member Level ControlFramework Certification of Participants"@en ;
        ids:includedCertificationLevel  idsc:PARTICIPANT_MEMBER_LEVEL_CONTROL_FRAMEWORK .

idsc:PARTICIPANT_CENTRAL_LEVEL_MANAGEMENT_SYSTEM
        rdf:type                        ids:ParticipantCertificationLevel ;
        rdfs:label                      "Central Level Management System Certification of Participants"@en ;
        ids:includedCertificationLevel  idsc:PARTICIPANT_MEMBER_LEVEL_MANAGEMENT_SYSTEM .

idsc:PARTICIPANT_CENTRAL_LEVEL_CONTROL_FRAMEWORK
        rdf:type                        ids:ParticipantCertificationLevel ;
        rdfs:label                      "Central Level Control Framework Certification of Participants"@en ;
        ids:includedCertificationLevel  idsc:PARTICIPANT_CENTRAL_LEVEL_MANAGEMENT_SYSTEM .

idsc:COMPONENT_BASE_SECURITY_PROFILE_CHECKLIST_APPROACH
        rdf:type    ids:ComponentCertificationLevel ;
        rdfs:label  "Base Security Profile Certification of Components based on Checklist Approach"@en .

idsc:COMPONENT_BASE_SECURITY_PROFILE_CONCEPT_REVIEW
        rdf:type                        ids:ComponentCertificationLevel ;
        rdfs:label                      "Base Security Profile Certification of Components based on Concept Review"@en ;
        ids:includedCertificationLevel  idsc:COMPONENT_BASE_SECURITY_PROFILE_CHECKLIST_APPROACH .

idsc:COMPONENT_TRUST_SECURITY_PROFILE_CONCEPT_REVIEW
        rdf:type                        ids:ComponentCertificationLevel ;
        rdfs:label                      "Trust Security Profile Certification of Components based on Concept Review"@en ;
        ids:includedCertificationLevel  idsc:COMPONENT_BASE_SECURITY_PROFILE_CONCEPT_REVIEW .

idsc:COMPONENT_TRUST_SECURITY_PROFILE_HIGH_ASSURANCE_EVALUATION
        rdf:type                        ids:ComponentCertificationLevel ;
        rdfs:label                      "Trust Security Profile Certification of Components based on High Assurance Evaluation"@en ;
        ids:includedCertificationLevel  idsc:COMPONENT_TRUST_SECURITY_PROFILE_CONCEPT_REVIEW .

idsc:COMPONENT_TRUSTPLUS_SECURITY_PROFILE_CONCEPT_REVIEW
        rdf:type                        ids:ComponentCertificationLevel ;
        rdfs:label                      "Trust-Plus Security Profile Certification of Components based on Concept Review"@en ;
        ids:includedCertificationLevel  idsc:COMPONENT_TRUST_SECURITY_PROFILE_CONCEPT_REVIEW .

idsc:COMPONENT_TRUSTPLUS_SECURITY_PROFILE_HIGH_ASSURANCE_EVALUATION
        rdf:type                        ids:ComponentCertificationLevel ;
        rdfs:label                      "Trust-Plus Security Profile Certification of Components based on High AssuranceEvaluation"@en ;
        ids:includedCertificationLevel  idsc:COMPONENT_TRUSTPLUS_SECURITY_PROFILE_CONCEPT_REVIEW .
@prefix owl:   <http://www.w3.org/2002/07/owl#> .
@prefix rdfs:  <http://www.w3.org/2000/01/rdf-schema#> .
@prefix ids:   <https://w3id.org/idsa/core/> .
@prefix idsc:  <https://w3id.org/idsa/code/> .

idsc:TEST_DEPLOYMENT  rdf:type  ids:ConnectorDeployMode ;
        rdfs:label    "Test Deployment"@en ;
        rdfs:comment  "Indicates that a Connector is deployed for testing."@en .

idsc:PRODUCTIVE_DEPLOYMENT
        rdf:type      ids:ConnectorDeployMode ;
        rdfs:label    "Productive Deployment"@en ;
        rdfs:comment  "Indicates that a Connector is deployed for productive use."@en .
@prefix owl:   <http://www.w3.org/2002/07/owl#> .
@prefix rdfs:  <http://www.w3.org/2000/01/rdf-schema#> .
@prefix ids:   <https://w3id.org/idsa/core/> .
@prefix idsc:  <https://w3id.org/idsa/code/> .

idsc:CONNECTOR_ONLINE
        rdf:type      ids:ConnectorStatus ;
        rdfs:label    "Connector Online"@en ;
        rdfs:comment  "Indicates that a Connector is online."@en .

idsc:CONNECTOR_OFFLINE
        rdf:type      ids:ConnectorStatus ;
        rdfs:label    "Connector Offline"@en ;
        rdfs:comment  "Indicates that a Connector is offline."@en .

idsc:CONNECTOR_BADLY_CONFIGURED
        rdf:type      ids:ConnectorStatus ;
        rdfs:label    "Connector badly configured"@en ;
        rdfs:comment  "Indicates that a Connector is badly configured."@en .
@prefix owl:   <http://www.w3.org/2002/07/owl#> .
@prefix rdfs:  <http://www.w3.org/2000/01/rdf-schema#> .
@prefix dct:   <http://purl.org/dc/terms/> .
@prefix ids:   <https://w3id.org/idsa/core/> .
@prefix idsc:  <https://w3id.org/idsa/code/> .
@prefix skos:  <http://www.w3.org/2004/02/skos/core#> .

idsc:INTERFACE_DEFINITION
        rdf:type      dct:DCMIType ;
        rdfs:label    "Interface definition" ;
        rdfs:comment  "Formal, machine-interpretable definition of a protocol-specific API, e.g., OpenAPI, GraphQL, API Blueprint, WSDL."@en .

idsc:SCHEMA_DEFINITION
        rdf:type      dct:DCMIType ;
        rdfs:label    "Schema definition" ;
        rdfs:comment  "Formal, machine-interpretable definition of a data schema, e.g., XMLSchema, JSONSchema"@en .
@prefix dc:    <http://purl.org/dc/terms/> .
@prefix rdfs:  <http://www.w3.org/2000/01/rdf-schema#> .
@prefix skos:  <http://www.w3.org/2004/02/skos/core#> .
@prefix dcam:  <http://purl.org/dc/dcam/> .
@prefix ids:   <https://w3id.org/idsa/core/> .
@prefix idsc:  <https://w3id.org/idsa/code/> .
@prefix owl:   <http://www.w3.org/2002/07/owl#> .

idsc:TRIENNIAL  rdf:type  ids:Frequency ;
        rdfs:label        "Triennial"@en ;
        skos:prefLabel    "Triennial"@en ;
        rdfs:comment      "The event occurs every three years."@en ;
        owl:sameAs        <http://purl.org/cld/freq/triennial> ;
        rdfs:isDefinedBy  <http://purl.org/cld/freq/> ;
        rdfs:seeAlso      <https://www.loc.gov/marc/holdings/hd853855.html> ;
        skos:inScheme     <http://purl.org/cld/terms/Frequency> ;
        dcam:memberOf     <http://purl.org/cld/terms/Frequency> .

idsc:BIENNIAL  rdf:type   ids:Frequency ;
        rdf:type          skos:Concept ;
        rdfs:label        "Biennial"@en ;
        skos:prefLabel    "Biennial"@en ;
        rdfs:comment      "The event occurs every two years."@en ;
        owl:sameAs        <http://purl.org/cld/freq/biennial> ;
        rdfs:isDefinedBy  <http://purl.org/cld/freq/> ;
        rdfs:seeAlso      <https://www.loc.gov/marc/holdings/hd853855.html> ;
        skos:inScheme     <http://purl.org/cld/terms/Frequency> ;
        dcam:memberOf     <http://purl.org/cld/terms/Frequency> .

idsc:ANNUAL  rdf:type     ids:Frequency ;
        rdf:type          skos:Concept ;
        rdfs:label        "Annual"@en ;
        skos:prefLabel    "Annual"@en ;
        rdfs:comment      "The event occurs once a year."@en ;
        owl:sameAs        <http://purl.org/cld/freq/annual> ;
        rdfs:isDefinedBy  <http://purl.org/cld/freq/> ;
        rdfs:seeAlso      <https://www.loc.gov/marc/holdings/hd853855.html> ;
        skos:inScheme     <http://purl.org/cld/terms/Frequency> ;
        dcam:memberOf     <http://purl.org/cld/terms/Frequency> .

idsc:SEMIANNUAL  rdf:type  ids:Frequency ;
        rdf:type          skos:Concept ;
        rdfs:label        "Semiannual"@en ;
        skos:prefLabel    "Semiannual"@en ;
        rdfs:comment      "The event occurs twice a year."@en ;
        owl:sameAs        <http://purl.org/cld/freq/semiannual> ;
        rdfs:isDefinedBy  <http://purl.org/cld/freq/> ;
        rdfs:seeAlso      <https://www.loc.gov/marc/holdings/hd853855.html> ;
        skos:inScheme     <http://purl.org/cld/terms/Frequency> ;
        dcam:memberOf     <http://purl.org/cld/terms/Frequency> .

idsc:THREE_TIMES_A_YEAR
        rdf:type          ids:Frequency ;
        rdf:type          skos:Concept ;
        rdfs:label        "Three times a year"@en ;
        skos:prefLabel    "Three times a year"@en ;
        rdfs:comment      "The event occurs three times a year."@en ;
        owl:sameAs        <http://purl.org/cld/freq/threeTimesAYear> ;
        rdfs:isDefinedBy  <http://purl.org/cld/freq/> ;
        rdfs:seeAlso      <https://www.loc.gov/marc/holdings/hd853855.html> ;
        skos:inScheme     <http://purl.org/cld/terms/Frequency> ;
        dcam:memberOf     <http://purl.org/cld/terms/Frequency> .

idsc:QUARTERLY  rdf:type  ids:Frequency ;
        rdf:type          skos:Concept ;
        rdfs:label        "Quarterly"@en ;
        skos:prefLabel    "Quarterly"@en ;
        rdfs:comment      "The event occurs every three months."@en ;
        owl:sameAs        <http://purl.org/cld/freq/quarterly> ;
        rdfs:isDefinedBy  <http://purl.org/cld/freq/> ;
        rdfs:seeAlso      <https://www.loc.gov/marc/holdings/hd853855.html> ;
        skos:inScheme     <http://purl.org/cld/terms/Frequency> ;
        dcam:memberOf     <http://purl.org/cld/terms/Frequency> .

idsc:BIMONTHLY  rdf:type  ids:Frequency ;
        rdf:type          skos:Concept ;
        rdfs:label        "Bimonthly"@en ;
        skos:prefLabel    "Bimonthly"@en ;
        rdfs:comment      "The event occurs every two months."@en ;
        owl:sameAs        <http://purl.org/cld/freq/bimonthly> ;
        rdfs:isDefinedBy  <http://purl.org/cld/freq/> ;
        rdfs:seeAlso      <https://www.loc.gov/marc/holdings/hd853855.html> ;
        skos:inScheme     <http://purl.org/cld/terms/Frequency> ;
        dcam:memberOf     <http://purl.org/cld/terms/Frequency> .

idsc:MONTHLY  rdf:type    ids:Frequency ;
        rdf:type          skos:Concept ;
        rdfs:label        "Monthly"@en ;
        skos:prefLabel    "Monthly"@en ;
        rdfs:comment      "The event occurs once a month."@en ;
        owl:sameAs        <http://purl.org/cld/freq/monthly> ;
        rdfs:isDefinedBy  <http://purl.org/cld/freq/> ;
        rdfs:seeAlso      <https://www.loc.gov/marc/holdings/hd853855.html> ;
        skos:inScheme     <http://purl.org/cld/terms/Frequency> ;
        dcam:memberOf     <http://purl.org/cld/terms/Frequency> .

idsc:SEMIMONTHLY  rdf:type  ids:Frequency ;
        rdf:type          skos:Concept ;
        rdfs:label        "Semimonthly"@en ;
        skos:prefLabel    "Semimonthly"@en ;
        rdfs:comment      "The event occurs twice a month."@en ;
        owl:sameAs        <http://purl.org/cld/freq/semimonthly> ;
        rdfs:isDefinedBy  <http://purl.org/cld/freq/> ;
        rdfs:seeAlso      <https://www.loc.gov/marc/holdings/hd853855.html> ;
        skos:inScheme     <http://purl.org/cld/terms/Frequency> ;
        dcam:memberOf     <http://purl.org/cld/terms/Frequency> .

idsc:BIWEEKLY  rdf:type   ids:Frequency ;
        rdf:type          skos:Concept ;
        rdfs:label        "Biweekly"@en ;
        skos:prefLabel    "Biweekly"@en ;
        rdfs:comment      "The event occurs every two weeks."@en ;
        owl:sameAs        <http://purl.org/cld/freq/biweekly> ;
        rdfs:isDefinedBy  <http://purl.org/cld/freq/> ;
        rdfs:seeAlso      <https://www.loc.gov/marc/holdings/hd853855.html> ;
        skos:inScheme     <http://purl.org/cld/terms/Frequency> ;
        dcam:memberOf     <http://purl.org/cld/terms/Frequency> .

idsc:THREE_TIMES_A_MONTH
        rdf:type          ids:Frequency ;
        rdf:type          skos:Concept ;
        rdfs:label        "Three times a month"@en ;
        skos:prefLabel    "Three times a month"@en ;
        rdfs:comment      "The event occurs three times a month."@en ;
        owl:sameAs        <http://purl.org/cld/freq/threeTimesAMonth> ;
        rdfs:isDefinedBy  <http://purl.org/cld/freq/> ;
        rdfs:seeAlso      <https://www.loc.gov/marc/holdings/hd853855.html> ;
        skos:inScheme     <http://purl.org/cld/terms/Frequency> ;
        dcam:memberOf     <http://purl.org/cld/terms/Frequency> .

idsc:WEEKLY  rdf:type     ids:Frequency ;
        rdf:type          skos:Concept ;
        rdfs:label        "Weekly"@en ;
        skos:prefLabel    "Weekly"@en ;
        rdfs:comment      "The event occurs once a week."@en ;
        owl:sameAs        <http://purl.org/cld/freq/weekly> ;
        rdfs:isDefinedBy  <http://purl.org/cld/freq/> ;
        rdfs:seeAlso      <https://www.loc.gov/marc/holdings/hd853855.html> ;
        skos:inScheme     <http://purl.org/cld/terms/Frequency> ;
        dcam:memberOf     <http://purl.org/cld/terms/Frequency> .

idsc:SEMIWEEKLY  rdf:type  ids:Frequency ;
        rdf:type          skos:Concept ;
        rdfs:label        "Semiweekly"@en ;
        skos:prefLabel    "Semiweekly"@en ;
        rdfs:comment      "The event occurs twice a week."@en ;
        owl:sameAs        <http://purl.org/cld/freq/semiweekly> ;
        rdfs:isDefinedBy  <http://purl.org/cld/freq/> ;
        rdfs:seeAlso      <https://www.loc.gov/marc/holdings/hd853855.html> ;
        skos:inScheme     <http://purl.org/cld/terms/Frequency> ;
        dcam:memberOf     <http://purl.org/cld/terms/Frequency> .

idsc:THREE_TIMES_A_WEEK
        rdf:type          ids:Frequency ;
        rdf:type          skos:Concept ;
        rdfs:label        "Three times a week"@en ;
        skos:prefLabel    "Three times a week"@en ;
        rdfs:comment      "The event occurs three times a week."@en ;
        owl:sameAs        <http://purl.org/cld/freq/threeTimesAWeek> ;
        rdfs:isDefinedBy  <http://purl.org/cld/freq/> ;
        rdfs:seeAlso      <https://www.loc.gov/marc/holdings/hd853855.html> ;
        skos:inScheme     <http://purl.org/cld/terms/Frequency> ;
        dcam:memberOf     <http://purl.org/cld/terms/Frequency> .

idsc:DAILY  rdf:type      ids:Frequency ;
        rdf:type          skos:Concept ;
        rdfs:label        "Daily"@en ;
        skos:prefLabel    "Daily"@en ;
        rdfs:comment      "The event occurs once a day."@en ;
        owl:sameAs        <http://purl.org/cld/freq/daily> ;
        rdfs:isDefinedBy  <http://purl.org/cld/freq/> ;
        rdfs:seeAlso      <https://www.loc.gov/marc/holdings/hd853855.html> ;
        skos:inScheme     <http://purl.org/cld/terms/Frequency> ;
        dcam:memberOf     <http://purl.org/cld/terms/Frequency> .

idsc:TWO_TIMES_A_DAY  rdf:type  ids:Frequency ;
        rdf:type      skos:Concept ;
        rdfs:label    "Two times a day"@en ;
        rdfs:comment  "The event occurs twice a day."@en .

idsc:EVERY_THREE_HOURS
        rdf:type      ids:Frequency ;
        rdf:type      skos:Concept ;
        rdfs:label    "Every three hours"@en ;
        rdfs:comment  "The event occurs every three hours."@en .

idsc:BIHOURLY  rdf:type  ids:Frequency ;
        rdf:type      skos:Concept ;
        rdfs:label    "Bihourly"@en ;
        rdfs:comment  "The event occurs twice an hour."@en .

idsc:HOURLY  rdf:type  ids:Frequency ;
        rdf:type      skos:Concept ;
        rdfs:label    "Hourly"@en ;
        rdfs:comment  "The event occurs every hour."@en .

idsc:EVERY_30_MINUTES
        rdf:type      ids:Frequency ;
        rdf:type      skos:Concept ;
        rdfs:label    "Every 30 minutes"@en ;
        rdfs:comment  "The event occurs every 30 minutes."@en .

idsc:EVERY_15_MINUTES
        rdf:type      ids:Frequency ;
        rdf:type      skos:Concept ;
        rdfs:label    "Every 15 minutes"@en ;
        rdfs:comment  "The event occurs every 15 minutes."@en .

idsc:EVERY_10_MINUTES
        rdf:type      ids:Frequency ;
        rdf:type      skos:Concept ;
        rdfs:label    "Every 10 minutes"@en ;
        rdfs:comment  "The event occurs every 10 minutes."@en .

idsc:EVERY_5_MINUTES  rdf:type  ids:Frequency ;
        rdf:type      skos:Concept ;
        rdfs:label    "Every 5 minutes"@en ;
        rdfs:comment  "The event occurs every 5 minutes."@en .

idsc:EVERY_1_MINUTE  rdf:type  ids:Frequency ;
        rdf:type      skos:Concept ;
        rdfs:label    "Every 1 minutes"@en ;
        rdfs:comment  "The event occurs every 1 minute."@en .

idsc:ONCE  rdf:type   ids:Frequency ;
        rdf:type      skos:Concept ;
        rdfs:label    "Once"@en ;
        rdfs:comment  "The event occurs only once."@en .

idsc:CONTINUOUS  rdf:type  ids:Frequency ;
        rdf:type          skos:Concept ;
        rdfs:label        "Continuous"@en ;
        skos:prefLabel    "Continuous"@en ;
        rdfs:comment      "The event repeats without interruption."@en ;
        owl:sameAs        <http://purl.org/cld/freq/continuous> ;
        rdfs:isDefinedBy  <http://purl.org/cld/freq/> ;
        rdfs:seeAlso      <https://www.loc.gov/marc/holdings/hd853855.html> ;
        skos:inScheme     <http://purl.org/cld/terms/Frequency> ;
        dcam:memberOf     <http://purl.org/cld/terms/Frequency> .

idsc:IRREGULAR  rdf:type  ids:Frequency ;
        rdf:type          skos:Concept ;
        rdfs:label        "Irregular"@en ;
        skos:prefLabel    "Irregular"@en ;
        rdfs:comment      "The event occurs at uneven intervals."@en ;
        owl:sameAs        <http://purl.org/cld/freq/irregular> ;
        rdfs:isDefinedBy  <http://purl.org/cld/freq/> ;
        rdfs:seeAlso      <https://www.loc.gov/marc/holdings/hd853855.html> ;
        skos:inScheme     <http://purl.org/cld/terms/Frequency> ;
        dcam:memberOf     <http://purl.org/cld/terms/Frequency> .
@prefix owl:   <http://www.w3.org/2002/07/owl#> .
@prefix rdfs:  <http://www.w3.org/2000/01/rdf-schema#> .
@prefix dct:   <http://purl.org/dc/terms/> .
@prefix xsd:   <http://www.w3.org/2001/XMLSchema#> .
@prefix ids:   <https://w3id.org/idsa/core/> .
@prefix idsc:  <https://w3id.org/idsa/code/> .

idsc:IDS-REST  rdf:type  ids:IdsProtocolSpecification ;
        rdfs:label    "IDS REST" ;
        rdfs:comment  "The REST specification of the IDS interactions."@en ;
        rdfs:seeAlso  <https://github.com/International-Data-Spaces-Association/path/to/ids/rest/spec/> .

idsc:IDS-CP  rdf:type  ids:IdsProtocolSpecification ;
        rdfs:label    "IDS-CP" ;
        rdfs:comment  "The IDS-CP specification of the IDS interactions."@en ;
        rdfs:seeAlso  <https://github.com/International-Data-Spaces-Association/path/to/idscp/spec/> .

idsc:QUERY  rdf:type  ids:IdsProtocolSpecification ;
        rdfs:label    "Query" ;
        rdfs:comment  "Queries conforming to IDS specifications."@en ;
        rdfs:seeAlso  <https://www.w3.org/TR/sparql11-overview/> .

idsc:MULTIPART  rdf:type  ids:IdsProtocolSpecification ;
        rdfs:label    "IDS over Multipart" ;
        rdfs:comment  "The Multipart Messages implementation of the IDS interactions."@en ;
        rdfs:seeAlso  <https://github.com/International-Data-Spaces-Association/path/to/multipart/spec/> .
@prefix owl:   <http://www.w3.org/2002/07/owl#> .
@prefix rdfs:  <http://www.w3.org/2000/01/rdf-schema#> .
@prefix dct:   <http://purl.org/dc/terms/> .
@prefix xsd:   <http://www.w3.org/2001/XMLSchema#> .
@prefix ids:   <https://w3id.org/idsa/core/> .
@prefix idsc:  <https://w3id.org/idsa/code/> .

idsc:DSA  rdf:type  ids:KeyType ;
        rdfs:label  "DSA"@en .

idsc:ECDSA  rdf:type  ids:KeyType ;
        rdfs:label  "ECDSA"@en .

idsc:RSA  rdf:type  ids:KeyType ;
        rdfs:label  "RSA"@en .

idsc:ED25519  rdf:type  ids:KeyType ;
        rdfs:label  "ED25519"@en .
@prefix rdfs:  <http://www.w3.org/2000/01/rdf-schema#> .
@prefix owl:   <http://www.w3.org/2002/07/owl#> .
@prefix ids:   <https://w3id.org/idsa/core/> .
@prefix idsc:  <https://w3id.org/idsa/code/> .

idsc:MULTI_LINGUAL  rdf:type  ids:Language ;
        rdfs:label    "Multilingual"@en ;
        rdfs:comment  "Code indicates that several languages are used or no concrete language can be determined." .

idsc:AB  rdf:type   ids:Language ;
        rdfs:label  "Abkhaz"@en ;
        owl:sameAs  <http://dbpedia.org/resource/ISO_639:ab> .

idsc:AA  rdf:type   ids:Language ;
        rdfs:label  "Afar"@en ;
        owl:sameAs  <http://dbpedia.org/resource/ISO_639:aa> .

idsc:AF  rdf:type   ids:Language ;
        rdfs:label  "Afrikaans"@en ;
        owl:sameAs  <http://dbpedia.org/resource/ISO_639:af> .

idsc:AK  rdf:type   ids:Language ;
        rdfs:label  "Akan"@en ;
        owl:sameAs  <http://dbpedia.org/resource/ISO_639:ak> .

idsc:SQ  rdf:type   ids:Language ;
        rdfs:label  "Albanian"@en ;
        owl:sameAs  <http://dbpedia.org/resource/ISO_639:sq> .

idsc:AM  rdf:type   ids:Language ;
        rdfs:label  "Amharic"@en ;
        owl:sameAs  <http://dbpedia.org/resource/ISO_639:am> .

idsc:AR  rdf:type   ids:Language ;
        rdfs:label  "Arabic"@en ;
        owl:sameAs  <http://dbpedia.org/resource/ISO_639:ar> .

idsc:AN  rdf:type   ids:Language ;
        rdfs:label  "Aragonese"@en ;
        owl:sameAs  <http://dbpedia.org/resource/ISO_639:an> .

idsc:HY  rdf:type   ids:Language ;
        rdfs:label  "Armenian"@en ;
        owl:sameAs  <http://dbpedia.org/resource/ISO_639:hy> .

idsc:AS  rdf:type   ids:Language ;
        rdfs:label  "Assamese"@en ;
        owl:sameAs  <http://dbpedia.org/resource/ISO_639:as> .

idsc:AV  rdf:type   ids:Language ;
        rdfs:label  "Avaric"@en ;
        owl:sameAs  <http://dbpedia.org/resource/ISO_639:av> .

idsc:AE  rdf:type   ids:Language ;
        rdfs:label  "Avestan"@en ;
        owl:sameAs  <http://dbpedia.org/resource/ISO_639:ae> .

idsc:AY  rdf:type   ids:Language ;
        rdfs:label  "Aymara"@en ;
        owl:sameAs  <http://dbpedia.org/resource/ISO_639:ay> .

idsc:AZ  rdf:type   ids:Language ;
        rdfs:label  "Azerbaijani"@en ;
        owl:sameAs  <http://dbpedia.org/resource/ISO_639:az> .

idsc:BM  rdf:type   ids:Language ;
        rdfs:label  "Bambara"@en ;
        owl:sameAs  <http://dbpedia.org/resource/ISO_639:bm> .

idsc:BA  rdf:type   ids:Language ;
        rdfs:label  "Bashkir"@en ;
        owl:sameAs  <http://dbpedia.org/resource/ISO_639:ba> .

idsc:EU  rdf:type   ids:Language ;
        rdfs:label  "Basque"@en ;
        owl:sameAs  <http://dbpedia.org/resource/ISO_639:eu> .

idsc:BE  rdf:type   ids:Language ;
        rdfs:label  "Belarusian"@en ;
        owl:sameAs  <http://dbpedia.org/resource/ISO_639:be> .

idsc:BN  rdf:type   ids:Language ;
        rdfs:label  "Bengali, Bangla"@en ;
        owl:sameAs  <http://dbpedia.org/resource/ISO_639:bn> .

idsc:BH  rdf:type   ids:Language ;
        rdfs:label  "Bihari"@en ;
        owl:sameAs  <http://dbpedia.org/resource/ISO_639:bh> .

idsc:BI  rdf:type   ids:Language ;
        rdfs:label  "Bislama"@en ;
        owl:sameAs  <http://dbpedia.org/resource/ISO_639:bi> .

idsc:BS  rdf:type   ids:Language ;
        rdfs:label  "Bosnian"@en ;
        owl:sameAs  <http://dbpedia.org/resource/ISO_639:bs> .

idsc:BR  rdf:type   ids:Language ;
        rdfs:label  "Breton"@en ;
        owl:sameAs  <http://dbpedia.org/resource/ISO_639:br> .

idsc:BG  rdf:type   ids:Language ;
        rdfs:label  "Bulgarian"@en ;
        owl:sameAs  <http://dbpedia.org/resource/ISO_639:bg> .

idsc:MY  rdf:type   ids:Language ;
        rdfs:label  "Burmese"@en ;
        owl:sameAs  <http://dbpedia.org/resource/ISO_639:my> .

idsc:CA  rdf:type   ids:Language ;
        rdfs:label  "Catalan"@en ;
        owl:sameAs  <http://dbpedia.org/resource/ISO_639:ca> .

idsc:CH  rdf:type   ids:Language ;
        rdfs:label  "Chamorro"@en ;
        owl:sameAs  <http://dbpedia.org/resource/ISO_639:ch> .

idsc:CE  rdf:type   ids:Language ;
        rdfs:label  "Chechen"@en ;
        owl:sameAs  <http://dbpedia.org/resource/ISO_639:ce> .

idsc:NY  rdf:type   ids:Language ;
        rdfs:label  "Chichewa, Chewa, Nyanja"@en ;
        owl:sameAs  <http://dbpedia.org/resource/ISO_639:ny> .

idsc:ZH  rdf:type   ids:Language ;
        rdfs:label  "Chinese"@en ;
        owl:sameAs  <http://dbpedia.org/resource/ISO_639:zh> .

idsc:CV  rdf:type   ids:Language ;
        rdfs:label  "Chuvash"@en ;
        owl:sameAs  <http://dbpedia.org/resource/ISO_639:cv> .

idsc:KW  rdf:type   ids:Language ;
        rdfs:label  "Cornish"@en ;
        owl:sameAs  <http://dbpedia.org/resource/ISO_639:kw> .

idsc:CO  rdf:type   ids:Language ;
        rdfs:label  "Corsican"@en ;
        owl:sameAs  <http://dbpedia.org/resource/ISO_639:co> .

idsc:CR  rdf:type   ids:Language ;
        rdfs:label  "Cree"@en ;
        owl:sameAs  <http://dbpedia.org/resource/ISO_639:cr> .

idsc:HR  rdf:type   ids:Language ;
        rdfs:label  "Croatian"@en ;
        owl:sameAs  <http://dbpedia.org/resource/ISO_639:hr> .

idsc:CS  rdf:type   ids:Language ;
        rdfs:label  "Czech"@en ;
        owl:sameAs  <http://dbpedia.org/resource/ISO_639:cs> .

idsc:DA  rdf:type   ids:Language ;
        rdfs:label  "Danish"@en ;
        owl:sameAs  <http://dbpedia.org/resource/ISO_639:da> .

idsc:DV  rdf:type   ids:Language ;
        rdfs:label  "Divehi, Dhivehi, Maldivian"@en ;
        owl:sameAs  <http://dbpedia.org/resource/ISO_639:dv> .

idsc:NL  rdf:type   ids:Language ;
        rdfs:label  "Dutch"@en ;
        owl:sameAs  <http://dbpedia.org/resource/ISO_639:nl> .

idsc:DZ  rdf:type   ids:Language ;
        rdfs:label  "Dzongkha"@en ;
        owl:sameAs  <http://dbpedia.org/resource/ISO_639:dz> .

idsc:EN  rdf:type   ids:Language ;
        rdfs:label  "English"@en ;
        owl:sameAs  <http://dbpedia.org/resource/ISO_639:en> .

idsc:EO  rdf:type   ids:Language ;
        rdfs:label  "Esperanto"@en ;
        owl:sameAs  <http://dbpedia.org/resource/ISO_639:eo> .

idsc:ET  rdf:type   ids:Language ;
        rdfs:label  "Estonian"@en ;
        owl:sameAs  <http://dbpedia.org/resource/ISO_639:et> .

idsc:EE  rdf:type   ids:Language ;
        rdfs:label  "Ewe"@en ;
        owl:sameAs  <http://dbpedia.org/resource/ISO_639:ee> .

idsc:FO  rdf:type   ids:Language ;
        rdfs:label  "Faroese"@en ;
        owl:sameAs  <http://dbpedia.org/resource/ISO_639:fo> .

idsc:FJ  rdf:type   ids:Language ;
        rdfs:label  "Fijian"@en ;
        owl:sameAs  <http://dbpedia.org/resource/ISO_639:fj> .

idsc:FI  rdf:type   ids:Language ;
        rdfs:label  "Finnish"@en ;
        owl:sameAs  <http://dbpedia.org/resource/ISO_639:fi> .

idsc:FR  rdf:type   ids:Language ;
        rdfs:label  "French"@en ;
        owl:sameAs  <http://dbpedia.org/resource/ISO_639:fr> .

idsc:FF  rdf:type   ids:Language ;
        rdfs:label  "Fula, Fulah, Pulaar, Pular"@en ;
        owl:sameAs  <http://dbpedia.org/resource/ISO_639:ff> .

idsc:GL  rdf:type   ids:Language ;
        rdfs:label  "Galician"@en ;
        owl:sameAs  <http://dbpedia.org/resource/ISO_639:gl> .

idsc:KA  rdf:type   ids:Language ;
        rdfs:label  "Georgian"@en ;
        owl:sameAs  <http://dbpedia.org/resource/ISO_639:ka> .

idsc:DE  rdf:type   ids:Language ;
        rdfs:label  "German"@en ;
        owl:sameAs  <http://dbpedia.org/resource/ISO_639:de> .

idsc:EL  rdf:type   ids:Language ;
        rdfs:label  "Greek (modern)"@en ;
        owl:sameAs  <http://dbpedia.org/resource/ISO_639:el> .

idsc:GN  rdf:type   ids:Language ;
        rdfs:label  "Guaraní"@en ;
        owl:sameAs  <http://dbpedia.org/resource/ISO_639:gn> .

idsc:GU  rdf:type   ids:Language ;
        rdfs:label  "Gujarati"@en ;
        owl:sameAs  <http://dbpedia.org/resource/ISO_639:gu> .

idsc:HT  rdf:type   ids:Language ;
        rdfs:label  "Haitian, Haitian Creole"@en ;
        owl:sameAs  <http://dbpedia.org/resource/ISO_639:ht> .

idsc:HA  rdf:type   ids:Language ;
        rdfs:label  "Hausa"@en ;
        owl:sameAs  <http://dbpedia.org/resource/ISO_639:ha> .

idsc:HE  rdf:type   ids:Language ;
        rdfs:label  "Hebrew (modern)"@en ;
        owl:sameAs  <http://dbpedia.org/resource/ISO_639:he> .

idsc:HZ  rdf:type   ids:Language ;
        rdfs:label  "Herero"@en ;
        owl:sameAs  <http://dbpedia.org/resource/ISO_639:hz> .

idsc:HI  rdf:type   ids:Language ;
        rdfs:label  "Hindi"@en ;
        owl:sameAs  <http://dbpedia.org/resource/ISO_639:hi> .

idsc:HO  rdf:type   ids:Language ;
        rdfs:label  "Hiri Motu"@en ;
        owl:sameAs  <http://dbpedia.org/resource/ISO_639:ho> .

idsc:HU  rdf:type   ids:Language ;
        rdfs:label  "Hungarian"@en ;
        owl:sameAs  <http://dbpedia.org/resource/ISO_639:hu> .

idsc:IA  rdf:type   ids:Language ;
        rdfs:label  "Interlingua"@en ;
        owl:sameAs  <http://dbpedia.org/resource/ISO_639:ia> .

idsc:ID  rdf:type   ids:Language ;
        rdfs:label  "Indonesian"@en ;
        owl:sameAs  <http://dbpedia.org/resource/ISO_639:id> .

idsc:IE  rdf:type   ids:Language ;
        rdfs:label  "Interlingue"@en ;
        owl:sameAs  <http://dbpedia.org/resource/ISO_639:ie> .

idsc:GA  rdf:type   ids:Language ;
        rdfs:label  "Irish"@en ;
        owl:sameAs  <http://dbpedia.org/resource/ISO_639:ga> .

idsc:IG  rdf:type   ids:Language ;
        rdfs:label  "Igbo"@en ;
        owl:sameAs  <http://dbpedia.org/resource/ISO_639:ig> .

idsc:IK  rdf:type   ids:Language ;
        rdfs:label  "Inupiaq"@en ;
        owl:sameAs  <http://dbpedia.org/resource/ISO_639:ik> .

idsc:IO  rdf:type   ids:Language ;
        rdfs:label  "Ido"@en ;
        owl:sameAs  <http://dbpedia.org/resource/ISO_639:io> .

idsc:IS  rdf:type   ids:Language ;
        rdfs:label  "Icelandic"@en ;
        owl:sameAs  <http://dbpedia.org/resource/ISO_639:is> .

idsc:IT  rdf:type   ids:Language ;
        rdfs:label  "Italian"@en ;
        owl:sameAs  <http://dbpedia.org/resource/ISO_639:it> .

idsc:IU  rdf:type   ids:Language ;
        rdfs:label  "Inuktitut"@en ;
        owl:sameAs  <http://dbpedia.org/resource/ISO_639:iu> .

idsc:JA  rdf:type   ids:Language ;
        rdfs:label  "Japanese"@en ;
        owl:sameAs  <http://dbpedia.org/resource/ISO_639:ja> .

idsc:JV  rdf:type   ids:Language ;
        rdfs:label  "Javanese"@en ;
        owl:sameAs  <http://dbpedia.org/resource/ISO_639:jv> .

idsc:KL  rdf:type   ids:Language ;
        rdfs:label  "Kalaallisut, Greenlandic"@en ;
        owl:sameAs  <http://dbpedia.org/resource/ISO_639:kl> .

idsc:KN  rdf:type   ids:Language ;
        rdfs:label  "Kannada"@en ;
        owl:sameAs  <http://dbpedia.org/resource/ISO_639:kn> .

idsc:KR  rdf:type   ids:Language ;
        rdfs:label  "Kanuri"@en ;
        owl:sameAs  <http://dbpedia.org/resource/ISO_639:kr> .

idsc:KS  rdf:type   ids:Language ;
        rdfs:label  "Kashmiri"@en ;
        owl:sameAs  <http://dbpedia.org/resource/ISO_639:ks> .

idsc:KK  rdf:type   ids:Language ;
        rdfs:label  "Kazakh"@en ;
        owl:sameAs  <http://dbpedia.org/resource/ISO_639:kk> .

idsc:KM  rdf:type   ids:Language ;
        rdfs:label  "Khmer"@en ;
        owl:sameAs  <http://dbpedia.org/resource/ISO_639:km> .

idsc:KI  rdf:type   ids:Language ;
        rdfs:label  "Kikuyu, Gikuyu"@en ;
        owl:sameAs  <http://dbpedia.org/resource/ISO_639:ki> .

idsc:RW  rdf:type   ids:Language ;
        rdfs:label  "Kinyarwanda"@en ;
        owl:sameAs  <http://dbpedia.org/resource/ISO_639:rw> .

idsc:KY  rdf:type   ids:Language ;
        rdfs:label  "Kyrgyz"@en ;
        owl:sameAs  <http://dbpedia.org/resource/ISO_639:ky> .

idsc:KV  rdf:type   ids:Language ;
        rdfs:label  "Komi"@en ;
        owl:sameAs  <http://dbpedia.org/resource/ISO_639:kv> .

idsc:KG  rdf:type   ids:Language ;
        rdfs:label  "Kongo"@en ;
        owl:sameAs  <http://dbpedia.org/resource/ISO_639:kg> .

idsc:KO  rdf:type   ids:Language ;
        rdfs:label  "Korean"@en ;
        owl:sameAs  <http://dbpedia.org/resource/ISO_639:ko> .

idsc:KU  rdf:type   ids:Language ;
        rdfs:label  "Kurdish"@en ;
        owl:sameAs  <http://dbpedia.org/resource/ISO_639:ku> .

idsc:KJ  rdf:type   ids:Language ;
        rdfs:label  "Kwanyama, Kuanyama"@en ;
        owl:sameAs  <http://dbpedia.org/resource/ISO_639:kj> .

idsc:LA  rdf:type   ids:Language ;
        rdfs:label  "Latin"@en ;
        owl:sameAs  <http://dbpedia.org/resource/ISO_639:la> .

idsc:LB  rdf:type   ids:Language ;
        rdfs:label  "Luxembourgish, Letzeburgesch"@en ;
        owl:sameAs  <http://dbpedia.org/resource/ISO_639:lb> .

idsc:LG  rdf:type   ids:Language ;
        rdfs:label  "Ganda"@en ;
        owl:sameAs  <http://dbpedia.org/resource/ISO_639:lg> .

idsc:LI  rdf:type   ids:Language ;
        rdfs:label  "Limburgish, Limburgan, Limburger"@en ;
        owl:sameAs  <http://dbpedia.org/resource/ISO_639:li> .

idsc:LN  rdf:type   ids:Language ;
        rdfs:label  "Lingala"@en ;
        owl:sameAs  <http://dbpedia.org/resource/ISO_639:ln> .

idsc:LO  rdf:type   ids:Language ;
        rdfs:label  "Lao"@en ;
        owl:sameAs  <http://dbpedia.org/resource/ISO_639:lo> .

idsc:LT  rdf:type   ids:Language ;
        rdfs:label  "Lithuanian"@en ;
        owl:sameAs  <http://dbpedia.org/resource/ISO_639:lt> .

idsc:LU  rdf:type   ids:Language ;
        rdfs:label  "Luba-Katanga"@en ;
        owl:sameAs  <http://dbpedia.org/resource/ISO_639:lu> .

idsc:LV  rdf:type   ids:Language ;
        rdfs:label  "Latvian"@en ;
        owl:sameAs  <http://dbpedia.org/resource/ISO_639:lv> .

idsc:GV  rdf:type   ids:Language ;
        rdfs:label  "Manx"@en ;
        owl:sameAs  <http://dbpedia.org/resource/ISO_639:gv> .

idsc:MK  rdf:type   ids:Language ;
        rdfs:label  "Macedonian"@en ;
        owl:sameAs  <http://dbpedia.org/resource/ISO_639:mk> .

idsc:MG  rdf:type   ids:Language ;
        rdfs:label  "Malagasy"@en ;
        owl:sameAs  <http://dbpedia.org/resource/ISO_639:mg> .

idsc:MS  rdf:type   ids:Language ;
        rdfs:label  "Malay"@en ;
        owl:sameAs  <http://dbpedia.org/resource/ISO_639:ms> .

idsc:ML  rdf:type   ids:Language ;
        rdfs:label  "Malayalam"@en ;
        owl:sameAs  <http://dbpedia.org/resource/ISO_639:ml> .

idsc:MT  rdf:type   ids:Language ;
        rdfs:label  "Maltese"@en ;
        owl:sameAs  <http://dbpedia.org/resource/ISO_639:mt> .

idsc:MI  rdf:type   ids:Language ;
        rdfs:label  "Māori"@en ;
        owl:sameAs  <http://dbpedia.org/resource/ISO_639:mi> .

idsc:MR  rdf:type   ids:Language ;
        rdfs:label  "Marathi (Marāṭhī)"@en ;
        owl:sameAs  <http://dbpedia.org/resource/ISO_639:mr> .

idsc:MH  rdf:type   ids:Language ;
        rdfs:label  "Marshallese"@en ;
        owl:sameAs  <http://dbpedia.org/resource/ISO_639:mh> .

idsc:MN  rdf:type   ids:Language ;
        rdfs:label  "Mongolian"@en ;
        owl:sameAs  <http://dbpedia.org/resource/ISO_639:mn> .

idsc:NA  rdf:type   ids:Language ;
        rdfs:label  "Nauruan"@en ;
        owl:sameAs  <http://dbpedia.org/resource/ISO_639:na> .

idsc:NV  rdf:type   ids:Language ;
        rdfs:label  "Navajo, Navaho"@en ;
        owl:sameAs  <http://dbpedia.org/resource/ISO_639:nv> .

idsc:ND  rdf:type   ids:Language ;
        rdfs:label  "Northern Ndebele"@en ;
        owl:sameAs  <http://dbpedia.org/resource/ISO_639:nd> .

idsc:NE  rdf:type   ids:Language ;
        rdfs:label  "Nepali"@en ;
        owl:sameAs  <http://dbpedia.org/resource/ISO_639:ne> .

idsc:NG  rdf:type   ids:Language ;
        rdfs:label  "Ndonga"@en ;
        owl:sameAs  <http://dbpedia.org/resource/ISO_639:ng> .

idsc:NB  rdf:type   ids:Language ;
        rdfs:label  "Norwegian Bokmål"@en ;
        owl:sameAs  <http://dbpedia.org/resource/ISO_639:nb> .

idsc:NN  rdf:type   ids:Language ;
        rdfs:label  "Norwegian Nynorsk"@en ;
        owl:sameAs  <http://dbpedia.org/resource/ISO_639:nn> .

idsc:NO  rdf:type   ids:Language ;
        rdfs:label  "Norwegian"@en ;
        owl:sameAs  <http://dbpedia.org/resource/ISO_639:no> .

idsc:II  rdf:type   ids:Language ;
        rdfs:label  "Nuosu"@en ;
        owl:sameAs  <http://dbpedia.org/resource/ISO_639:ii> .

idsc:NR  rdf:type   ids:Language ;
        rdfs:label  "Southern Ndebele"@en ;
        owl:sameAs  <http://dbpedia.org/resource/ISO_639:nr> .

idsc:OC  rdf:type   ids:Language ;
        rdfs:label  "Occitan"@en ;
        owl:sameAs  <http://dbpedia.org/resource/ISO_639:oc> .

idsc:OJ  rdf:type   ids:Language ;
        rdfs:label  "Ojibwe, Ojibwa"@en ;
        owl:sameAs  <http://dbpedia.org/resource/ISO_639:oj> .

idsc:CU  rdf:type   ids:Language ;
        rdfs:label  "Old Church Slavonic, Church Slavonic, Old Bulgarian"@en ;
        owl:sameAs  <http://dbpedia.org/resource/ISO_639:cu> .

idsc:OM  rdf:type   ids:Language ;
        rdfs:label  "Oromo"@en ;
        owl:sameAs  <http://dbpedia.org/resource/ISO_639:om> .

idsc:OR  rdf:type   ids:Language ;
        rdfs:label  "Oriya"@en ;
        owl:sameAs  <http://dbpedia.org/resource/ISO_639:or> .

idsc:OS  rdf:type   ids:Language ;
        rdfs:label  "Ossetian, Ossetic"@en ;
        owl:sameAs  <http://dbpedia.org/resource/ISO_639:os> .

idsc:PA  rdf:type   ids:Language ;
        rdfs:label  "(Eastern) Punjabi"@en ;
        owl:sameAs  <http://dbpedia.org/resource/ISO_639:pa> .

idsc:PI  rdf:type   ids:Language ;
        rdfs:label  "Pāli"@en ;
        owl:sameAs  <http://dbpedia.org/resource/ISO_639:pi> .

idsc:FA  rdf:type   ids:Language ;
        rdfs:label  "Persian (Farsi)"@en ;
        owl:sameAs  <http://dbpedia.org/resource/ISO_639:fa> .

idsc:PL  rdf:type   ids:Language ;
        rdfs:label  "Polish"@en ;
        owl:sameAs  <http://dbpedia.org/resource/ISO_639:pl> .

idsc:PS  rdf:type   ids:Language ;
        rdfs:label  "Pashto, Pushto"@en ;
        owl:sameAs  <http://dbpedia.org/resource/ISO_639:ps> .

idsc:PT  rdf:type   ids:Language ;
        rdfs:label  "Portuguese"@en ;
        owl:sameAs  <http://dbpedia.org/resource/ISO_639:pt> .

idsc:QU  rdf:type   ids:Language ;
        rdfs:label  "Quechua"@en ;
        owl:sameAs  <http://dbpedia.org/resource/ISO_639:qu> .

idsc:RM  rdf:type   ids:Language ;
        rdfs:label  "Romansh"@en ;
        owl:sameAs  <http://dbpedia.org/resource/ISO_639:rm> .

idsc:RN  rdf:type   ids:Language ;
        rdfs:label  "Kirundi"@en ;
        owl:sameAs  <http://dbpedia.org/resource/ISO_639:rn> .

idsc:RO  rdf:type   ids:Language ;
        rdfs:label  "Romanian"@en ;
        owl:sameAs  <http://dbpedia.org/resource/ISO_639:ro> .

idsc:RU  rdf:type   ids:Language ;
        rdfs:label  "Russian"@en ;
        owl:sameAs  <http://dbpedia.org/resource/ISO_639:ru> .

idsc:SA  rdf:type   ids:Language ;
        rdfs:label  "Sanskrit (Saṁskṛta)"@en ;
        owl:sameAs  <http://dbpedia.org/resource/ISO_639:sa> .

idsc:SC  rdf:type   ids:Language ;
        rdfs:label  "Sardinian"@en ;
        owl:sameAs  <http://dbpedia.org/resource/ISO_639:sc> .

idsc:SD  rdf:type   ids:Language ;
        rdfs:label  "Sindhi"@en ;
        owl:sameAs  <http://dbpedia.org/resource/ISO_639:sd> .

idsc:SE  rdf:type   ids:Language ;
        rdfs:label  "Northern Sami"@en ;
        owl:sameAs  <http://dbpedia.org/resource/ISO_639:se> .

idsc:SM  rdf:type   ids:Language ;
        rdfs:label  "Samoan"@en ;
        owl:sameAs  <http://dbpedia.org/resource/ISO_639:sm> .

idsc:SG  rdf:type   ids:Language ;
        rdfs:label  "Sango"@en ;
        owl:sameAs  <http://dbpedia.org/resource/ISO_639:sg> .

idsc:SR  rdf:type   ids:Language ;
        rdfs:label  "Serbian"@en ;
        owl:sameAs  <http://dbpedia.org/resource/ISO_639:sr> .

idsc:GD  rdf:type   ids:Language ;
        rdfs:label  "Scottish Gaelic, Gaelic"@en ;
        owl:sameAs  <http://dbpedia.org/resource/ISO_639:gd> .

idsc:SN  rdf:type   ids:Language ;
        rdfs:label  "Shona"@en ;
        owl:sameAs  <http://dbpedia.org/resource/ISO_639:sn> .

idsc:SI  rdf:type   ids:Language ;
        rdfs:label  "Sinhalese, Sinhala"@en ;
        owl:sameAs  <http://dbpedia.org/resource/ISO_639:si> .

idsc:SK  rdf:type   ids:Language ;
        rdfs:label  "Slovak"@en ;
        owl:sameAs  <http://dbpedia.org/resource/ISO_639:sk> .

idsc:SL  rdf:type   ids:Language ;
        rdfs:label  "Slovene"@en ;
        owl:sameAs  <http://dbpedia.org/resource/ISO_639:sl> .

idsc:SO  rdf:type   ids:Language ;
        rdfs:label  "Somali"@en ;
        owl:sameAs  <http://dbpedia.org/resource/ISO_639:so> .

idsc:ST  rdf:type   ids:Language ;
        rdfs:label  "Southern Sotho"@en ;
        owl:sameAs  <http://dbpedia.org/resource/ISO_639:st> .

idsc:ES  rdf:type   ids:Language ;
        rdfs:label  "Spanish"@en ;
        owl:sameAs  <http://dbpedia.org/resource/ISO_639:es> .

idsc:SU  rdf:type   ids:Language ;
        rdfs:label  "Sundanese"@en ;
        owl:sameAs  <http://dbpedia.org/resource/ISO_639:su> .

idsc:SW  rdf:type   ids:Language ;
        rdfs:label  "Swahili"@en ;
        owl:sameAs  <http://dbpedia.org/resource/ISO_639:sw> .

idsc:SS  rdf:type   ids:Language ;
        rdfs:label  "Swati"@en ;
        owl:sameAs  <http://dbpedia.org/resource/ISO_639:ss> .

idsc:SV  rdf:type   ids:Language ;
        rdfs:label  "Swedish"@en ;
        owl:sameAs  <http://dbpedia.org/resource/ISO_639:sv> .

idsc:TA  rdf:type   ids:Language ;
        rdfs:label  "Tamil"@en ;
        owl:sameAs  <http://dbpedia.org/resource/ISO_639:ta> .

idsc:TE  rdf:type   ids:Language ;
        rdfs:label  "Telugu"@en ;
        owl:sameAs  <http://dbpedia.org/resource/ISO_639:te> .

idsc:TG  rdf:type   ids:Language ;
        rdfs:label  "Tajik"@en ;
        owl:sameAs  <http://dbpedia.org/resource/ISO_639:tg> .

idsc:TH  rdf:type   ids:Language ;
        rdfs:label  "Thai"@en ;
        owl:sameAs  <http://dbpedia.org/resource/ISO_639:th> .

idsc:TI  rdf:type   ids:Language ;
        rdfs:label  "Tigrinya"@en ;
        owl:sameAs  <http://dbpedia.org/resource/ISO_639:ti> .

idsc:BO  rdf:type   ids:Language ;
        rdfs:label  "Tibetan Standard, Tibetan, Central"@en ;
        owl:sameAs  <http://dbpedia.org/resource/ISO_639:bo> .

idsc:TK  rdf:type   ids:Language ;
        rdfs:label  "Turkmen"@en ;
        owl:sameAs  <http://dbpedia.org/resource/ISO_639:tk> .

idsc:TL  rdf:type   ids:Language ;
        rdfs:label  "Tagalog"@en ;
        owl:sameAs  <http://dbpedia.org/resource/ISO_639:tl> .

idsc:TN  rdf:type   ids:Language ;
        rdfs:label  "Tswana"@en ;
        owl:sameAs  <http://dbpedia.org/resource/ISO_639:tn> .

idsc:TO  rdf:type   ids:Language ;
        rdfs:label  "Tonga (Tonga Islands)"@en ;
        owl:sameAs  <http://dbpedia.org/resource/ISO_639:to> .

idsc:TR  rdf:type   ids:Language ;
        rdfs:label  "Turkish"@en ;
        owl:sameAs  <http://dbpedia.org/resource/ISO_639:tr> .

idsc:TS  rdf:type   ids:Language ;
        rdfs:label  "Tsonga"@en ;
        owl:sameAs  <http://dbpedia.org/resource/ISO_639:ts> .

idsc:TT  rdf:type   ids:Language ;
        rdfs:label  "Tatar"@en ;
        owl:sameAs  <http://dbpedia.org/resource/ISO_639:tt> .

idsc:TW  rdf:type   ids:Language ;
        rdfs:label  "Twi"@en ;
        owl:sameAs  <http://dbpedia.org/resource/ISO_639:tw> .

idsc:TY  rdf:type   ids:Language ;
        rdfs:label  "Tahitian"@en ;
        owl:sameAs  <http://dbpedia.org/resource/ISO_639:ty> .

idsc:UG  rdf:type   ids:Language ;
        rdfs:label  "Uyghur"@en ;
        owl:sameAs  <http://dbpedia.org/resource/ISO_639:ug> .

idsc:UK  rdf:type   ids:Language ;
        rdfs:label  "Ukrainian"@en ;
        owl:sameAs  <http://dbpedia.org/resource/ISO_639:uk> .

idsc:UR  rdf:type   ids:Language ;
        rdfs:label  "Urdu"@en ;
        owl:sameAs  <http://dbpedia.org/resource/ISO_639:ur> .

idsc:UZ  rdf:type   ids:Language ;
        rdfs:label  "Uzbek"@en ;
        owl:sameAs  <http://dbpedia.org/resource/ISO_639:uz> .

idsc:VE  rdf:type   ids:Language ;
        rdfs:label  "Venda"@en ;
        owl:sameAs  <http://dbpedia.org/resource/ISO_639:ve> .

idsc:VI  rdf:type   ids:Language ;
        rdfs:label  "Vietnamese"@en ;
        owl:sameAs  <http://dbpedia.org/resource/ISO_639:vi> .

idsc:VO  rdf:type   ids:Language ;
        rdfs:label  "Volapük"@en ;
        owl:sameAs  <http://dbpedia.org/resource/ISO_639:vo> .

idsc:WA  rdf:type   ids:Language ;
        rdfs:label  "Walloon"@en ;
        owl:sameAs  <http://dbpedia.org/resource/ISO_639:wa> .

idsc:CY  rdf:type   ids:Language ;
        rdfs:label  "Welsh"@en ;
        owl:sameAs  <http://dbpedia.org/resource/ISO_639:cy> .

idsc:WO  rdf:type   ids:Language ;
        rdfs:label  "Wolof"@en ;
        owl:sameAs  <http://dbpedia.org/resource/ISO_639:wo> .

idsc:FY  rdf:type   ids:Language ;
        rdfs:label  "Western Frisian"@en ;
        owl:sameAs  <http://dbpedia.org/resource/ISO_639:fy> .

idsc:XH  rdf:type   ids:Language ;
        rdfs:label  "Xhosa"@en ;
        owl:sameAs  <http://dbpedia.org/resource/ISO_639:xh> .

idsc:YI  rdf:type   ids:Language ;
        rdfs:label  "Yiddish"@en ;
        owl:sameAs  <http://dbpedia.org/resource/ISO_639:yi> .

idsc:YO  rdf:type   ids:Language ;
        rdfs:label  "Yoruba"@en ;
        owl:sameAs  <http://dbpedia.org/resource/ISO_639:yo> .

idsc:ZA  rdf:type   ids:Language ;
        rdfs:label  "Zhuang, Chuang"@en ;
        owl:sameAs  <http://dbpedia.org/resource/ISO_639:za> .

idsc:ZU  rdf:type   ids:Language ;
        rdfs:label  "Zulu"@en ;
        owl:sameAs  <http://dbpedia.org/resource/ISO_639:zu> .
@prefix owl:   <http://www.w3.org/2002/07/owl#> .
@prefix rdfs:  <http://www.w3.org/2000/01/rdf-schema#> .
@prefix dct:   <http://purl.org/dc/terms/> .
@prefix xsd:   <http://www.w3.org/2001/XMLSchema#> .
@prefix ids:   <https://w3id.org/idsa/core/> .
@prefix idsc:  <https://w3id.org/idsa/code/> .
@prefix skos:  <http://www.w3.org/2004/02/skos/core#> .
@prefix time:  <http://www.w3.org/2006/time#> .
@prefix odrl:  <http://www.w3.org/ns/odrl/2/> .

idsc:PAYMENT  rdf:type  odrl:LeftOperand ;
        rdfs:label    "payment"@en ;
        rdfs:comment  "Monetary payment, without any further sepcification on the type, amount or purpose."@en .

idsc:PAY_AMOUNT  rdf:type  odrl:LeftOperand ;
        skos:broader  odrl:payAmount ;
        ids:broader   idsc:PAYMENT ;
        rdfs:label    "payAmount"@en ;
        rdfs:comment  "Monetary amount to pay, usually used with idsc:EQ. Datatype is double. Currency required."@en .

idsc:POLICY_EVALUATION_TIME
        rdf:type      odrl:LeftOperand ;
        skos:broader  odrl:dateTime ;
        rdfs:label    "policy evaluation time"@en ;
        rdfs:comment  "The current system time (as UTC xsd:dateTimeStamp) for evaluating a time-related constraint. Allowed operators are idsc:AFTER, idsc:BEFORE, idsc:CONTAINS, idsc:TEMPORAL_DISJOINT, idsc:DURING, idsc:TEMPORAL_EQUALS, idsc:FINISHED_BY, idsc:FINISHES, idsc:MEETS, idsc:MET_BY, idsc:OVERLAPS, idsc:OVERLAPPED_BY, idsc:STARTS, idsc:STARTED_BY and idsc:DURATION_EQ with RightOperand time:TemporalEntity."@en .

idsc:ELAPSED_TIME  rdf:type  odrl:LeftOperand ;
        skos:broader  odrl:elapsedTime ;
        rdfs:label    "elapsed time"@en ;
        rdfs:comment  "A continuous elapsed time period which may be used for exercising of the action of the Rule. Allowed operators are idsc:SHORTER, idsc:SHORTER_EQ, idsc:LONGER, idsc:LONGER_EQ, and idsc:DURATION_EQ with datatype xsd:duration."@en .

idsc:DELAY  rdf:type  odrl:LeftOperand ;
        rdfs:label    "delay"@en ;
        rdfs:comment  "Delay the action. Use idsc:DURATION_EQ, idsc:LONGER, idsc:LONGER_EQ, idsc:SHORTER_EQ, or idsc:SHORTER with datatype xsd:duration."@en .

idsc:DATE_TIME  rdf:type  odrl:LeftOperand ;
        rdfs:label    "date time"@en ;
        rdfs:comment  "The date and time of exercising the action of the Rule. Right operand value must be an xsd:dateTimeStamp."@en .

idsc:EVENT  rdf:type  odrl:LeftOperand ;
        rdfs:label    "current event"@en ;
        rdfs:comment  "The feature dimension regarding whether current events are happening. Does NOT refer 'events' as in real-time data, sensor observations, or Complex Event Processing but rather as 'World Cup 2018' or 'Hannover Trade Fair'."@en .

idsc:HASH_ALGORITHM  rdf:type  odrl:LeftOperand ;
        rdfs:label    "hash algorithm"@en ;
        rdfs:comment  "Indicate the hash value to be used, eg.SHA256."@en .

idsc:STATE  rdf:type  odrl:LeftOperand ;
        rdfs:label    "state"@en ;
        rdfs:comment  "Specifies whether an (external) resource is true/false, active/inactive, has happened/not happened, etc. Operator must be idsc:EQUALS with RightOperands of datatype xsd:anyURI. The referenced URI should point to a (remote) resource which returns a xsd:boolean value."@en .

idsc:JSON_PATH  rdf:type  odrl:LeftOperand ;
        rdfs:label    "json path"@en ;
        rdfs:comment  "An expression that refers to a part of a JSON structured data."@en .

idsc:XPATH  rdf:type  odrl:LeftOperand ;
        rdfs:label    "xpath"@en ;
        rdfs:comment  "An expression that refers to specific elements of an XML document."@en .

idsc:REPLACE_WITH  rdf:type  odrl:LeftOperand ;
        rdfs:label    "repace with"@en ;
        rdfs:comment  "Specifies a new value for a specific field. The action must be idsc:REPLACE and the operator must be idsc:EQUALS."@en .

idsc:ABSOLUTE_SPATIAL_POSITION
        rdf:type      odrl:LeftOperand ;
        skos:broader  odrl:absoluteSpatialPosition ;
        rdfs:label    "Absolute geo-spatial position"@en ;
        rdfs:comment  "The current geospatial position of the *consuming connector*. In case the connector only appears as a virtual entity, the physical location of the hosting server is referenced. Allowed operators are idsc:in. No other spatial operators (close to, north of, etc.) are currently allowed."@en .

idsc:OPERAND  rdf:type  odrl:LeftOperand ;
        rdfs:label    "operand"@en ;
        rdfs:comment  "To indicate the second operand value for the Actions idsc:ADD, idsc:MULTIPLY and idsc:DIVIDE."@en .

idsc:USER  rdf:type   odrl:LeftOperand ;
        rdfs:label    "user"@en ;
        rdfs:comment  "The user of a system at the *consuming connector* requesting access to a resource. Recommended usage for checking whether the user's role is sufficient for his/her desired action. Allowed operators are idsc:MEMBER_OF, idsc:HAS_MEMBERSHIP, idsc:HAS_SITE with a RightOperand referencing a (set of) acceptable organisations (ids:Participant),memberships, sites. Preferred behaviour is that the RightOperand dereferences to an endpoint hosting the required role information."@en .

idsc:ROLE  rdf:type   odrl:LeftOperand ;
        rdfs:label    "role"@en ;
        rdfs:comment  "As end user role, not the IDS participant type."@en .

idsc:RECIPIENT  rdf:type  odrl:LeftOperand ;
        rdfs:label    "recipient"@en ;
        rdfs:comment  "For example, the recipient of the notify/inform action."@en .

idsc:PURPOSE  rdf:type  odrl:LeftOperand ;
        skos:broader  odrl:purpose ;
        rdfs:label    "purpose"@en ;
        rdfs:comment  "A defined purpose for exercising the action of the Rule. Use with idsc:IN or idsc:SAME_AS and RDF Resources."@en .

idsc:TARGET_POLICY  rdf:type  odrl:LeftOperand ;
        rdfs:label    "target policy"@en ;
        rdfs:comment  "In order to attach/address a policy to a contract. "@en .

idsc:ARTIFACT_STATE  rdf:type  odrl:LeftOperand ;
        rdfs:label    "artifact state"@en ;
        rdfs:comment  "Suggested values exist in the Information Model : idsc:ANONYMIZED, idsc:PSEUDONYMIZED, idsc:ENCRYPTED, idsc:COMBINED. "@en .

idsc:COUNT  rdf:type  odrl:LeftOperand ;
        skos:broader  odrl:count ;
        rdfs:label    "count"@en ;
        rdfs:comment  "Numeric count of executions of the Rule. Operators can be idsc:LT, idsc:LTEQ, idsc:EQ, idsc:GT, idsc:GTEQ. Datatype is xsd:double."@en .

idsc:QUANTITY  rdf:type  odrl:LeftOperand ;
        rdfs:label    "quantity" ;
        rdfs:comment  "Quantity limitation for exercising the action of the Rule. Operators can be idsc:LT, idsc:LTEQ, idsc:EQ, idsc:GT, idsc:GTEQ. Datatype is xsd:double." .

idsc:RECURRENCE_RATE  rdf:type  odrl:LeftOperand ;
        rdfs:label    "recurrence rate" ;
        rdfs:comment  "The limit how often exercising the action of the Rule may be possible. Operators can be idsc:LT, idsc:LTEQ, idsc:EQ, idsc:GT, idsc:GTEQ. Datatype is xsd:double." .

idsc:SECURITY_LEVEL  rdf:type  odrl:LeftOperand ;
        rdfs:label    "security level" ;
        rdfs:comment  "The security level the consuming connector must have. Use together with idsc:SAME_AS or idsc:IN. The value decides which attribute dimension is regarded."@en .

idsc:SYSTEM  rdf:type  odrl:LeftOperand ;
        rdfs:label    "execution system" ;
        rdfs:comment  "Execution system or execution environment that is used to access the asset under consideration, usually an IDS Connector. The regarded data object should correspond to the IDS Connector class and its attributes. Must be used together with idsc:SAME_AS, idsc:NOT, idsc:HAS_STATE, idsc:IN, idsc:COVERED_BY idsc:INSIDE, idsc:SPATIAL_EQUALS, idsc:DISJOINT, or idsc:INSIDE_NETWORK operators. RightOperandReference must be a URI identifying the target system(s)."@en .

idsc:SYSTEM_DEVICE  rdf:type  odrl:LeftOperand ;
        rdfs:label    "system device" ;
        rdfs:comment  "The ODRL definitions is “An identified computing system or computing device used for exercising the action of the Rule.” "@en .

idsc:ENDPOINT  rdf:type  odrl:LeftOperand ;
        rdfs:label    "endpoint" ;
        rdfs:comment  "Remote target for an action or information provider (PIP). Must be used together with idsc:IS or idsc:IN operators. RightOperand must be a xsd:anyURI or an URL which should point to an actually deployed endpoint. An example is a refinement of idsc:NOTIFY where idsc:REMOTE points to a Clearing House."@en .

idsc:APPLICATION  rdf:type  odrl:LeftOperand ;
        rdfs:label    "application" ;
        rdfs:comment  "An application is a program or piece of software designed to fulfill a particular purpose. For example, a certified IDS App."@en .

idsc:CONNECTOR  rdf:type  odrl:LeftOperand ;
        rdfs:label    "connector" ;
        rdfs:comment  "Accepts an IDS connector URI."@en .

idsc:LOG_LEVEL  rdf:type  odrl:LeftOperand ;
        rdfs:label    "log level" ;
        rdfs:comment  "Accepted values: ON_DENY, ON_ALLOW, ON_DUTY_EXERCISED, ON_ACTION_OPERATED."@en .

idsc:NOTIFICATION_LEVEL
        rdf:type      odrl:LeftOperand ;
        rdfs:label    "notification level" ;
        rdfs:comment  "Similar to the idsc:LOG_LEVEL."@en .

idsc:PATH  rdf:type   odrl:LeftOperand ;
        rdfs:label    "path to attribute" ;
        rdfs:comment  "Path to specific attribute (default JsonPath). Must be used together with idsc:STRING_EQ, idsc:STRING_CONTAINS, idsc:STRING_IS_CONTAINED, or idsc:MATCHES operators. RightOperand must be a xsd:string."@en .
@prefix owl:   <http://www.w3.org/2002/07/owl#> .
@prefix rdfs:  <http://www.w3.org/2000/01/rdf-schema#> .
@prefix ids:   <https://w3id.org/idsa/core/> .
@prefix idsc:  <https://w3id.org/idsa/code/> .

idsc:NO_LOGGING  rdf:type  ids:LogLevel ;
        rdfs:label    "No Logging"@en ;
        rdfs:comment  "No logging."@en .

idsc:MINIMAL_LOGGING  rdf:type  ids:LogLevel ;
        rdfs:label    "Minimal Logging"@en ;
        rdfs:comment  "Minimal logging."@en .

idsc:DEBUG_LEVEL_LOGGING
        rdf:type      ids:LogLevel ;
        rdfs:label    "Debug Level Logging"@en ;
        rdfs:comment  "Debug level logging."@en .
@prefix owl:   <http://www.w3.org/2002/07/owl#> .
@prefix rdfs:  <http://www.w3.org/2000/01/rdf-schema#> .
@prefix ids:   <https://w3id.org/idsa/core/> .
@prefix idsc:  <https://w3id.org/idsa/code/> .
@prefix owl:   <http://www.w3.org/2002/07/owl#> .
@prefix rdfs:  <http://www.w3.org/2000/01/rdf-schema#> .
@prefix dct:   <http://purl.org/dc/terms/> .
@prefix xsd:   <http://www.w3.org/2001/XMLSchema#> .
@prefix ids:   <https://w3id.org/idsa/core/> .
@prefix idsc:  <https://w3id.org/idsa/code/> .

idsc:FREE  rdf:type   ids:PaymentModality ;
        rdfs:comment  "To express that the exchange of resource is free"@en ;
        rdfs:label    "free"@en .

idsc:FIXED_PRICE  rdf:type  ids:PaymentModality ;
        rdfs:comment  "To express that the exchange of resource is with a fixed price"@en ;
        rdfs:label    "fixed price"@en .

idsc:NEGOTIATION_BASIS
        rdf:type      ids:PaymentModality ;
        rdfs:comment  "To express that the exchange of resource is negotiation-based."@en ;
        rdfs:label    "negotiation basis"@en .
@prefix owl:   <http://www.w3.org/2002/07/owl#> .
@prefix rdfs:  <http://www.w3.org/2000/01/rdf-schema#> .
@prefix dct:   <http://purl.org/dc/terms/> .
@prefix ids:   <https://w3id.org/idsa/core/> .
@prefix idsc:  <https://w3id.org/idsa/code/> .

idsc:SPARQL  rdf:type  ids:QueryLanguage ;
        rdfs:label  "SPARQL" .

idsc:SQL  rdf:type  ids:QueryLanguage ;
        rdfs:label  "SQL" .

idsc:XQUERY  rdf:type  ids:QueryLanguage ;
        rdfs:label  "XQUERY" .
@prefix owl:   <http://www.w3.org/2002/07/owl#> .
@prefix rdfs:  <http://www.w3.org/2000/01/rdf-schema#> .
@prefix dct:   <http://purl.org/dc/terms/> .
@prefix ids:   <https://w3id.org/idsa/core/> .
@prefix idsc:  <https://w3id.org/idsa/code/> .

idsc:ALL  rdf:type  ids:QueryScope ;
        rdfs:label  "ALL" .

idsc:ACTIVE_ONLY  rdf:type  ids:QueryScope ;
        rdfs:label  "ACTIVE_ONLY" .

idsc:INACTIVE_ONLY  rdf:type  ids:QueryScope ;
        rdfs:label  "INACTIVE_ONLY" .
@prefix owl:   <http://www.w3.org/2002/07/owl#> .
@prefix rdfs:  <http://www.w3.org/2000/01/rdf-schema#> .
@prefix dct:   <http://purl.org/dc/terms/> .
@prefix ids:   <https://w3id.org/idsa/core/> .
@prefix idsc:  <https://w3id.org/idsa/code/> .
@prefix skos:  <http://www.w3.org/2004/02/skos/core#> .

idsc:BROKER  rdf:type  ids:QueryTarget ;
        rdfs:label  "BROKER" .

idsc:APPSTORE  rdf:type  ids:QueryTarget ;
        rdfs:label  "APPSTORE" .

idsc:PARIS  rdf:type  ids:QueryTarget ;
        rdfs:label  "PARTICIPANT INFORMATION SERVICE" .

idsc:CLEARING_HOUSE  rdf:type  ids:QueryTarget ;
        rdfs:label  "CLEARING_HOUSE" .

idsc:ANY  rdf:type  ids:QueryTarget ;
        rdfs:label  "ANY" .
@prefix owl:   <http://www.w3.org/2002/07/owl#> .
@prefix rdfs:  <http://www.w3.org/2000/01/rdf-schema#> .
@prefix dct:   <http://purl.org/dc/terms/> .
@prefix ids:   <https://w3id.org/idsa/core/> .
@prefix idsc:  <https://w3id.org/idsa/code/> .

idsc:NOT_FOUND  rdf:type  ids:RejectionReason ;
        rdfs:label    "NOT_FOUND" ;
        rdfs:comment  "Requested Resource was not found." .

idsc:NOT_AUTHENTICATED
        rdf:type      ids:RejectionReason ;
        rdfs:label    "NOT_AUTHENTICATED" ;
        rdfs:comment  "Authenticity of a message sender has failed or is not verifiable." .

idsc:NOT_AUTHORIZED  rdf:type  ids:RejectionReason ;
        rdfs:label    "NOT_AUTHORIZED" ;
        rdfs:comment  "Sender is not authorized to initiate the command." .

idsc:TOO_MANY_RESULTS
        rdf:type      ids:RejectionReason ;
        rdfs:label    "TOO_MANY_RESULTS" ;
        rdfs:comment  "Processing of the command would lead to too many results (computational or bandwidth limitations)" .

idsc:MALFORMED_MESSAGE
        rdf:type      ids:RejectionReason ;
        rdfs:label    "MALFORMED_MESSAGE" ;
        rdfs:comment  "The originating message is malformed or missing information." .

idsc:INTERNAL_RECIPIENT_ERROR
        rdf:type      ids:RejectionReason ;
        rdfs:label    "INTERNAL_RECIPIENT_ERROR" ;
        rdfs:comment  "The message recipient encountered an internal error while processing the message (e.g., storage capacity exceeded)." .

idsc:METHOD_NOT_SUPPORTED
        rdf:type      ids:RejectionReason ;
        rdfs:label    "METHOD_NOT_SUPPORTED" ;
        rdfs:comment  "The sender of the rejection does not implement a certain functionality stated in the message (e.g., query language)." .

idsc:MESSAGE_TYPE_NOT_SUPPORTED
        rdf:type      ids:RejectionReason ;
        rdfs:label    "MESSAGE_TYPE_NOT_SUPPORTED" ;
        rdfs:comment  "The sender of the rejection does not support the incoming message type (e.g., ids:QueryMessage)." .

idsc:VERSION_NOT_SUPPORTED
        rdf:type      ids:RejectionReason ;
        rdfs:label    "VERSION_NOT_SUPPORTED" ;
        rdfs:comment  "The version of the information model against which the referenced message should be interpreted, is not supported by the recipient." .

idsc:BAD_PARAMETERS  rdf:type  ids:RejectionReason ;
        rdfs:label    "BAD_PARAMETERS" ;
        rdfs:comment  "At least one query or operation parameter is not acceptable for the sender of this rejection message." .

idsc:TEMPORARILY_NOT_AVAILABLE
        rdf:type      ids:RejectionReason ;
        rdfs:label    "TEMPORARILY_NOT_AVAILABLE" ;
        rdfs:comment  "The requested resource, representation or artifact is temporarily not available but might be back later." .
@prefix rdf:   <http://www.w3.org/1999/02/22-rdf-syntax-ns#> .
@prefix rdfs:  <http://www.w3.org/2000/01/rdf-schema#> .
@prefix owl:   <http://www.w3.org/2002/07/owl#> .
@prefix dct:   <http://purl.org/dc/terms/> .
@prefix xsd:   <http://www.w3.org/2001/XMLSchema#> .
@prefix skos:  <http://www.w3.org/2004/02/skos/core#> .
@prefix ids:   <https://w3id.org/idsa/core/> .
@prefix idsc:  <https://w3id.org/idsa/code/> .
@prefix odrl:  <http://www.w3.org/ns/odrl/2/> .

idsc:RequestTemplate  rdf:type  ids:PolicyTemplate ;
        rdfs:label    "Policy Request Template" ;
        rdfs:comment  "A generic template for policy requests with one permission and several constraints" ;
        skos:note     "The <Consumer Participant URI> asks <Provider Participant URI> to [ids:use|ids:read|...] \n\t\tits [<Representation URI>|<Artifact URI>].\n\t\tOptional: This only holds if <Attribute URI> is [equal|lower than|greater than] the [<Value URI>|<Value Literal>].\n\t\tOptional: This only holds if also <Attribute URI> is [equal|lower than|greater than] the [<Value URI>|<Value Literal>]."@en ;
        skos:note     "{ \n\t\t\"@context\": \"https://w3id.org/idsa/contexts/context.jsonld\",\n\t\t\"@type\": \"ContractRequest\", \n\t\t\"uid\": \"<contract ID>\", \n\t\t\"refersTo\": \"idsc:RequestTemplate\" ,\n\t\t\"target\": \"[<Representation URI>|<Artifact URI>]\",\n\t\t\"ids:provider\": \"<Provider Participant URI>\",\n\t\t\"ids:consumer\": \"<Consumer Participant URI>\", \n\t\t\"odrl:permission\": {\n\t\t\t\"odrl:action\": \"[ids:use|ids:read|...]\" ,\n\t\t\t[\"odrl:constraint\" : {    \n\t\t\t\t\t \"odrl:leftOperand\" : \"<Attribute URI>\",\n\t\t\t\t\t \"odrl:operator\" : \"[ids:eq|ids:lt|ids:gt]\",\n\t\t\t\t\t \"odrl:rightOperand\" : \"[<Value URI>|<Value Literal>]\"\n\t\t\t } [,]]*\n\t\t} }" ;
        skos:note     "@prefix ids: <https://w3id.org/idsa/core/> .\n\t\t@prefix idsc: <https://w3id.org/idsa/code/> .\n\t\t@prefix rdf: <http://www.w3.org/1999/02/22-rdf-syntax-ns#> .\n\t\t@prefix rdfs: <http://www.w3.org/2000/01/rdf-schema#> .\n\t\t@prefix xsd: <http://www.w3.org/2001/XMLSchema#> .\n\n\t\t[<contract URI>| [] ] a ids:ContractRequest ;\n\t\t\tids:uid <contract ID> ;\n\t\t\tids:refersTo idsc:RequestTemplate ;\n\t\t\tids:target [<Representation URI>|<Artifact URI>] ;\n\t\t\tids:consumer <Consumer Participant URI> ;\n\t\t\tids:provider <Provider Participant URI>\n\t\t\t[odrl:permission[\n\t\t\t\todrl:action ids:[use|read|...] ;\n\t\t\t\todrl:constraint [\n\t\t\t\t\todrl:leftOperand <Attribute URI> ;\n\t\t\t\t\todrl:operator [ids:eq|ids:lt|ids:gt] ;\n\t\t\t\t\todrl:rightOperand [<Value URI>|<Value Literal>]\n\t\t\t\t]\n\t\t\t] ;]*\n\t\t." .
@prefix owl:   <http://www.w3.org/2002/07/owl#> .
@prefix rdfs:  <http://www.w3.org/2000/01/rdf-schema#> .
@prefix dct:   <http://purl.org/dc/terms/> .
@prefix xsd:   <http://www.w3.org/2001/XMLSchema#> .
@prefix ids:   <https://w3id.org/idsa/core/> .
@prefix idsc:  <https://w3id.org/idsa/code/> .

ids:IntegrityGuarantee
        rdf:type         owl:Class ;
        rdfs:subClassOf  ids:SecurityGuarantee ;
        rdfs:label       "Integrity protection and verification"@en ;
        rdfs:comment     "Level of integrity protection and verification of the installed software stack. Trusted boot is an example of local integrity protection, remote integrity verification comprises, for example, remote attestation."@en .

_:b9    rdf:first  idsc:INTEGRITY_PROTECTION_NONE ;
        rdf:rest   _:b10 .

_:b10   rdf:first  idsc:INTEGRITY_PROTECTION_LOCAL ;
        rdf:rest   _:b11 .

_:b11   rdf:first  idsc:INTEGRITY_VERIFICATION_REMOTE ;
        rdf:rest   rdf:nil .

ids:IntegrityGuarantee
        owl:oneOf  _:b9 .

idsc:INTEGRITY_PROTECTION_NONE
        rdf:type    ids:IntegrityGuarantee ;
        rdfs:label  "Integrity Protection None" .

idsc:INTEGRITY_PROTECTION_LOCAL
        rdf:type    ids:IntegrityGuarantee ;
        rdfs:label  "Integrity Protection Local" .

idsc:INTEGRITY_VERIFICATION_REMOTE
        rdf:type    ids:IntegrityGuarantee ;
        rdfs:label  "Integrity Protection Remote" .

ids:IntegrityVerificationScopeGuarantee
        rdf:type         owl:Class ;
        rdfs:subClassOf  ids:SecurityGuarantee ;
        rdfs:label       "Integrity verification scope"@en ;
        rdfs:comment     "Level/extent of verifying the software stack."@en .

_:b12   rdf:first  idsc:INTEGRITY_VERIFICATION_SCOPE_NONE ;
        rdf:rest   _:b13 .

_:b13   rdf:first  idsc:INTEGRITY_VERIFICATION_SCOPE_KERNEL_CORE_CONTAINER ;
        rdf:rest   _:b14 .

_:b14   rdf:first  idsc:INTEGRITY_VERIFICATION_SCOPE_KERNEL_CORE_CONTAINER_APPLICATION ;
        rdf:rest   rdf:nil .

ids:IntegrityVerificationScopeGuarantee
        owl:oneOf  _:b12 .

idsc:INTEGRITY_VERIFICATION_SCOPE_NONE
        rdf:type    ids:IntegrityVerificationScopeGuarantee ;
        rdfs:label  "Integrity Verification Scope None" .

idsc:INTEGRITY_VERIFICATION_SCOPE_KERNEL_CORE_CONTAINER
        rdf:type    ids:IntegrityVerificationScopeGuarantee ;
        rdfs:label  "Integrity Verification Scope Kernel Core Container" .

idsc:INTEGRITY_VERIFICATION_SCOPE_KERNEL_CORE_CONTAINER_APPLICATION
        rdf:type    ids:IntegrityVerificationScopeGuarantee ;
        rdfs:label  "Integrity Verification Scope Kernel Core Container Application" .

ids:AuthenticationGuarantee
        rdf:type         owl:Class ;
        rdfs:subClassOf  ids:SecurityGuarantee ;
        rdfs:label       "Authentication"@en ;
        rdfs:comment     "Authentication mechanism applied prior to opening a connection. Examples are the verification server's identity or doing mutual authentication."@en .

_:b15   rdf:first  idsc:AUTHENTICATION_NONE ;
        rdf:rest   _:b16 .

_:b16   rdf:first  idsc:AUTHENTICATION_SERVER_SIDE ;
        rdf:rest   _:b17 .

_:b17   rdf:first  idsc:AUTHENTICATION_MUTUAL ;
        rdf:rest   rdf:nil .

ids:AuthenticationGuarantee
        owl:oneOf  _:b15 .

idsc:AUTHENTICATION_NONE
        rdf:type    ids:AuthenticationGuarantee ;
        rdfs:label  "Authentication None" .

idsc:AUTHENTICATION_SERVER_SIDE
        rdf:type    ids:AuthenticationGuarantee ;
        rdfs:label  "Authentication Serverside" .

idsc:AUTHENTICATION_MUTUAL
        rdf:type    ids:AuthenticationGuarantee ;
        rdfs:label  "Authentication Mutual" .

ids:ServiceIsolationGuarantee
        rdf:type         owl:Class ;
        rdfs:subClassOf  ids:SecurityGuarantee ;
        rdfs:label       "Service isolation"@en ;
        rdfs:comment     "Service isolation mechanism supported by the Connector. Examples are process group (Docker) or by least privilege with clear separation and support for additional security modules as done by trustme."@en .

_:b18   rdf:first  idsc:SERVICE_ISOLATION_NONE ;
        rdf:rest   _:b19 .

_:b19   rdf:first  idsc:SERVICE_ISOLATION_PROCESS_GROUP ;
        rdf:rest   _:b20 .

_:b20   rdf:first  idsc:SERVICE_ISOLATION_LEAST_PRIVILEGE ;
        rdf:rest   rdf:nil .

ids:ServiceIsolationGuarantee
        owl:oneOf  _:b18 .

idsc:SERVICE_ISOLATION_NONE
        rdf:type    ids:ServiceIsolationGuarantee ;
        rdfs:label  "Service Isolation None" .

idsc:SERVICE_ISOLATION_PROCESS_GROUP
        rdf:type    ids:ServiceIsolationGuarantee ;
        rdfs:label  "Service Isolation Process Group" .

idsc:SERVICE_ISOLATION_LEAST_PRIVILEGE
        rdf:type    ids:ServiceIsolationGuarantee ;
        rdfs:label  "Service Isolation Least Privilege" .

ids:AppExecutionResources
        rdf:type         owl:Class ;
        rdfs:subClassOf  ids:SecurityGuarantee ;
        rdfs:label       "App execution resources"@en ;
        rdfs:comment     "Resource control for deployed services."@en .

_:b21   rdf:first  idsc:APP_RESOURCES_NONE ;
        rdf:rest   _:b22 .

_:b22   rdf:first  idsc:APP_RESOURCES_LOCAL_ENFORCEMENT ;
        rdf:rest   _:b23 .

_:b23   rdf:first  idsc:APP_RESOURCES_REMOTE_VERIFICATION ;
        rdf:rest   rdf:nil .

ids:AppExecutionResources
        owl:oneOf  _:b21 .

idsc:APP_RESOURCES_NONE
        rdf:type    ids:AppExecutionResources ;
        rdfs:label  "App Resources None" .

idsc:APP_RESOURCES_LOCAL_ENFORCEMENT
        rdf:type    ids:AppExecutionResources ;
        rdfs:label  "App Resources Local Enforcement" .

idsc:APP_RESOURCES_REMOTE_VERIFICATION
        rdf:type    ids:AppExecutionResources ;
        rdfs:label  "App Resources Remote Verification" .

ids:UsageControlGuarantee
        rdf:type         owl:Class ;
        rdfs:subClassOf  ids:SecurityGuarantee ;
        rdfs:label       "Usage control"@en ;
        rdfs:comment     "Extent of supporting usage control."@en .

_:b24   rdf:first  idsc:USAGE_CONTROL_NONE ;
        rdf:rest   _:b25 .

_:b25   rdf:first  idsc:USAGE_CONTROL_POLICY_ENFORCEMENT ;
        rdf:rest   _:b26 .

_:b26   rdf:first  idsc:USAGE_CONTROL_REMOTE_COMPLIANCE_VERIFICATION ;
        rdf:rest   rdf:nil .

ids:UsageControlGuarantee
        owl:oneOf  _:b24 .

idsc:USAGE_CONTROL_NONE
        rdf:type    ids:UsageControlGuarantee ;
        rdfs:label  "Usage Control None" .

idsc:USAGE_CONTROL_POLICY_ENFORCEMENT
        rdf:type    ids:UsageControlGuarantee ;
        rdfs:label  "Usage Control Policy Enforcement" .

idsc:USAGE_CONTROL_REMOTE_COMPLIANCE_VERIFICATION
        rdf:type    ids:UsageControlGuarantee ;
        rdfs:label  "Usage Control Remote Compliance Verification" .

ids:AuditGuarantee  rdf:type  owl:Class ;
        rdfs:subClassOf  ids:SecurityGuarantee ;
        rdfs:label       "Audit guarantee"@en ;
        rdfs:comment     "Local audit logging (including integrity protection) is the baseline for auditing and clearing. Remote audit log tracing provides means to do external audit verification."@en .

_:b27   rdf:first  idsc:AUDIT_NONE ;
        rdf:rest   _:b28 .

_:b28   rdf:first  idsc:AUDIT_LOCAL_LOGGING ;
        rdf:rest   _:b29 .

_:b29   rdf:first  idsc:AUDIT_REMOTE_TRACING ;
        rdf:rest   rdf:nil .

ids:AuditGuarantee  owl:oneOf  _:b27 .

idsc:AUDIT_NONE  rdf:type  ids:AuditGuarantee ;
        rdfs:label  "Audit None" .

idsc:AUDIT_LOCAL_LOGGING
        rdf:type    ids:AuditGuarantee ;
        rdfs:label  "Audit Local Logging" .

idsc:AUDIT_REMOTE_TRACING
        rdf:type    ids:AuditGuarantee ;
        rdfs:label  "Audit Remote Tracing" .

ids:LocalDataConfidentialityGuarantee
        rdf:type         owl:Class ;
        rdfs:subClassOf  ids:SecurityGuarantee ;
        rdfs:label       "Local data confidentiality"@en ;
        rdfs:comment     "Means by which local data is protected."@en .

_:b30   rdf:first  idsc:LOCAL_DATA_CONFIDENTIALITY_NONE ;
        rdf:rest   _:b31 .

_:b31   rdf:first  idsc:LOCAL_DATA_CONFIDENTIALITY_SECURE_ERASURE ;
        rdf:rest   _:b32 .

_:b32   rdf:first  idsc:LOCAL_DATA_CONFIDENTIALITY_FULL_ENCRYPTION ;
        rdf:rest   rdf:nil .

ids:LocalDataConfidentialityGuarantee
        owl:oneOf  _:b30 .

idsc:LOCAL_DATA_CONFIDENTIALITY_NONE
        rdf:type    ids:LocalDataConfidentialityGuarantee ;
        rdfs:label  "Local Data Confidentiality None" .

idsc:LOCAL_DATA_CONFIDENTIALITY_SECURE_ERASURE
        rdf:type    ids:LocalDataConfidentialityGuarantee ;
        rdfs:label  "Local Data Confidentiality Secure Erasure" .

idsc:LOCAL_DATA_CONFIDENTIALITY_FULL_ENCRYPTION
        rdf:type    ids:LocalDataConfidentialityGuarantee ;
        rdfs:label  "Local Data Confidentiality Full Encryption" .

idsc:BASE_SECURITY_PROFILE
        rdf:type               ids:SecurityProfile ;
        rdfs:label             "Base security profile"@en ;
        rdfs:comment           "Default security profile of a certified IDS Connector."@en ;
        ids:securityGuarantee  idsc:INTEGRITY_PROTECTION_NONE ;
        ids:securityGuarantee  idsc:INTEGRITY_VERIFICATION_SCOPE_NONE ;
        ids:securityGuarantee  idsc:APP_RESOURCES_NONE ;
        ids:securityGuarantee  idsc:USAGE_CONTROL_NONE ;
        ids:securityGuarantee  idsc:LOCAL_DATA_CONFIDENTIALITY_NONE ;
        ids:securityGuarantee  idsc:AUTHENTICATION_MUTUAL ;
        ids:securityGuarantee  idsc:SERVICE_ISOLATION_PROCESS_GROUP ;
        ids:securityGuarantee  idsc:AUDIT_LOCAL_LOGGING .

idsc:TRUST_SECURITY_PROFILE
        rdf:type               ids:SecurityProfile ;
        rdfs:label             "Trust security profile"@en ;
        rdfs:comment           "The Security Profile TRUST as defined by the IDS certification criteria."@en ;
        ids:securityGuarantee  idsc:INTEGRITY_VERIFICATION_REMOTE ;
        ids:securityGuarantee  idsc:AUTHENTICATION_MUTUAL ;
        ids:securityGuarantee  idsc:SERVICE_ISOLATION_LEAST_PRIVILEGE ;
        ids:securityGuarantee  idsc:INTEGRITY_VERIFICATION_SCOPE_KERNEL_CORE_CONTAINER ;
        ids:securityGuarantee  idsc:APP_RESOURCES_LOCAL_ENFORCEMENT ;
        ids:securityGuarantee  idsc:USAGE_CONTROL_POLICY_ENFORCEMENT ;
        ids:securityGuarantee  idsc:AUDIT_LOCAL_LOGGING ;
        ids:securityGuarantee  idsc:LOCAL_DATA_CONFIDENTIALITY_FULL_ENCRYPTION .

idsc:TRUST_PLUS_SECURITY_PROFILE
        rdf:type               ids:SecurityProfile ;
        rdfs:label             "Trust Plus security profile"@en ;
        rdfs:comment           "The Security Profile TRUST+ as defined by the IDS certification criteria."@en ;
        ids:securityGuarantee  idsc:INTEGRITY_VERIFICATION_REMOTE ;
        ids:securityGuarantee  idsc:AUTHENTICATION_MUTUAL ;
        ids:securityGuarantee  idsc:SERVICE_ISOLATION_LEAST_PRIVILEGE ;
        ids:securityGuarantee  idsc:INTEGRITY_VERIFICATION_SCOPE_KERNEL_CORE_CONTAINER_APPLICATION ;
        ids:securityGuarantee  idsc:APP_RESOURCES_REMOTE_VERIFICATION ;
        ids:securityGuarantee  idsc:USAGE_CONTROL_REMOTE_COMPLIANCE_VERIFICATION ;
        ids:securityGuarantee  idsc:AUDIT_REMOTE_TRACING ;
        ids:securityGuarantee  idsc:LOCAL_DATA_CONFIDENTIALITY_FULL_ENCRYPTION .
@prefix rdf:   <http://www.w3.org/1999/02/22-rdf-syntax-ns#> .
@prefix rdfs:  <http://www.w3.org/2000/01/rdf-schema#> .
@prefix owl:   <http://www.w3.org/2002/07/owl#> .
@prefix dct:   <http://purl.org/dc/terms/> .
@prefix ids:   <https://w3id.org/idsa/core/> .
@prefix idsc:  <https://w3id.org/idsa/code/> .

idsc:JWT  rdf:type  ids:TokenFormat ;
        rdfs:label  "Json Web Token" .

idsc:SWT  rdf:type  ids:TokenFormat ;
        rdfs:label  "Simple Web Token" .

idsc:SAML_1_1  rdf:type  ids:TokenFormat ;
        rdfs:label  "Security Assertion Markup Language (SAML) 1.1" .

idsc:SAML_2_0  rdf:type  ids:TokenFormat ;
        rdfs:label  "Security Assertion Markup Language (SAML) 2.0" .

idsc:OTHER  rdf:type  ids:TokenFormat ;
        rdfs:label  "Other" .

idsc:UNKNOWN  rdf:type  ids:TokenFormat ;
        rdfs:label  "Unknown" .
@prefix owl:   <http://www.w3.org/2002/07/owl#> .
@prefix rdfs:  <http://www.w3.org/2000/01/rdf-schema#> .
@prefix ids:   <https://w3id.org/idsa/core/> .
@prefix idsc:  <https://w3id.org/idsa/code/> .

idsc:ALLOW_DATA_USAGE
        rdf:type      ids:UsagePolicyClass ;
        rdfs:label    "Allow data usage"@en ;
        rdfs:comment  "This policy restricts the usage of the data to a specific Data Consumer, regardless of how many connectors they have and without any further usage restriction."@en .

idsc:CONNECTOR_RESTRICTED_DATA_USAGE
        rdf:type      ids:UsagePolicyClass ;
        rdfs:label    "Connector restricted data usage"@en ;
        rdfs:comment  "This policy restrict the usage of the data to a specific IDS connector."@en .

idsc:APPLICATION_RESTRICTED_DATA_USAGE
        rdf:type      ids:UsagePolicyClass ;
        rdfs:label    "System restricted data usage"@en ;
        rdfs:comment  "This policy restricts the usage of the data to a specific system or application inside an IDS Connector."@en .

idsc:INTERVAL_RESTRICTED_DATA_USAGE
        rdf:type      ids:UsagePolicyClass ;
        rdfs:label    "Interval restricted data usage"@en ;
        rdfs:comment  "This policy restricts the usage of the data to a specific (time) interval."@en .

idsc:DURATION_RESTRICTED_DATA_USAGE
        rdf:type      ids:UsagePolicyClass ;
        rdfs:label    "Duration restricted data usage"@en ;
        rdfs:comment  "This policy restricts the usage of the data to a specific duration."@en .

idsc:LOCATION_RESTRICTED_DATA_USAGE
        rdf:type      ids:UsagePolicyClass ;
        rdfs:label    "Location restricted data usage"@en ;
        rdfs:comment  "This policy restricts the usage of the data to a specific location, e.g., expressed via location areas, geographic points or geographic bounding polygons."@en .

idsc:PREPATUAL_DATA_SALE
        rdf:type      ids:UsagePolicyClass ;
        rdfs:label    "Prepatual data sale"@en ;
        rdfs:comment  "This policy restricts the transfer of a Data Asset against a one-off payment in a given currency."@en .

idsc:DATA_RENTAL  rdf:type  ids:UsagePolicyClass ;
        rdfs:label    "Data rental"@en ;
        rdfs:comment  "This policy restricts transfer of data in return for a monthly fee. The ending is not specified. Nevertheless, the policy ends when a notice of termination has been made by any of the policy partners."@en .

idsc:ROLE_RESTRICTED_DATA_USAGE
        rdf:type      ids:UsagePolicyClass ;
        rdfs:label    "Role restricted data usage"@en ;
        rdfs:comment  "This policy restricts the usage of the data to a specific role. \n\t\t\t\t\tFor example, you can instantiate a policy of this class that allows only the members of the engineering department to use your data. \n\t\t\t\t\tThis policy class faces few limitations, i.e., in order to evaluate the conditions, it requires that the user roles are available and follow a common vocabulary"@en .

idsc:PURPOSE_RESTRICTED_DATA_USAGE
        rdf:type      ids:UsagePolicyClass ;
        rdfs:label    "Purpose restricted data usage"@en ;
        rdfs:comment  "This policy restricts the usage of data assets limited to specific purposes."@en .

idsc:EVENT_RESTRICTED_DATA_USAGE
        rdf:type      ids:UsagePolicyClass ;
        rdfs:label    "Event restricted data usage"@en ;
        rdfs:comment  "This policy restricts the usage of data assets limited to specific events.\n\t\t\t\t\tThe ODRL language defines an identified event as a context for exercising the action of the Rule. \n\t\t\t\t\tEvents are temporal periods of time. A Data Provider may want to restrict the usage of the data to a specific event when the exact time and date of the event is not clear in advance. \n\t\t\t\t\tTherefore, the event condition can be specified in a policy."@en .

idsc:RESTRICTED_NUMBER_OF_USAGES
        rdf:type      ids:UsagePolicyClass ;
        rdfs:label    "Restricted number of usages"@en ;
        rdfs:comment  "This policy restricts the usage of data assets limited to numeric count of executions of actions. \n\t\t\t\t\tA mechanism is needed that counts the usage of data in order to enforce the policy."@en .

idsc:SECURITY_LEVEL_RESTRICTED_POLICY
        rdf:type      ids:UsagePolicyClass ;
        rdfs:label    "Security level restricted policy"@en ;
        rdfs:comment  "This policy restricts the usage of data assets limited to a security level the consumer must conform to."@en .

idsc:USE_DATA_AND_DELETE_AFTER
        rdf:type      ids:UsagePolicyClass ;
        rdfs:label    "Use data and delete after"@en ;
        rdfs:comment  "This policy restricts the usage of data assets with the obligation to delete the asset after usage."@en .

idsc:MODIFY_DATA_IN_TRANSIT
        rdf:type      ids:UsagePolicyClass ;
        rdfs:label    "Modfy data in transit"@en ;
        rdfs:comment  "This policy restricts the usage of data assets with the obligation to anonymize the data when it is leaving the Data Provider connector or when it is entering the Data Consumer connector"@en .

idsc:MODIFY_DATA_IN_REST
        rdf:type      ids:UsagePolicyClass ;
        rdfs:label    "Modfy data in rest"@en ;
        rdfs:comment  "This policy restricts the usage of data assets with the obligation to anonymize the data before permission to use the data is granted. \n\t\t\t\t\tIn contrast to the idsc:MODIFY_DATA_IN_TRANSIT policy class, it demands the modifications to be done when data is stored."@en .

idsc:LOCAL_LOGGING  rdf:type  ids:UsagePolicyClass ;
        rdfs:label    "Local logging"@en ;
        rdfs:comment  "This policy restricts the usage of data assets with the obligation to log prior specified processes, such as the data access."@en .

idsc:REMOTE_NOTIFICATION
        rdf:type      ids:UsagePolicyClass ;
        rdfs:label    "Remote notification"@en ;
        rdfs:comment  "This policy restricts the usage of data assets with the obligation to notify a specific party about the data usage."@en .

idsc:ATTACH_POLICY_FOR_THIRD_PARTY
        rdf:type      ids:UsagePolicyClass ;
        rdfs:label    "Remote notification"@en ;
        rdfs:comment  "This policy restricts the usage of data assets with the obligation to notify a specific party about the data usage."@en .

idsc:DISTRIBUTE_ONLY_IF_ENCRYPTED
        rdf:type      ids:UsagePolicyClass ;
        rdfs:label    "Distribute only if encrypted"@en ;
        rdfs:comment  "This policy restricts the usage of data assets with the obligation to encrypt the data asset before distribution."@en .

idsc:STATE_RESTRICTED_POLICY
        rdf:type      ids:UsagePolicyClass ;
        rdfs:label    "State restricted policy"@en ;
        rdfs:comment  "This policy restricts the usage of data assets limited to specific states. Possible states include, for example, that the contract for the given data asset has not yet expired."@en .
@prefix owl:   <http://www.w3.org/2002/07/owl#> .
@prefix rdfs:  <http://www.w3.org/2000/01/rdf-schema#> .
@prefix ids:   <https://w3id.org/idsa/core/> .
@prefix xsd:   <http://www.w3.org/2001/XMLSchema#> .

ids:ParticipantCertificationLevel
        rdf:type         owl:Class ;
        rdfs:subClassOf  ids:CertificationLevel ;
        rdfs:label       "Participant Certification Level"@en ;
        rdfs:comment     "Level of a Participant Certification"@en .

ids:ComponentCertificationLevel
        rdf:type          owl:Class ;
        rdfs:subClassOf   ids:CertificationLevel ;
        owl:disjointWith  ids:ParticipantCertificationLevel ;
        rdfs:label        "Component Certification Level"@en ;
        rdfs:comment      "Level of a Component Certification"@en .

ids:ParticipantCertification
        rdf:type         owl:Class ;
        rdfs:subClassOf  ids:Certification .

_:b33   rdf:type           owl:Restriction ;
        owl:onProperty     ids:certificationLevel ;
        owl:allValuesFrom  ids:ParticipantCertificationLevel .

ids:ParticipantCertification
        rdfs:subClassOf  _:b33 ;
        rdfs:label       "Participant Certification"@en ;
        rdfs:comment     "Process and result of certifying an interested party in order to become a certified member of the International Data Space."@en .

ids:ComponentCertification
        rdf:type         owl:Class ;
        rdfs:subClassOf  ids:Certification .

_:b34   rdf:type           owl:Restriction ;
        owl:onProperty     ids:certificationLevel ;
        owl:allValuesFrom  ids:ComponentCertificationLevel .

ids:ComponentCertification
        rdfs:subClassOf   _:b34 ;
        owl:disjointWith  ids:ParticipantCertification ;
        rdfs:label        "Component Certification"@en ;
        rdfs:comment      "Process and result of certifying a software component/servivce in order to become a certified part of the International Data Space infrastructure."@en .

ids:membershipEnd  rdf:type  owl:DatatypeProperty ;
        rdfs:label    "membership end"@en ;
        rdfs:domain   ids:ParticipantCertification ;
        rdfs:range    xsd:dateTimeStamp ;
        rdfs:comment  "End of the participant's IDS membership."@en .
@prefix owl:   <http://www.w3.org/2002/07/owl#> .
@prefix rdfs:  <http://www.w3.org/2000/01/rdf-schema#> .
@prefix dct:   <http://purl.org/dc/terms/> .
@prefix xsd:   <http://www.w3.org/2001/XMLSchema#> .
@prefix odrl:  <http://www.w3.org/ns/odrl/2/> .
@prefix rdf:   <http://www.w3.org/1999/02/22-rdf-syntax-ns#> .
@prefix ids:   <https://w3id.org/idsa/core/> .

ids:SalesAgreement  rdf:type  owl:Class ;
        rdfs:subClassOf  ids:ContractAgreement ;
        rdfs:label       "Sales Agreement"@en ;
        rdfs:comment     "The ContractAgreement class representing the Perpetual Data Sale policy class."@en .

ids:PurposeAgreement  rdf:type  owl:Class ;
        rdfs:subClassOf  ids:ContractAgreement ;
        rdfs:label       "Purpose Agreement"@en ;
        rdfs:comment     "The ContractAgreement class representing the 'Purpose-restricted Data Usage' policy class."@en .

ids:SecurityAgreement
        rdf:type         owl:Class ;
        rdfs:subClassOf  ids:ContractAgreement ;
        rdfs:label       "Security Agreement"@en ;
        rdfs:comment     "The ContractAgreement class representing the 'Security Level Restricted Policy' policy class."@en .

ids:NotMoreThanNAgreement
        rdf:type         owl:Class ;
        rdfs:subClassOf  ids:ContractAgreement ;
        rdfs:label       "Use Not More Than N Times Agreement"@en ;
        rdfs:comment     "The ContractAgreement class representing the 'Restricted Number of Usages' policy class."@en .

ids:RentalAgreement  rdf:type  owl:Class ;
        rdfs:subClassOf  ids:ContractAgreement ;
        rdfs:label       "Rental Agreement"@en ;
        rdfs:comment     "The ContractAgreement class representing the 'Data Rental' policy class."@en .

ids:SwapAgreement  rdf:type  owl:Class ;
        rdfs:subClassOf  ids:ContractAgreement ;
        rdfs:label       "Swap Agreement"@en ;
        rdfs:comment     "The ContractAgreement class representing the 'Data Swap' policy class."@en .

ids:RolebasedAgreement
        rdf:type         owl:Class ;
        rdfs:subClassOf  ids:ContractAgreement ;
        rdfs:label       "Role-restricted Data Usage Agreement"@en ;
        rdfs:comment     "The ContractAgreement class representing the 'Role-restricted Data Usage' policy class."@en .

ids:ConnectorbasedAgreement
        rdf:type         owl:Class ;
        rdfs:subClassOf  ids:ContractAgreement ;
        rdfs:label       "Connector-restricted Data Usage Agreement"@en ;
        rdfs:comment     "The ContractAgreement class representing the 'Connector-restricted Data Usage' policy class."@en .

ids:EventAgreement  rdf:type  owl:Class ;
        rdfs:subClassOf  ids:ContractAgreement ;
        rdfs:label       "Event-restricted Data Usage Agreement"@en ;
        rdfs:comment     "The ContractAgreement class representing the 'Event-restricted Usage Policy' policy class."@en .

ids:DurationAgreement
        rdf:type         owl:Class ;
        rdfs:subClassOf  ids:ContractAgreement ;
        rdfs:label       "Duration Agreement"@en ;
        rdfs:comment     "The ContractAgreement class representing the 'Duration-restricted Data Usage' policy class."@en .

ids:IntervalUsageAgreement
        rdf:type         owl:Class ;
        rdfs:subClassOf  ids:ContractAgreement ;
        rdfs:label       "Interval Usage Agreement"@en ;
        rdfs:comment     "The ContractAgreement class representing the 'Interval-restricted Data Usage' policy class."@en .

ids:SpatialAgreement  rdf:type  owl:Class ;
        rdfs:subClassOf  ids:ContractAgreement ;
        rdfs:label       "Spatial Usage Agreement"@en ;
        rdfs:comment     "The ContractAgreement class representing the 'Location Restricted Usage' policy class."@en .

ids:DeleteAfterIntervalAgreement
        rdf:type         owl:Class ;
        rdfs:subClassOf  ids:ContractAgreement ;
        rdfs:label       "Delete After Interval Agreement"@en ;
        rdfs:comment     "The ContractAgreement class representing the 'Interval-restricted Data Usage' policy class with the further obligation to delete the data."@en .

ids:DistributeEcryptedAgreement
        rdf:type         owl:Class ;
        rdfs:subClassOf  ids:ContractAgreement ;
        rdfs:label       "Distribute Encrypted Agreement"@en ;
        rdfs:comment     "The ContractAgreement class representing the 'Distribute only if Encrypted' policy class."@en .

ids:LoggingAgreement  rdf:type  owl:Class ;
        rdfs:subClassOf  ids:ContractAgreement ;
        rdfs:label       "Logging Agreement"@en ;
        rdfs:comment     "The ContractAgreement class representing the 'Local Logging' policy class."@en .

ids:NotificationAgreement
        rdf:type         owl:Class ;
        rdfs:subClassOf  ids:ContractAgreement ;
        rdfs:label       "Notification Agreement"@en ;
        rdfs:comment     "The ContractAgreement class representing the 'Remote Notifications' policy class."@en .

ids:SalesOffer  rdf:type  owl:Class ;
        rdfs:subClassOf  ids:ContractOffer ;
        rdfs:label       "Sales Offer"@en ;
        rdfs:comment     "The ContractOffer class representing the 'Perpetual Data Sale' policy class."@en .

ids:PurposeOffer  rdf:type  owl:Class ;
        rdfs:subClassOf  ids:ContractOffer ;
        rdfs:label       "Sales Offer"@en ;
        rdfs:comment     "The ContractOffer class representing the 'Purpose-restricted Data Usage' policy class."@en .

ids:SecurityOffer  rdf:type  owl:Class ;
        rdfs:subClassOf  ids:ContractOffer ;
        rdfs:label       "Security Offer"@en ;
        rdfs:comment     "The ContractOffer class representing the 'Security Level Restricted Policy' policy class."@en .

ids:NotMoreThanNOffer
        rdf:type         owl:Class ;
        rdfs:subClassOf  ids:ContractOffer ;
        rdfs:label       "Sales Offer"@en ;
        rdfs:comment     "The ContractOffer class representing the 'Restricted Number of Usages' policy class."@en .

ids:RentalOffer  rdf:type  owl:Class ;
        rdfs:subClassOf  ids:ContractOffer ;
        rdfs:label       "Sales Offer"@en ;
        rdfs:comment     "The ContractOffer class representing the 'Data Rental' policy class."@en .

ids:SwapOffer  rdf:type  owl:Class ;
        rdfs:subClassOf  ids:ContractOffer ;
        rdfs:label       "Sales Offer"@en ;
        rdfs:comment     "The ContractOffer class representing the 'Data Swap' policy class."@en .

ids:RolebasedOffer  rdf:type  owl:Class ;
        rdfs:subClassOf  ids:ContractOffer ;
        rdfs:label       "Role-restricted Data Usage Offer"@en ;
        rdfs:comment     "The ContractOffer class representing the 'Role-restricted Data Usage' policy class."@en .

ids:ConnectorbasedOffer
        rdf:type         owl:Class ;
        rdfs:subClassOf  ids:ContractOffer ;
        rdfs:label       "Connector-restricted Data Usage Offer"@en ;
        rdfs:comment     "The ContractOffer class representing the 'Connector-restricted Data Usage' policy class."@en .

ids:EventOffer  rdf:type  owl:Class ;
        rdfs:subClassOf  ids:ContractOffer ;
        rdfs:label       "Event-restricted Data Usage Offer"@en ;
        rdfs:comment     "The ContractOffer class representing the 'Event-restricted Usage Policy' policy class."@en .

ids:DurationOffer  rdf:type  owl:Class ;
        rdfs:subClassOf  ids:ContractOffer ;
        rdfs:label       "Sales Offer"@en ;
        rdfs:comment     "The ContractOffer class representing the 'Duration-restricted Data Usage' policy class."@en .

ids:IntervalUsageOffer
        rdf:type         owl:Class ;
        rdfs:subClassOf  ids:ContractOffer ;
        rdfs:label       "Sales Offer"@en ;
        rdfs:comment     "The ContractOffer class representing the 'Interval-restricted Data Usage' policy class."@en .

ids:SpatialOffer  rdf:type  owl:Class ;
        rdfs:subClassOf  ids:ContractOffer ;
        rdfs:label       "Spatial Usage Offer"@en ;
        rdfs:comment     "The ContractOffer class representing the 'Location Restricted Usage' policy class."@en .

ids:DeleteAfterIntervalOffer
        rdf:type         owl:Class ;
        rdfs:subClassOf  ids:ContractOffer ;
        rdfs:label       "Sales Offer"@en ;
        rdfs:comment     "The ContractOffer class representing the 'Interval-restricted Data Usage' policy class with the further obligation to delete the data."@en .

ids:DistributeEcryptedOffer
        rdf:type         owl:Class ;
        rdfs:subClassOf  ids:ContractOffer ;
        rdfs:label       "Distribute Encrypted Offer"@en ;
        rdfs:comment     "The ContractOffer class representing the 'Distribute only if Encrypted' policy class."@en .

ids:LoggingOffer  rdf:type  owl:Class ;
        rdfs:subClassOf  ids:ContractOffer ;
        rdfs:label       "Sales Offer"@en ;
        rdfs:comment     "The ContractOffer class representing the 'Local Logging' policy class."@en .

ids:NotificationOffer
        rdf:type         owl:Class ;
        rdfs:subClassOf  ids:ContractOffer ;
        rdfs:label       "Sales Offer"@en ;
        rdfs:comment     "The ContractOffer class representing the 'Remote Notifications' policy class."@en .

ids:SalesRequest  rdf:type  owl:Class ;
        rdfs:subClassOf  ids:ContractRequest ;
        rdfs:label       "Sales Request"@en ;
        rdfs:comment     "The ContractRequest class representing the 'Perpetual Data Sale' policy class."@en .

ids:PurposeRequest  rdf:type  owl:Class ;
        rdfs:subClassOf  ids:ContractRequest ;
        rdfs:label       "Sales Request"@en ;
        rdfs:comment     "The ContractRequest class representing the 'Purpose-restricted Data Usage' policy class."@en .

ids:SecurityRequest  rdf:type  owl:Class ;
        rdfs:subClassOf  ids:ContractRequest ;
        rdfs:label       "Security Request"@en ;
        rdfs:comment     "The ContractRequest class representing the 'Security Level Restricted Policy' policy class."@en .

ids:NotMoreThanNRequest
        rdf:type         owl:Class ;
        rdfs:subClassOf  ids:ContractRequest ;
        rdfs:label       "Sales Request"@en ;
        rdfs:comment     "The ContractRequest class representing the 'Restricted Number of Usages' policy class."@en .

ids:RentalRequest  rdf:type  owl:Class ;
        rdfs:subClassOf  ids:ContractRequest ;
        rdfs:label       "Sales Request"@en ;
        rdfs:comment     "The ContractRequest class representing the 'Data Rental' policy class."@en .

ids:SwapRequest  rdf:type  owl:Class ;
        rdfs:subClassOf  ids:ContractRequest ;
        rdfs:label       "Sales Request"@en ;
        rdfs:comment     "The ContractRequest class representing the 'Data Swap' policy class."@en .

ids:RolebasedRequest  rdf:type  owl:Class ;
        rdfs:subClassOf  ids:ContractRequest ;
        rdfs:label       "Role-restricted Data Usage Request"@en ;
        rdfs:comment     "The ContractRequest class representing the 'Role-restricted Data Usage' policy class."@en .

ids:ConnectorbasedRequest
        rdf:type         owl:Class ;
        rdfs:subClassOf  ids:ContractRequest ;
        rdfs:label       "Connector-restricted Data Usage Request"@en ;
        rdfs:comment     "The ContractRequest class representing the 'Connector-restricted Data Usage' policy class."@en .

ids:EventRequest  rdf:type  owl:Class ;
        rdfs:subClassOf  ids:ContractRequest ;
        rdfs:label       "Event-restricted Data Usage Request"@en ;
        rdfs:comment     "The ContractRequest class representing the 'Event-restricted Usage Policy' policy class."@en .

ids:DurationRequest  rdf:type  owl:Class ;
        rdfs:subClassOf  ids:ContractRequest ;
        rdfs:label       "Sales Request"@en ;
        rdfs:comment     "The ContractRequest class representing the 'Duration-restricted Data Usage' policy class."@en .

ids:IntervalUsageRequest
        rdf:type         owl:Class ;
        rdfs:subClassOf  ids:ContractRequest ;
        rdfs:label       "Sales Request"@en ;
        rdfs:comment     "The ContractRequest class representing the 'Interval-restricted Data Usage' policy class."@en .

ids:SpatialRequest  rdf:type  owl:Class ;
        rdfs:subClassOf  ids:ContractRequest ;
        rdfs:label       "Spatial Usage Request"@en ;
        rdfs:comment     "The ContractRequest class representing the 'Location Restricted Usage' policy class."@en .

ids:DeleteAfterIntervalRequest
        rdf:type         owl:Class ;
        rdfs:subClassOf  ids:ContractRequest ;
        rdfs:label       "Sales Request"@en ;
        rdfs:comment     "The ContractRequest class representing the 'Interval-restricted Data Usage' policy class with the further obligation to delete the data."@en .

ids:DistributeEcryptedRequest
        rdf:type         owl:Class ;
        rdfs:subClassOf  ids:ContractRequest ;
        rdfs:label       "Distribute Encrypted Request"@en ;
        rdfs:comment     "The ContractRequest class representing the 'Distribute only if Encrypted' policy class."@en .

ids:LoggingRequest  rdf:type  owl:Class ;
        rdfs:subClassOf  ids:ContractRequest ;
        rdfs:label       "Sales Request"@en ;
        rdfs:comment     "The ContractRequest class representing the 'Local Logging' policy class."@en .

ids:NotificationRequest
        rdf:type         owl:Class ;
        rdfs:subClassOf  ids:ContractRequest ;
        rdfs:label       "Sales Request"@en ;
        rdfs:comment     "The ContractRequest class representing the 'Remote Notifications' policy class."@en .
@prefix owl:   <http://www.w3.org/2002/07/owl#> .
@prefix rdf:   <http://www.w3.org/1999/02/22-rdf-syntax-ns#> .
@prefix rdfs:  <http://www.w3.org/2000/01/rdf-schema#> .
@prefix xsd:   <http://www.w3.org/2001/XMLSchema#> .
@prefix dct:   <http://purl.org/dc/terms/> .
@prefix ids:   <https://w3id.org/idsa/core/> .

ids:RequestMessage  rdf:type  owl:Class ;
        rdfs:subClassOf  ids:Message ;
        rdfs:label       "Request Message"@en ;
        rdfs:comment     "Client-generated message initiating a communication, motivated by a certain reason and with an answer expected."@en .

ids:ResponseMessage  rdf:type  owl:Class ;
        rdfs:subClassOf  ids:Message ;
        rdfs:label       "Response Message"@en ;
        rdfs:comment     "Response messages hold information about the reaction of a recipient to a formerly sent command or event. They must be correlated to this message."@en .

ids:NotificationMessage
        rdf:type         owl:Class ;
        rdfs:subClassOf  ids:Message ;
        rdfs:label       "Notification Message"@en ;
        rdfs:comment     "Event messages are informative and no response is expected by the sender."@en .

ids:CommandMessage  rdf:type  owl:Class ;
        rdfs:subClassOf  ids:RequestMessage ;
        rdfs:label       "Command Message"@en ;
        rdfs:comment     "Command messages are usually sent when a response is expected by the sender. Changes state on the recipient side. Therefore, commands are not 'safe' in the sense of REST."@en .

ids:ResultMessage  rdf:type  owl:Class ;
        rdfs:subClassOf  ids:ResponseMessage ;
        rdfs:label       "Result Message"@en ;
        rdfs:comment     "Result messages are intended to annotate the results of a query command. "@en .

ids:RejectionMessage  rdf:type  owl:Class ;
        rdfs:subClassOf  ids:ResponseMessage ;
        rdfs:label       "Rejection Message"@en ;
        rdfs:comment     "Rejection messages are specialized response messages that notify the sender of a message that processing of this message has failed."@en .

ids:RejectionReason  rdf:type  owl:Class ;
        rdfs:label    "RejectionReason"@en ;
        rdfs:comment  "Class of reasons that might lead to issuing a Rejection message."@en .

ids:rejectionReason  rdf:type  owl:ObjectProperty ;
        rdfs:domain   ids:RejectionMessage ;
        rdfs:range    ids:RejectionReason ;
        rdfs:label    "rejectionReason"@en ;
        rdfs:comment  "Specifies the reason of the rejection."@en .

ids:DescriptionRequestMessage
        rdf:type         owl:Class ;
        rdfs:subClassOf  ids:RequestMessage ;
        rdfs:label       "Description Request Message"@en ;
        rdfs:comment     "Message requesting metadata. If no URI is supplied via the ids:requestedElement field, this messages is treated like a self-description request and the recipient should return its self-description via an ids:DescriptionResponseMessage. However, if a URI is supplied, the Connector should either return metadata about the requested element via an ids:DescriptionResponseMessage, or send an ids:RejectionMessage, e.g., because the element was not found."@en .

ids:DescriptionResponseMessage
        rdf:type         owl:Class ;
        rdfs:subClassOf  ids:ResponseMessage ;
        rdfs:label       "Description Response Message"@en ;
        rdfs:comment     "Message containing the metadata, which a Connector previously requested via the ids:DescriptionRequestMessage, in its payload."@en .

ids:requestedElement  rdf:type  owl:DatatypeProperty ;
        rdfs:label    "requested Element"@en ;
        rdfs:comment  "The element whose metadata is requested. "@en ;
        rdfs:domain   ids:DescriptionRequestMessage ;
        rdfs:range    xsd:anyURI .

ids:ConnectorNotificationMessage
        rdf:type         owl:Class ;
        rdfs:subClassOf  ids:NotificationMessage ;
        rdfs:label       "Connector Notification Message"@en ;
        rdfs:comment     "Superclass of all messages, indicating a change of a connector's conditions."@en .

ids:ConnectorUpdateMessage
        rdf:type         owl:Class ;
        rdfs:subClassOf  ids:ConnectorNotificationMessage ;
        rdfs:label       "Connector Update Message"@en ;
        rdfs:comment     "Event notifying the recipient(s) about the availability and current configuration of a connector. The payload of the message must contain the updated connector's self-description."@en .

ids:ConnectorUnavailableMessage
        rdf:type         owl:Class ;
        rdfs:subClassOf  ids:ConnectorNotificationMessage ;
        rdfs:label       "Connector Unavailable Message"@en ;
        rdfs:comment     "Event notifying the recipient(s) that a connector will be unavailable. The same connector may be available again in the future."@en .

ids:ConnectorCertificateGrantedMessage
        rdf:type         owl:Class ;
        rdfs:subClassOf  ids:ConnectorNotificationMessage ;
        rdfs:label       "Connector Certificate Granted Message"@en ;
        rdfs:comment     "Whenever a Connector has been successfully certified by the Certification Body, the Identity Provider can use this message to notify Infrastructure Components."@en .

ids:ConnectorCertificateRevokedMessage
        rdf:type         owl:Class ;
        rdfs:subClassOf  ids:ConnectorNotificationMessage ;
        rdfs:label       "Connector Certificate Revoked Message"@en ;
        rdfs:comment     "Indicates that a (previously certified) Connector is no more certified. This could happen, for instance, if the Certification Body revokes a granted certificate or if the certificate just expires."@en .

ids:affectedConnector
        rdf:type      owl:ObjectProperty ;
        rdfs:label    "affected Connector"@en ;
        rdfs:domain   ids:ConnectorNotificationMessage ;
        rdfs:range    ids:Connector ;
        rdfs:comment  "References the connector that is affected by the runtime condition change."@en .

ids:ParticipantNotificationMessage
        rdf:type         owl:Class ;
        rdfs:subClassOf  ids:NotificationMessage ;
        rdfs:label       "Participant Notification Message"@en ;
        rdfs:comment     "Superclass of all messages, indicating a change of a particpants's conditions."@en .

ids:ParticipantUpdateMessage
        rdf:type         owl:Class ;
        rdfs:subClassOf  ids:ParticipantNotificationMessage ;
        rdfs:label       "Participant Available Message"@en ;
        rdfs:comment     "Event notifying the recipient(s) about the availability and current description of a participant. The payload of the message must contain the participant's self-description."@en .

ids:ParticipantUnavailableMessage
        rdf:type         owl:Class ;
        rdfs:subClassOf  ids:ParticipantNotificationMessage ;
        rdfs:label       "Participant Unavailable Message"@en ;
        rdfs:comment     "Event notifying the recipient(s) that a participant will be unavailable. The same participant may be available again in the future."@en .

ids:ParticipantCertificateGrantedMessage
        rdf:type         owl:Class ;
        rdfs:subClassOf  ids:ParticipantNotificationMessage ;
        rdfs:label       "Participant Certificate Granted Message"@en ;
        rdfs:comment     "Whenever a Participant has been successfully certified by the Certification Body, the Identity Provider can use this message to notify Infrastructure Components."@en .

ids:ParticipantCertificateRevokedMessage
        rdf:type         owl:Class ;
        rdfs:subClassOf  ids:ParticipantNotificationMessage ;
        rdfs:label       "Participant Certificate Revoked Message"@en ;
        rdfs:comment     "Indicates that a (previously certified) Participant is no more certified. This could happen, for instance, if the Certification Body revokes a granted certificate or if the certificate just expires."@en .

ids:affectedParticipant
        rdf:type      owl:ObjectProperty ;
        rdfs:label    "affected Participant"@en ;
        rdfs:domain   ids:ParticipantNotificationMessage ;
        rdfs:range    ids:Participant ;
        rdfs:comment  "References the participant that is referenced in the participant-related notification messages."@en .

ids:revocationReason  rdf:type  owl:DatatypeProperty ;
        rdfs:label  "Revocation Reason"@en .

_:b35   rdf:first  ids:ConnectorCertificateRevokedMessage ;
        rdf:rest   _:b36 .

_:b36   rdf:first  ids:ParticipantCertificateRevokedMessage ;
        rdf:rest   rdf:nil .

_:b37   owl:unionOf  _:b35 .

ids:revocationReason  rdfs:domain  _:b37 ;
        rdfs:range    xsd:string ;
        rdfs:comment  "Plain Text containing the reason for revoking an existing certificate of either a connector or participant."@en .

ids:QueryMessage  rdf:type  owl:Class ;
        rdfs:subClassOf  ids:RequestMessage ;
        rdfs:label       "Query Message"@en ;
        rdfs:comment     "Query message intended to be consumed by a component."@en .

ids:QueryLanguage  rdf:type  owl:Class ;
        rdfs:label    "QueryLanguage"@en ;
        rdfs:comment  "Class of query languages in which query strings may be formalized."@en .

ids:QueryScope  rdf:type  owl:Class ;
        rdfs:label    "Query Scope"@en ;
        rdfs:comment  "Class of scopes that may limit the space of query results, e.g., ALL, ACTIVE_ONLY."@en .

ids:QueryTarget  rdf:type  owl:Class ;
        rdfs:label    "Query Target"@en ;
        rdfs:comment  "Class of recipients of a query message, e.g., BROKER, APPSTORE, ANY."@en .

ids:queryLanguage  rdf:type  owl:ObjectProperty ;
        rdfs:domain   ids:QueryMessage ;
        rdfs:range    ids:QueryLanguage ;
        rdfs:label    "queryLanguage"@en ;
        rdfs:comment  "This property specifies the language of the query."@en .

ids:queryScope  rdf:type  owl:ObjectProperty ;
        rdfs:label    "queryScope"@en ;
        rdfs:domain   ids:QueryMessage ;
        rdfs:range    ids:QueryScope ;
        rdfs:comment  "Refers to the scope property of a query message, see ids:QueryScope."@en .

ids:recipientScope  rdf:type  owl:ObjectProperty ;
        rdfs:label    "recipient scope"@en ;
        rdfs:domain   ids:QueryMessage ;
        rdfs:range    ids:QueryTarget ;
        rdfs:comment  "Refers to the target property of a query message, see ids:QueryTarget."@en .

ids:ContractRequestMessage
        rdf:type         owl:Class ;
        rdfs:subClassOf  ids:RequestMessage ;
        rdfs:label       "Contract Request Message"@en ;
        rdfs:comment     "Message containing a suggested content contract (as offered by the data consumer to the data provider) in the associated payload (which is an instance of ids:ContractRequest)."@en .

ids:ContractResponseMessage
        rdf:type         owl:Class ;
        rdfs:subClassOf  ids:ResponseMessage ;
        rdfs:label       "Contract Response Message"@en ;
        rdfs:comment     "Message containing a response to a contract request (of a data consumer) in form of a counter-proposal of a contract in the associated payload (which is an instance of ids:ContractOffer). "@en .

ids:ContractOfferMessage
        rdf:type         owl:Class ;
        rdfs:subClassOf  ids:NotificationMessage ;
        rdfs:label       "Contract Offer Message"@en ;
        rdfs:comment     "Message containing a offered content contract (as offered by a data provider to the data consumer) in the associated payload (which is an instance of ids:ContractOffer). In contrast to the ids:ContractResponseMessage, the ids:ContractOfferMessage is not related to a previous contract "@en .

ids:ContractAgreementMessage
        rdf:type         owl:Class ;
        rdfs:subClassOf  ids:ResponseMessage ;
        rdfs:label       "Contract Agreement Message"@en ;
        rdfs:comment     "Message containing a contract, as an instance of ids:ContractAgreement, with resource access modalities on which two parties have agreed in the payload."@en .

ids:ContractRejectionMessage
        rdf:type         owl:Class ;
        rdfs:subClassOf  ids:RejectionMessage ;
        rdfs:label       "Contract Rejection Message"@en ;
        rdfs:comment     "Message indicating rejection of a contract."@en .

ids:ContractSupplementMessage
        rdf:type         owl:Class ;
        rdfs:subClassOf  ids:NotificationMessage ;
        rdfs:label       "Contract Supplement Message"@en ;
        rdfs:comment     "Message containing supplemental information to access resources of a contract (e.g., resource access tokens)."@en .

ids:contractRejectionReason
        rdf:type      owl:DatatypeProperty ;
        rdfs:label    "Contract Rejection Reason"@en ;
        rdfs:domain   ids:ContractRejectionMessage ;
        rdfs:range    xsd:string ;
        rdfs:comment  "Human-readable text describing the reason for contract rejection."@en .

ids:AccessTokenRequestMessage
        rdf:type         owl:Class ;
        rdfs:subClassOf  ids:RequestMessage ;
        rdfs:label       "AccessToken Request Message"@en ;
        rdfs:comment     "Message requesting an access token. This is intended for point-to-point communication with, e.g., Brokers."@en .

ids:AccessTokenResponseMessage
        rdf:type         owl:Class ;
        rdfs:subClassOf  ids:ResponseMessage ;
        rdfs:label       "Access Token Response"@en ;
        rdfs:comment     "Response to an access token request, intended for point-to-point communication."@en .

ids:ResourceNotificationMessage
        rdf:type         owl:Class ;
        rdfs:subClassOf  ids:NotificationMessage ;
        rdfs:label       "Resource Notification Message"@en ;
        rdfs:comment     "Superclass of all messages, indicating a change of a resource."@en .

ids:ResourceUpdateMessage
        rdf:type         owl:Class ;
        rdfs:subClassOf  ids:ResourceNotificationMessage ;
        rdfs:label       "Resource Update Message"@en ;
        rdfs:comment     "Message indicating the availability and current description of a specific resource. The resource must be present in the payload of this message."@en .

ids:ResourceUnavailableMessage
        rdf:type         owl:Class ;
        rdfs:subClassOf  ids:ResourceNotificationMessage ;
        rdfs:label       "Resource Unavailable Message"@en ;
        rdfs:comment     "Message indicating that a specific resource is unavailable. The same resource may be available again in the future."@en .

ids:affectedResource  rdf:type  owl:ObjectProperty ;
        rdfs:domain   ids:ResourceNotificationMessage ;
        rdfs:range    ids:Resource ;
        rdfs:label    "affected Resource"@en ;
        rdfs:comment  "The affected resource that is referenced in the resource-related notification messages. "@en .

ids:InvokeOperationMessage
        rdf:type         owl:Class ;
        rdfs:subClassOf  ids:RequestMessage ;
        rdfs:label       "Invoke Operation Message"@en ;
        rdfs:comment     "Message requesting the recipient to invoke a specific operation."@en .

ids:operationReference
        rdf:type      owl:DatatypeProperty ;
        rdfs:domain   ids:InvokeOperationMessage ;
        rdfs:range    xsd:anyURI ;
        rdfs:label    "Operation Reference"@en ;
        rdfs:comment  "References the operation to be invoked on the recipient's side by an URI."@en .

ids:RequestInProcessMessage
        rdf:type         owl:Class ;
        rdfs:subClassOf  ids:NotificationMessage ;
        rdfs:label       "Request In Process Message"@en ;
        rdfs:comment     "Notification that a request has been accepted and is being processed."@en .

ids:MessageProcessedNotificationMessage
        rdf:type         owl:Class ;
        rdfs:subClassOf  ids:NotificationMessage ;
        rdfs:label       "Message Processed Notification Message"@en ;
        rdfs:comment     "Notification that a message has been successfully processed (i.e. not ignored or rejected)."@en .

ids:OperationResultMessage
        rdf:type         owl:Class ;
        rdfs:subClassOf  ids:ResponseMessage ;
        rdfs:label       "Operation Result Message"@en ;
        rdfs:comment     "Message indicating that the result of a former InvokeOperation message is available. May transfer the result data in its associated payload section."@en .

ids:ArtifactRequestMessage
        rdf:type         owl:Class ;
        rdfs:subClassOf  ids:RequestMessage ;
        rdfs:label       "Artifact Request Message"@en ;
        rdfs:comment     "Message asking for retrieving the specified Artifact as the payload of an ArtifactResponse message."@en .

ids:ArtifactResponseMessage
        rdf:type         owl:Class ;
        rdfs:subClassOf  ids:ResponseMessage ;
        rdfs:label       "Artifact Response Message"@en ;
        rdfs:comment     "Message that follows up a RetrieveArtifact Message and contains the Artifact's data in the payload section."@en .

ids:requestedArtifact
        rdf:type      owl:ObjectProperty ;
        rdfs:domain   ids:ArtifactRequestMessage ;
        rdfs:range    ids:Artifact ;
        rdfs:label    "Requested Artifact"@en ;
        rdfs:comment  "References an artifact in the context of a request."@en .

ids:UploadMessage  rdf:type  owl:Class ;
        rdfs:subClassOf  ids:RequestMessage ;
        rdfs:label       "Upload Message"@en ;
        rdfs:comment     "Message used to upload a data to a recipient. Payload contains data."@en .

ids:UploadResponseMessage
        rdf:type         owl:Class ;
        rdfs:subClassOf  ids:ResponseMessage ;
        rdfs:label       "Upload Response Message"@en ;
        rdfs:comment     "Message that follows up a UploadMessage and contains the upload confirmation."@en .

ids:ParticipantRequestMessage
        rdf:type         owl:Class ;
        rdfs:subClassOf  ids:RequestMessage ;
        owl:deprecated   true ;
        rdfs:label       "Participant Request Message (Deprecated)"@en ;
        rdfs:comment     "This class is deprecated. Use ids:DescriptionRequestMessage instead. Message asking for retrieving the specified Participants information as the payload of an ids:ParticipantResponse message."@en .

ids:ParticipantResponseMessage
        rdf:type         owl:Class ;
        rdfs:subClassOf  ids:ResponseMessage ;
        owl:deprecated   true ;
        rdfs:label       "Participant Response Message (Deprecated)"@en ;
        rdfs:comment     "This class is deprecated. Use ids:DescriptionResponseMessage instead. ParticipantResponseMessage follows up a ParticipantRequestMessage and contains the Participant's information in the payload section."@en .

ids:requestedParticipant
        rdf:type        owl:ObjectProperty ;
        owl:deprecated  true ;
        rdfs:domain     ids:ParticipantRequestMessage ;
        rdfs:range      ids:Participant ;
        rdfs:label      "Requested Participant (Deprecated)"@en ;
        rdfs:comment    "This property is deprecated. Use ids:requestedElement along with ids:DescriptionRequestMessage instead. References a Participant in the context of a request."@en .

ids:LogMessage  rdf:type  owl:Class ;
        rdfs:subClassOf  ids:NotificationMessage ;
        rdfs:label       "Log Message"@en ;
        rdfs:comment     "Log Message which can be used to transfer logs e.g., to the clearing house."@en .

ids:AppRegistrationRequestMessage
        rdf:type         owl:Class ;
        rdfs:subClassOf  ids:RequestMessage ;
        rdfs:label       "App Registration Request Message"@en ;
        rdfs:comment     "Message that asks for registration or update of a data app to the App Store. Payload contains app-related metadata (instance of class ids:AppResource). Message header may contain an app identifier parameter of a prior registered data app. If the app identifier is supplied, the message should be interpreted as a registration for an app update. Otherwise this message is used to register a new app. "@en .

ids:affectedDataApp  rdf:type  owl:ObjectProperty ;
        rdfs:domain   ids:AppRegistrationRequestMessage ;
        rdfs:range    ids:AppResource ;
        rdfs:label    "affected AppResource"@en ;
        rdfs:comment  "The affected data app that is referenced in the App-related messages. "@en .

ids:AppRegistrationResponseMessage
        rdf:type         owl:Class ;
        rdfs:subClassOf  ids:ResponseMessage ;
        rdfs:label       "App Registration Response Message"@en ;
        rdfs:comment     "Message that follows up an AppRegistrationRequestMessage and contains the app registration confimation."@en .

ids:AppUploadMessage  rdf:type  owl:Class ;
        rdfs:subClassOf  ids:UploadMessage ;
        rdfs:label       "App Upload Message"@en ;
        rdfs:comment     "Message that usually follows a AppRegistrationResponseMessage and is used to upload a data app to the app store. Payload contains data app. Note that the message must refer to the prior sent, corresponding AppResource instance. The IRI of the ids:appArtifactReference must must match the IRI of the artifact which is the value for the ids:instance property. The ids:instance is specific for each representation. Therefore, if someone wants to upload multiple representations for an app, he has to state them using multiple ids:instance properties inside the AppRepresentation (and therefore inside the AppResource). Otherwise no mapping between payload and app metadata can be achieved."@en .

ids:AppUploadResponseMessage
        rdf:type         owl:Class ;
        rdfs:subClassOf  ids:UploadResponseMessage ;
        rdfs:label       "App Upload Response Message"@en ;
        rdfs:comment     "Message that follows up an AppUploadMessage and contains the app upload confimation."@en .

ids:appArtifactReference
        rdf:type      owl:ObjectProperty ;
        rdfs:domain   ids:AppUploadMessage ;
        rdfs:range    ids:Artifact ;
        rdfs:label    "app artifact reference"@en ;
        rdfs:comment  "IRI reference to the ids:Artifact, whose corresponding data is transfered as payload of the AppUploadMessage. The Artifact IRI reference must match the IRI of the instance IRI for the corresponding ids:AppRepresentation."@en .

ids:AppNotificationMessage
        rdf:type         owl:Class ;
        rdfs:subClassOf  ids:ResourceNotificationMessage ;
        rdfs:label       "App Notification Message"@en ;
        rdfs:comment     "Superclass of all messages, indicating a change of a DataApp. Unlike Resource-related Messages, AppNotificationMessages should lead to a state change for an app at the recipient, the AppStore."@en .

ids:AppAvailableMessage
        rdf:type         owl:Class ;
        rdfs:subClassOf  ids:AppNotificationMessage ;
        rdfs:label       "App Available Message"@en ;
        rdfs:comment     "Message indicating that a specific App should be available (again) in the AppStore."@en .

ids:AppUnavailableMessage
        rdf:type         owl:Class ;
        rdfs:subClassOf  ids:AppNotificationMessage ;
        rdfs:label       "App Unavailable Message"@en ;
        rdfs:comment     "Message indicating that a specific App should be unavailable in the AppStore."@en .

ids:AppDeleteMessage  rdf:type  owl:Class ;
        rdfs:subClassOf  ids:AppNotificationMessage ;
        rdfs:label       "App Delete Message"@en ;
        rdfs:comment     "Message indicating that an App should be deleted from the AppStore."@en .
@prefix owl:   <http://www.w3.org/2002/07/owl#> .
@prefix rdfs:  <http://www.w3.org/2000/01/rdf-schema#> .
@prefix dct:   <http://purl.org/dc/terms/> .
@prefix dcat:  <http://www.w3.org/ns/dcat#> .
@prefix ids:   <https://w3id.org/idsa/core/> .
@prefix xsd:   <http://www.w3.org/2001/XMLSchema#> .

ids:DataRepresentation
        rdf:type         owl:Class ;
        rdfs:subClassOf  dcat:Distribution ;
        rdfs:label       "Data representation"@en ;
        rdfs:comment     "Physical representation of (structured) data."@en .

ids:dataType  rdf:type  owl:DatatypeProperty ;
        rdfs:domain   ids:DataRepresentation ;
        rdfs:range    xsd:anyURI ;
        rdfs:label    "Data type"@en ;
        rdfs:comment  "Indicates the data type of the Representation."@en .

ids:dataTypeSchema  rdf:type  owl:ObjectProperty ;
        rdfs:domain   ids:DataRepresentation ;
        rdfs:range    ids:Resource ;
        rdfs:label    "Data Type Schema"@en ;
        rdfs:comment  "Indicates the data type schema of the Representation."@en .

ids:TextRepresentation
        rdf:type         owl:Class ;
        rdfs:subClassOf  dcat:Distribution ;
        rdfs:label       "Text representation"@en ;
        rdfs:comment     "Representation of a textual content."@en .

ids:AudioRepresentation
        rdf:type         owl:Class ;
        rdfs:subClassOf  dcat:Distribution ;
        rdfs:label       "Audio Representation"@en ;
        rdfs:comment     "Audio representation"@en .

ids:samplingRate  rdf:type  owl:DatatypeProperty ;
        rdfs:domain   ids:AudioRepresentation ;
        rdfs:range    xsd:decimal ;
        rdfs:label    "sampling rate"@en ;
        rdfs:comment  "Audio sampling rate."@en .

ids:ImageRepresentation
        rdf:type         owl:Class ;
        rdfs:subClassOf  dcat:Distribution ;
        rdfs:label       "Image Representation"@en ;
        rdfs:comment     "Image representation"@en .

ids:width  rdf:type   owl:DatatypeProperty ;
        rdfs:domain   ids:ImageRepresentation ;
        rdfs:range    xsd:decimal ;
        rdfs:label    "width"@en ;
        rdfs:comment  "Width of the visible frame."@en .

ids:height  rdf:type  owl:DatatypeProperty ;
        rdfs:domain   ids:ImageRepresentation ;
        rdfs:range    xsd:decimal ;
        rdfs:label    "height"@en ;
        rdfs:comment  "Height of the visible frame."@en .

ids:VideoRepresentation
        rdf:type         owl:Class ;
        rdfs:subClassOf  dcat:Distribution ;
        rdfs:label       "Video Representation"@en ;
        rdfs:comment     "Video representation"@en .

ids:frameRate  rdf:type  owl:DatatypeProperty ;
        rdfs:domain   ids:VideoRepresentation ;
        rdfs:range    xsd:decimal ;
        rdfs:label    "frame rate"@en ;
        rdfs:comment  "Video frame rate, as frames/second."@en .

ids:SoftwareRepresentation
        rdf:type         owl:Class ;
        rdfs:subClassOf  dcat:Distribution ;
        rdfs:label       "Software Representation"@en ;
        rdfs:comment     "Software representation"@en .

ids:AppRepresentation
        rdf:type         owl:Class ;
        rdfs:subClassOf  ids:SoftwareRepresentation ;
        rdfs:label       "App Representation"@en ;
        rdfs:comment     "App representation"@en .

ids:dataAppInformation
        rdf:type      owl:ObjectProperty ;
        rdfs:label    "data app information"@en ;
        rdfs:domain   ids:AppRepresentation ;
        rdfs:range    ids:DataApp ;
        rdfs:comment  "Information about the concrete data app implementation"@en .

ids:dataAppDistributionService
        rdf:type      owl:DatatypeProperty ;
        rdfs:label    "data app distribution service"@en ;
        rdfs:comment  "IRI reference to storage and distribution system for the correspending data app. Unlinke regular representations for IDS resources, a data app may not be retrieved directly from a connector but from a separate registry instead."@en ;
        rdfs:domain   ids:AppRepresentation ;
        rdfs:range    xsd:anyURI .

ids:dataAppRuntimeEnvironment
        rdf:type      owl:DatatypeProperty ;
        rdfs:label    "data app runtime environment"@en ;
        rdfs:domain   ids:AppRepresentation ;
        rdfs:range    xsd:string ;
        rdfs:comment  "Runtime environment of a data app, e.g., software (or hardware) required to run the app."@en .
@prefix owl:   <http://www.w3.org/2002/07/owl#> .
@prefix rdfs:  <http://www.w3.org/2000/01/rdf-schema#> .
@prefix dct:   <http://purl.org/dc/terms/> .
@prefix ids:   <https://w3id.org/idsa/core/> .
@prefix skos:  <http://www.w3.org/2004/02/skos/core#> .

ids:DataResource  rdf:type  owl:Class ;
        rdfs:subClassOf  ids:Resource ;
        rdfs:label       "Data Resource"@en ;
        rdfs:comment     "Resource (at least partially) comprising data content."@en .

ids:TextResource  rdf:type  owl:Class ;
        rdfs:subClassOf  ids:Resource ;
        rdfs:label       "Text Resource"@en ;
        rdfs:comment     "Resource (at least partially) comprising textual content."@en .

ids:AudioResource  rdf:type  owl:Class ;
        rdfs:subClassOf  ids:Resource ;
        rdfs:label       "Audio Resource"@en ;
        rdfs:comment     "Resource (at least partially) comprising audio content."@en .

ids:ImageResource  rdf:type  owl:Class ;
        rdfs:subClassOf  ids:Resource ;
        rdfs:label       "Image Resource"@en ;
        rdfs:comment     "Resource (at least partially) comprising image content."@en .

ids:VideoResource  rdf:type  owl:Class ;
        rdfs:subClassOf  ids:Resource ;
        rdfs:label       "Video Resource"@en ;
        rdfs:comment     "Resource (at least partially) comprising video content."@en .

ids:SoftwareResource  rdf:type  owl:Class ;
        rdfs:subClassOf  ids:Resource ;
        rdfs:label       "Software Resource"@en ;
        rdfs:comment     "Resource (at least partially) comprising Software."@en .

ids:AppResource  rdf:type  owl:Class ;
        rdfs:subClassOf  ids:Resource ;
        rdfs:label       "App Resource"@en ;
        rdfs:comment     "Resource comprising IDS data apps."@en .
